Theory of finite maps now builds in Kan.0.

src/finite_map/finite_mapScript.sml
@@ -12,7 +12,7 @@
 (* @inproceedings{P-Collins-FMAP,  					  *)
 (*    author = {Graham Collins and Donald Syme},  			  *)
 (*    editor = {E. Thomas Schubert and Phillip J. Windley   		  *)
-(*              and Hames Alves-Foss},  				  *)
+(*              and James Alves-Foss},  				  *)
 (*    booktitle={Higher Order Logic Theorem Proving and its Applications},*)
 (*    publisher = {Springer-Verlag},  					  *)
 (*    series = {Lecture Notes in Computer Science},  			  *)
@@ -27,432 +27,390 @@
 
 structure finite_mapScript =
 struct
+(* interactive use:
 
-open HolKernel Parse basicHol90Lib
-     ind_defLib oneTheory sumTheory pairTheory numLib Num_induct;
-infix THEN THENL THENC ORELSE ORELSEC THEN_TCL ORELSE_TCL ## |->;
+ app load ["IndDefLib", "PairedDefinition", "numLib", "NonRecSize",
+           "oneTheory", "Q"];
+
+ open IndDefLib oneTheory sumTheory pairTheory PairedDefinition 
+      numTheory prim_recTheory numLib;
+*)
+
+
+open HolKernel Parse boolLib PairedDefinition IndDefLib numLib
+     oneTheory sumTheory pairTheory numTheory prim_recTheory;
+
 infixr -->;
+infix THEN THENL THENC ORELSE ORELSEC THEN_TCL ORELSE_TCL ## |->; 
 
-(* Definition of a finite map *)
 
 val _ = new_theory "finite_map";
 
+(*---------------------------------------------------------------------------
+        Definition of a finite map
 
-(* The representation is the type 'a -> ('b + one) where only a finite
- number of the 'a map to a 'b and the rest map to one. *)
+    The representation is the type 'a -> ('b + one) where only a finite
+    number of the 'a map to a 'b and the rest map to one.  We define a
+    notion of finiteness inductively.
+ --------------------------------------------------------------------------- *)
 
-
-(* We define an notion of finiteness inductively. *)
-
-val {rules=is_fmap_rules, induction=is_fmap_ind} =
- let val is_fmap = Term`is_fmap :('a -> 'b + one) -> bool`
-     infix ----------------------------------------;
-     fun (x ---------------------------------------- y) = (x,y)
-  in
-   indDefine "isfmap"
-
-      [ ([],                                  [])
-        ----------------------------------------
-               `^is_fmap (\a. (INR one))`       ,
+val (rules,ind,cases) = 
+gen_new_inductive_definition 
+  bool_monoset
+  (Term`is_fmap (\a. INR one) 
+   /\  (!f a b. is_fmap f ==> is_fmap (\x. if x=a then INL b else f x))`);
 
 
-          ([`^is_fmap f`                   ],[])
-        ----------------------------------------
-        `^is_fmap (\x. (x = a) => INL b | f x)` ]  Prefix  (`^is_fmap f`,[])
-   end;
+val rule_list as [is_fmap_empty, is_fmap_update] = CONJUNCTS rules;
 
-val [is_fmap_empty, is_fmap_update] = is_fmap_rules;
+val is_fmap_RULE_INDUCT_TAC = RULE_INDUCT_THEN ind STRIP_ASSUME_TAC;
 
-val strong_is_fmap_ind =
-  ind_defLib.derive_strong_induction(is_fmap_rules, is_fmap_ind);
-
-val is_fmap_RULE_INDUCT_TAC =
-   ind_defLib.RULE_INDUCT_THEN is_fmap_ind STRIP_ASSUME_TAC STRIP_ASSUME_TAC;
+val strong_ind = derive_strong_induction(rule_list, ind);
 
 
-(* Existence Theorem *)
+(*---------------------------------------------------------------------------
+        Existence theorem; type definition
+ ---------------------------------------------------------------------------*)
 
-val EXISTENCE_THM = prove
- (Term`?x:'a -> 'b + one.
-    (\f:'a -> 'b + one . is_fmap f) x `,
-EXISTS_TAC (Term`\x:'a. (INR one):'b + one`) THEN
-BETA_TAC THEN
-REWRITE_TAC [ is_fmap_empty ]);
+val EXISTENCE_THM = Q.prove
+(`?x:'a -> 'b + one. is_fmap x`,
+EXISTS_TAC (Term`\x:'a. (INR one):'b + one`) 
+ THEN REWRITE_TAC [is_fmap_empty]);
 
-val fmap_TY_DEF =
-    new_type_definition{name = "fmap",
-                        pred =Term`\f:'a -> 'b + one . is_fmap f`,
-                        inhab_thm = EXISTENCE_THM};
-val _ = add_infix_type{Prec = 50, ParseName = SOME "|->", Assoc = RIGHT,
-                       Name = "fmap"};
+val fmap_TY_DEF = new_type_definition("fmap", EXISTENCE_THM);
+
+val _ = add_infix_type
+           {Prec = 50, 
+            ParseName = SOME "|->", 
+            Assoc = RIGHT,
+            Name = "fmap"};
 
 (* --------------------------------------------------------------------- *)
-(* Define bijections  				 *)
+(* Define bijections                                                     *)
 (* --------------------------------------------------------------------- *)
+
 val fmap_ISO_DEF =
-    define_new_type_bijections {name  = "fmap_ISO_DEF",
-				ABS = "fmap_ABS",
-				REP = "fmap_REP",
-				tyax = fmap_TY_DEF};
+   define_new_type_bijections 
+       {name = "fmap_ISO_DEF",
+        ABS  = "fmap_ABS",
+        REP  = "fmap_REP",
+        tyax = fmap_TY_DEF};
 
 (* --------------------------------------------------------------------- *)
 (* Prove that REP is one-to-one.					 *)
 (* --------------------------------------------------------------------- *)
-val fmap_REP_11 = prove_rep_fn_one_one fmap_ISO_DEF;
 
-val fmap_REP_onto = prove_rep_fn_onto fmap_ISO_DEF;
-
-val fmap_ABS_11 = prove_abs_fn_one_one fmap_ISO_DEF;
-
+val fmap_REP_11   = prove_rep_fn_one_one fmap_ISO_DEF
+val fmap_REP_onto = prove_rep_fn_onto fmap_ISO_DEF
+val fmap_ABS_11   = prove_abs_fn_one_one fmap_ISO_DEF
 val fmap_ABS_onto = prove_abs_fn_onto fmap_ISO_DEF;
 
 val (fmap_ABS_REP_THM,fmap_REP_ABS_THM)  =
-   let
-       val thms = CONJUNCTS fmap_ISO_DEF;
-       val [t1,t2] = map (GEN_ALL o SYM o SPEC_ALL) thms
-   in
-       (t1,t2)
-   end;
+ let val thms = CONJUNCTS fmap_ISO_DEF
+     val [t1,t2] = map (GEN_ALL o SYM o SPEC_ALL) thms
+ in (t1,t2)
+  end;
 
 
-(*CANCELLATION THEOREMS*)
+(*---------------------------------------------------------------------------
+        CANCELLATION THEOREMS
+ ---------------------------------------------------------------------------*)
+
+val is_fmap_REP = Q.prove 
+(`!f:'a |-> 'b. is_fmap (fmap_REP f)`,
+ REWRITE_TAC [fmap_REP_onto] 
+  THEN GEN_TAC THEN Q.EXISTS_TAC `f` 
+  THEN REWRITE_TAC [fmap_REP_11]);
+
+val REP_ABS_empty = Q.prove 
+(`fmap_REP (fmap_ABS ((\a. INR one):'a -> 'b + one)) = \a. INR one`,
+ REWRITE_TAC [fmap_REP_ABS_THM] 
+  THEN REWRITE_TAC [is_fmap_empty]);
+
+val REP_ABS_update = Q.prove 
+(`!(f:'a |-> 'b) x y.
+     fmap_REP (fmap_ABS (\a. if a=x then INL y else fmap_REP f a))
+         =
+     \a. if a=x then INL y else fmap_REP f a`,
+ REPEAT GEN_TAC 
+   THEN REWRITE_TAC [fmap_REP_ABS_THM] 
+   THEN MATCH_MP_TAC is_fmap_update 
+   THEN REWRITE_TAC [is_fmap_REP]);
+
+val is_fmap_REP_ABS = Q.prove 
+(`!f:'a -> 'b + one. is_fmap f ==> (fmap_REP (fmap_ABS f) = f)`,
+ REPEAT STRIP_TAC 
+  THEN REWRITE_TAC [fmap_REP_ABS_THM]
+  THEN ASM_REWRITE_TAC []);
 
 
-val is_fmap_REP = prove (Term`!(f : ('a,'b) fmap). is_fmap (fmap_REP f)`,
-REWRITE_TAC [BETA_RULE  fmap_REP_onto] THEN
-GEN_TAC THEN
-EXISTS_TAC (Term`f: ('a,'b) fmap`) THEN
-REWRITE_TAC [fmap_REP_11]);
+(*---------------------------------------------------------------------------
+        DEFINITIONS OF UPDATE, EMPTY, APPLY and DOMAIN
+ ---------------------------------------------------------------------------*)
 
-val REP_ABS_empty = prove (
-Term`fmap_REP (fmap_ABS ((\a. INR one):'a -> 'b + one)) = (\a. INR one)`,
-REWRITE_TAC [fmap_REP_ABS_THM] THEN
-BETA_TAC THEN
-REWRITE_TAC [is_fmap_empty]);
+val FUPDATE_DEF = Q.new_definition 
+("FUPDATE_DEF",
+ `FUPDATE (f:'a |-> 'b) (x,y)
+    = fmap_ABS (\a. if a=x then INL y else fmap_REP f a)`);
 
+val FEMPTY_DEF = Q.new_definition 
+("FEMPTY_DEF",
+ `(FEMPTY:'a |-> 'b) = fmap_ABS (\a. INR one)`);
 
-val REP_ABS_update = prove (Term
- `!(f:('a,'b) fmap) x y.
-     fmap_REP (fmap_ABS (\a. (a = x) => INL y | fmap_REP f a))
-      =
-     (\a. (a = x) => INL y | fmap_REP f a)`,
-REPEAT GEN_TAC THEN
-REWRITE_TAC [fmap_REP_ABS_THM] THEN
-BETA_TAC THEN
-MATCH_MP_TAC  is_fmap_update THEN
-REWRITE_TAC [is_fmap_REP]);
+val FAPPLY_DEF = Q.new_definition 
+("FAPPLY_DEF",
+ `FAPPLY (f:'a |-> 'b) x = OUTL (fmap_REP f x)`);
 
-val is_fmap_REP_ABS = prove (Term
-`!(f:'a -> 'b + one). is_fmap f ==> (fmap_REP (fmap_ABS f) = f)`,
-REPEAT STRIP_TAC THEN
-REWRITE_TAC [fmap_REP_ABS_THM] THEN
-BETA_TAC THEN
-ASM_REWRITE_TAC []);
+val FDOM_DEF = Q.new_definition 
+("FDOM_DEF",
+ `FDOM (f:'a |-> 'b) x = ISL (fmap_REP f x)`);
 
+val update_rep = Term`\(f:'a->'b+one) x y. \a. if a=x then INL y else f a`;
 
-
-(*DEFINITIONS OF UPDATE, EMPTY, APPLY and DOMAIN*)
-
-val FUPDATE_DEF = new_definition ("FUPDATE_DEF",
-               Term`FUPDATE (f:('a,'b) fmap ) (x,y)
-                   = fmap_ABS (\a:'a. (a = x) => INL y | (fmap_REP f) a)`);
-
-val FEMPTY_DEF = new_definition ("FEMPTY_DEF",
-               Term`FEMPTY :('a,'b) fmap  =
-                   fmap_ABS (\a:'a. INR one)`);
-
-val FAPPLY_DEF = new_definition ("FAPPLY_DEF",
-               Term`FAPPLY (f:('a,'b) fmap ) (x:'a)
-                      =  OUTL ((fmap_REP f) x)`);
-
-val FDOM_DEF = new_definition ("FDOM_DEF",
-               Term`FDOM (f:('a,'b) fmap ) (x:'a)
-                      = ISL ((fmap_REP f) x)`);
-
-val update_rep =Term`\(f:'a -> 'b + one) x y.
-                           \a.
-                            (a = x) => INL y | f a`;
-
-val empty_rep =Term`(\a. INR one):'a -> 'b + one`;
+val empty_rep = Term`(\a. INR one):'a -> 'b + one`;
 
 
 
-(* Now some theorems *)
+(*---------------------------------------------------------------------------
+      Now some theorems
+ --------------------------------------------------------------------------- *)
 
-val FAPPLY_FUPDATE =
-store_thm ("FAPPLY_FUPDATE",
-Term`!(f:('a,'b) fmap) x y.
-         FAPPLY (FUPDATE f (x,y)) x = y`,
-REWRITE_TAC [FUPDATE_DEF, FAPPLY_DEF] THEN
-REPEAT GEN_TAC THEN
-REWRITE_TAC [REP_ABS_update] THEN
-BETA_TAC THEN
-REWRITE_TAC [sumTheory.OUTL]);
+val FAPPLY_FUPDATE = Q.store_thm ("FAPPLY_FUPDATE",
+`!(f:'a |-> 'b) x y. FAPPLY (FUPDATE f (x,y)) x = y`,
+ REWRITE_TAC [FUPDATE_DEF, FAPPLY_DEF] 
+   THEN REPEAT GEN_TAC 
+    THEN REWRITE_TAC [REP_ABS_update] THEN BETA_TAC
+    THEN REWRITE_TAC [sumTheory.OUTL]);
 
-val NOT_EQ_FAPPLY =
-store_thm ("NOT_EQ_FAPPLY",
-Term`!(f:('a,'b) fmap) a x y . ~(a = x) ==> (FAPPLY (FUPDATE f (x,y)) a = FAPPLY f a)`,
-REPEAT STRIP_TAC THEN
-REWRITE_TAC [FUPDATE_DEF, FAPPLY_DEF, REP_ABS_update] THEN
-BETA_TAC THEN
-ASM_REWRITE_TAC []);
+val NOT_EQ_FAPPLY = Q.store_thm ("NOT_EQ_FAPPLY",
+`!(f:'a|-> 'b) a x y . ~(a=x) ==> (FAPPLY (FUPDATE f (x,y)) a = FAPPLY f a)`, 
+REPEAT STRIP_TAC 
+  THEN REWRITE_TAC [FUPDATE_DEF, FAPPLY_DEF, REP_ABS_update] THEN BETA_TAC
+  THEN ASM_REWRITE_TAC []);
 
-val update_commutes_rep = (BETA_RULE o BETA_RULE) (prove (
-Term`!(f:'a -> 'b + one) a b c d.
-   ~(a = c) ==> (^update_rep (^update_rep f a b) c d =
-                    ^update_rep (^update_rep f c d) a b)`,
-REPEAT STRIP_TAC THEN
-BETA_TAC THEN
-MATCH_MP_TAC EQ_EXT THEN
-GEN_TAC THEN
-ASM_CASES_TAC (Term`(x:'a) = a`) THEN BETA_TAC THEN
-ASM_REWRITE_TAC []));
+val update_commutes_rep = (BETA_RULE o BETA_RULE) (Q.prove 
+(`!(f:'a -> 'b + one) a b c d.
+     ~(a = c) 
+        ==> 
+ (^update_rep (^update_rep f a b) c d = ^update_rep (^update_rep f c d) a b)`,
+REPEAT STRIP_TAC THEN BETA_TAC 
+  THEN MATCH_MP_TAC EQ_EXT 
+  THEN GEN_TAC 
+  THEN Q.ASM_CASES_TAC `x = a` THEN BETA_TAC 
+  THEN ASM_REWRITE_TAC []));
 
 
-val FUPDATE_COMMUTES = store_thm ("FUPDATE_COMMUTES",
-Term`!(f:('a,'b) fmap) a b c d.
-   ~(a = c) ==> (FUPDATE (FUPDATE f (a,b)) (c,d) =
-                    FUPDATE (FUPDATE f (c,d)) (a,b))`,
-REPEAT STRIP_TAC THEN
-REWRITE_TAC [FUPDATE_DEF, REP_ABS_update] THEN
-BETA_TAC THEN
-AP_TERM_TAC THEN
-MATCH_MP_TAC EQ_EXT THEN
-GEN_TAC THEN
-ASM_CASES_TAC (Term`(x:'a) = a`) THEN BETA_TAC THEN
-ASM_REWRITE_TAC []);
+val FUPDATE_COMMUTES = Q.store_thm ("FUPDATE_COMMUTES",
+`!(f:'a |-> 'b) a b c d.
+   ~(a = c) 
+     ==> 
+  (FUPDATE (FUPDATE f (a,b)) (c,d) = FUPDATE (FUPDATE f (c,d)) (a,b))`,
+REPEAT STRIP_TAC 
+  THEN REWRITE_TAC [FUPDATE_DEF, REP_ABS_update] THEN BETA_TAC 
+  THEN AP_TERM_TAC 
+  THEN MATCH_MP_TAC EQ_EXT 
+  THEN GEN_TAC 
+  THEN Q.ASM_CASES_TAC `x = a` THEN BETA_TAC 
+  THEN ASM_REWRITE_TAC []);
 
-val update_same_rep = (BETA_RULE o BETA_RULE) (prove (
-Term`!(f:'a -> 'b+one) a b c.
-    ^update_rep (^update_rep f a b) a c = ^update_rep f a c`,
-BETA_TAC THEN
-REPEAT GEN_TAC THEN
-MATCH_MP_TAC EQ_EXT THEN
-GEN_TAC THEN
-ASM_CASES_TAC (Term`(x:'a) = a`) THEN BETA_TAC THEN
-ASM_REWRITE_TAC []));
+val update_same_rep = (BETA_RULE o BETA_RULE) (Q.prove 
+(`!(f:'a -> 'b+one) a b c.
+   ^update_rep (^update_rep f a b) a c = ^update_rep f a c`,
+BETA_TAC THEN REPEAT GEN_TAC 
+  THEN MATCH_MP_TAC EQ_EXT 
+  THEN GEN_TAC 
+  THEN Q.ASM_CASES_TAC `x = a` THEN BETA_TAC 
+  THEN ASM_REWRITE_TAC []));
 
-val FUPDATE_EQ =store_thm ("FUPDATE_EQ",
-Term`!(f:('a,'b) fmap) a b c.
-     FUPDATE (FUPDATE f (a,b)) (a,c) =
-                    FUPDATE f (a,c)`,
-REPEAT STRIP_TAC THEN
-REWRITE_TAC [FUPDATE_DEF, REP_ABS_update] THEN
-BETA_TAC THEN
-AP_TERM_TAC THEN
-MATCH_MP_TAC EQ_EXT THEN
-GEN_TAC THEN
-ASM_CASES_TAC (Term`(x:'a) = a`) THEN BETA_TAC THEN
-ASM_REWRITE_TAC []);
+val FUPDATE_EQ = Q.store_thm ("FUPDATE_EQ",
+`!(f:'a |-> 'b) a b c. FUPDATE (FUPDATE f (a,b)) (a,c) = FUPDATE f (a,c)`,
+REPEAT STRIP_TAC 
+  THEN REWRITE_TAC [FUPDATE_DEF, REP_ABS_update] THEN BETA_TAC 
+  THEN AP_TERM_TAC 
+  THEN MATCH_MP_TAC EQ_EXT 
+  THEN GEN_TAC 
+  THEN Q.ASM_CASES_TAC `x = a` THEN BETA_TAC 
+  THEN ASM_REWRITE_TAC []);
 
-val lemma1 = prove (
-Term`~((ISL :'b + one -> bool) ((INR :one -> 'b + one) (one :one)))`,
-REWRITE_TAC [sumTheory.ISL]);
+val lemma1 = Q.prove
+(`~((ISL :'b + one -> bool) ((INR :one -> 'b + one) one))`,
+ REWRITE_TAC [sumTheory.ISL]);
 
-val FDOM_FEMPTY =
-store_thm ("FDOM_FEMPTY",
-Term`!a. FDOM (FEMPTY:('a,'b) fmap) a = F`,
-GEN_TAC THEN
-REWRITE_TAC [FDOM_DEF, FEMPTY_DEF, REP_ABS_empty,
-             sumTheory.ISL]);
+val FDOM_FEMPTY = Q.store_thm ("FDOM_FEMPTY",
+`!a. FDOM (FEMPTY:'a |-> 'b) a = F`,
+GEN_TAC THEN REWRITE_TAC [FDOM_DEF, FEMPTY_DEF, REP_ABS_empty, sumTheory.ISL]);
 
-val dom_update_rep = BETA_RULE (prove(
-Term`!f a b x. ISL (^update_rep (f:'a -> 'b+one ) a b x) = ((x = a)
-    \/  ISL (f x))`,
-REPEAT GEN_TAC THEN
-BETA_TAC THEN
-ASM_CASES_TAC (Term`(x:'a) = a`) THEN
-ASM_REWRITE_TAC [sumTheory.ISL]));
+val dom_update_rep = BETA_RULE (Q.prove
+(`!f a b x. ISL(^update_rep (f:'a -> 'b+one ) a b x) = ((x=a) \/ ISL (f x))`,
+REPEAT GEN_TAC THEN BETA_TAC 
+  THEN Q.ASM_CASES_TAC `x = a` 
+  THEN ASM_REWRITE_TAC [sumTheory.ISL]));
 
+val FDOM_FUPDATE = Q.store_thm("FDOM_FUPDATE",
+`!f a b x. FDOM (FUPDATE (f:'a |-> 'b) (a,b)) x = (x=a) \/ FDOM f x`,
+REPEAT GEN_TAC 
+  THEN REWRITE_TAC [FDOM_DEF,FUPDATE_DEF, REP_ABS_update] THEN BETA_TAC 
+  THEN Q.ASM_CASES_TAC `x = a` 
+  THEN ASM_REWRITE_TAC [sumTheory.ISL]);
 
-val FDOM_FUPDATE =
-store_thm("FDOM_FUPDATE",
-Term`!f a b x. FDOM (FUPDATE (f:('a,'b) fmap ) (a,b)) x = ((x = a)
-    \/  FDOM f x)`,
-REPEAT GEN_TAC THEN
-REWRITE_TAC [FDOM_DEF,FUPDATE_DEF, REP_ABS_update] THEN
-BETA_TAC THEN
-ASM_CASES_TAC (Term`(x:'a) = a`) THEN
-ASM_REWRITE_TAC [sumTheory.ISL]);
+val FAPPLY_FUPDATE_THM = Q.store_thm("FAPPLY_FUPDATE_THM",
+`!(f:'a |-> 'b) a b x.
+   FAPPLY(FUPDATE f (a,b)) x = if x=a then b else FAPPLY f x`,
+REPEAT STRIP_TAC 
+  THEN COND_CASES_TAC 
+  THEN ASM_REWRITE_TAC [FAPPLY_FUPDATE] 
+  THEN IMP_RES_TAC NOT_EQ_FAPPLY 
+  THEN ASM_REWRITE_TAC []);
 
-val FAPPLY_FUPDATE_THM = store_thm("FAPPLY_FUPDATE_THM",
-Term`!(f:('a,'b) fmap)  a b x.FAPPLY(FUPDATE f (a,b)) x = ((x=a) => b | FAPPLY f x)`,
-REPEAT STRIP_TAC THEN
-COND_CASES_TAC THEN
-ASM_REWRITE_TAC [FAPPLY_FUPDATE] THEN
-IMP_RES_TAC NOT_EQ_FAPPLY THEN
-ASM_REWRITE_TAC []);
+val not_eq_empty_update_rep = BETA_RULE (Q.prove 
+(`!(f:'a -> 'b + one) a b. ~(^empty_rep = ^update_rep f a b)`,
+REPEAT GEN_TAC THEN BETA_TAC 
+  THEN CONV_TAC (DEPTH_CONV FUN_EQ_CONV) 
+  THEN CONV_TAC NOT_FORALL_CONV 
+  THEN Q.EXISTS_TAC `a` THEN BETA_TAC
+  THEN DISCH_THEN (fn th => REWRITE_TAC [REWRITE_RULE [sumTheory.ISL]
+                               (REWRITE_RULE [th] lemma1)])));
 
-
-val not_eq_empty_update_rep = BETA_RULE (prove (
-Term`!(f:'a -> 'b + one) a b.
-   ~(^empty_rep = ^update_rep f a b)`,
-REPEAT GEN_TAC THEN
-BETA_TAC THEN
-CONV_TAC (DEPTH_CONV FUN_EQ_CONV) THEN
-CONV_TAC  NOT_FORALL_CONV THEN
-EXISTS_TAC (Term`a:'a`) THEN
-BETA_TAC THEN
-DISCH_THEN (fn th => REWRITE_TAC
-       [REWRITE_RULE [sumTheory.ISL]
-               (REWRITE_RULE [th] lemma1)])));
-
-
-val fmap_EQ_1 = prove (
-Term`!(f:('a,'b) fmap) g.
-    (f = g) ==> (FDOM f = FDOM g) /\ (FAPPLY f = FAPPLY g)`,
+val fmap_EQ_1 = Q.prove 
+(`!(f:'a |-> 'b) g. (f=g) ==> (FDOM f = FDOM g) /\ (FAPPLY f = FAPPLY g)`,
 REPEAT STRIP_TAC THEN ASM_REWRITE_TAC []);
 
-val NOT_EQ_FEMPTY_FUPDATE =
-store_thm ("NOT_EQ_FEMPTY_FUPDATE",
-Term`!(f:('a,'b) fmap) a b.
-   ~(FEMPTY = FUPDATE f (a,b))`,
-REPEAT STRIP_TAC THEN
-IMP_RES_TAC fmap_EQ_1 THEN
-UNDISCH_TAC (Term`FDOM (FEMPTY:('a,'b)fmap) =
-          FDOM (FUPDATE (f:('a,'b)fmap) (a,b))`) THEN
-CONV_TAC (DEPTH_CONV FUN_EQ_CONV) THEN
-REWRITE_TAC [] THEN
-CONV_TAC  NOT_FORALL_CONV THEN
-EXISTS_TAC (Term`a:'a`) THEN
-REWRITE_TAC [FDOM_FEMPTY, FDOM_FUPDATE]);
+val NOT_EQ_FEMPTY_FUPDATE = Q.store_thm ("NOT_EQ_FEMPTY_FUPDATE",
+`!(f:'a |-> 'b) a b. ~(FEMPTY = FUPDATE f (a,b))`,
+REPEAT STRIP_TAC 
+  THEN IMP_RES_TAC fmap_EQ_1 
+  THEN UNDISCH_TAC (Term`FDOM (FEMPTY:('a,'b)fmap) =
+          FDOM (FUPDATE (f:('a,'b)fmap) (a,b))`) 
+  THEN CONV_TAC (DEPTH_CONV FUN_EQ_CONV) 
+  THEN REWRITE_TAC [] 
+  THEN CONV_TAC NOT_FORALL_CONV 
+  THEN Q.EXISTS_TAC `a` 
+  THEN REWRITE_TAC [FDOM_FEMPTY, FDOM_FUPDATE]);
 
-val FDOM_EQ_FDOM_FUPDATE = store_thm("FDOM_EQ_FDOM_FUPDATE",
-Term`!(f:('a,'b) fmap) x. FDOM f x ==> (!y. FDOM (FUPDATE f (x,y)) = FDOM f)`,
-REPEAT STRIP_TAC THEN
-CONV_TAC (DEPTH_CONV FUN_EQ_CONV) THEN
-GEN_TAC THEN ASM_CASES_TAC (Term`(x':'a)=x`) THEN
-ASM_REWRITE_TAC [FDOM_FUPDATE]);
+val FDOM_EQ_FDOM_FUPDATE = Q.store_thm("FDOM_EQ_FDOM_FUPDATE",
+`!(f:'a |-> 'b) x. FDOM f x ==> (!y. FDOM (FUPDATE f (x,y)) = FDOM f)`,
+REPEAT STRIP_TAC 
+  THEN CONV_TAC (DEPTH_CONV FUN_EQ_CONV) 
+  THEN GEN_TAC THEN ASM_CASES_TAC (Term`(x':'a)=x`) 
+  THEN ASM_REWRITE_TAC [FDOM_FUPDATE]);
 
-
-(*A small lemma*)
-val lemma2 = prove (
-Term`!x y z. (x ==> (y /\ z)) ==> (x ==> y)`,
-REPEAT STRIP_TAC THEN RES_TAC);
+val lemma2 = Q.prove 
+(`!x y z. (x ==> (y /\ z)) ==> (x ==> y)`, REPEAT STRIP_TAC THEN RES_TAC);
 
 
-(*SIMPLE INDUCTION*)
+(*---------------------------------------------------------------------------
+       Simple induction
+ ---------------------------------------------------------------------------*)
 
-val fmap_SIMPLE_INDUCT = store_thm ("fmap_SIMPLE_INDUCT",
-Term`!P. P FEMPTY /\
-       (!f. P f ==> (!x y.  P(FUPDATE f (x,y)))) ==>
-       !f:('a,'b) fmap. P f`,
-REWRITE_TAC [FUPDATE_DEF, FEMPTY_DEF] THEN
-GEN_TAC THEN STRIP_TAC THEN
-GEN_TAC THEN
-CHOOSE_TAC (SPEC (Term`f:('a,'b)fmap`) fmap_ABS_onto) THEN
-ASM_REWRITE_TAC [] THEN
-ASSUM_LIST (fn ths => ASSUME_TAC (CONJUNCT2 (BETA_RULE (el 1 ths)))) THEN
-UNDISCH_TAC  (Term`is_fmap (r:'a -> 'b + one)`) THEN
-SPEC_TAC (Term`r:'a -> 'b + one`,Term`r:'a -> 'b + one`) THEN
-ind_defLib.RULE_INDUCT_THEN strong_is_fmap_ind ASSUME_TAC ASSUME_TAC THENL
-[
- ASM_REWRITE_TAC[],
- IMP_RES_TAC is_fmap_REP_ABS THEN
- RES_TAC THEN
- ASSUM_LIST (fn ths => REWRITE_TAC [REWRITE_RULE [el 3 ths] (el 2 ths)])
-]
-);
+val fmap_SIMPLE_INDUCT = Q.store_thm ("fmap_SIMPLE_INDUCT",
+`!P:('a |-> 'b) -> bool. 
+     P FEMPTY /\ 
+     (!f. P f ==> !x y. P (FUPDATE f (x,y)))
+     ==> 
+     !f. P f`,
+REWRITE_TAC [FUPDATE_DEF, FEMPTY_DEF] 
+  THEN GEN_TAC THEN STRIP_TAC THEN GEN_TAC 
+  THEN CHOOSE_THEN(CONJUNCTS_THEN2 SUBST1_TAC MP_TAC) (Q.SPEC`f` fmap_ABS_onto)
+  THEN Q.ID_SPEC_TAC `r`
+  THEN HO_MATCH_MP_TAC strong_ind 
+  THEN ASM_REWRITE_TAC []
+  THEN Q.PAT_ASSUM `P x` (K ALL_TAC)
+  THEN REPEAT STRIP_TAC THEN RES_TAC
+  THEN IMP_RES_THEN SUBST_ALL_TAC is_fmap_REP_ABS
+  THEN ASM_REWRITE_TAC[]);
 
-val FUPDATE_ABSORB_THM = prove (
-Term`!(f:('a,'b) fmap) x y. (FDOM f x)  /\ (FAPPLY f x = y) ==> (FUPDATE f (x,y) = f)`,
+val FUPDATE_ABSORB_THM = Q.prove 
+(`!(f:'a |-> 'b) x y. 
+     FDOM f x /\ (FAPPLY f x = y) ==> (FUPDATE f (x,y) = f)`,
+ INDUCT_THEN fmap_SIMPLE_INDUCT STRIP_ASSUME_TAC 
+   THEN REWRITE_TAC [FDOM_FEMPTY] 
+   THEN REPEAT STRIP_TAC 
+   THEN Q.ASM_CASES_TAC `x = x'` THENL
+   [ASM_REWRITE_TAC [FUPDATE_EQ] 
+      THEN Q.ASM_CASES_TAC `y = y'` 
+      THEN ASM_REWRITE_TAC [] 
+      THEN ASSUM_LIST (fn ths => ASSUME_TAC (
+           REWRITE_RULE [el 2 ths, FAPPLY_FUPDATE, el 1 ths] (el 3 ths))) 
+      THEN MATCH_MP_TAC FALSITY THEN ASM_REWRITE_TAC[],
+    IMP_RES_TAC FUPDATE_COMMUTES 
+      THEN ASM_REWRITE_TAC []
+      THEN ASSUM_LIST (fn ths => ASSUME_TAC 
+            (REWRITE_RULE [MATCH_MP NOT_EQ_FAPPLY (NOT_EQ_SYM (el 2 ths))]
+                  (el 3 ths))) 
+      THEN ASSUM_LIST (fn ths => ASSUME_TAC 
+            (REWRITE_RULE [FDOM_FUPDATE, (NOT_EQ_SYM (el 3 ths))] (el 5 ths)))
+      THEN RES_TAC 
+      THEN ASM_REWRITE_TAC []]);
 
-INDUCT_THEN  fmap_SIMPLE_INDUCT STRIP_ASSUME_TAC THEN
-REWRITE_TAC [FDOM_FEMPTY] THEN
-REPEAT STRIP_TAC THEN
-ASM_CASES_TAC (Term`(x:'a) = x'`) THENL
-[  ASM_REWRITE_TAC [FUPDATE_EQ] THEN
-   ASM_CASES_TAC (Term`(y:'b) = y'`) THEN
-   ASM_REWRITE_TAC [] THEN
-   ASSUM_LIST
-   (fn ths => ASSUME_TAC (
-     REWRITE_RULE [el 2 ths, FAPPLY_FUPDATE, el 1 ths] (el 3 ths))) THEN
-   UNDISCH_TAC (Term`F`) THEN
-   REWRITE_TAC [],
-   IMP_RES_TAC FUPDATE_COMMUTES THEN
-   ASM_REWRITE_TAC [] THEN
-   ASSUM_LIST (fn ths => ASSUME_TAC (
-     REWRITE_RULE [
-       MATCH_MP NOT_EQ_FAPPLY (NOT_EQ_SYM (el 2 ths))]
-        (el 3 ths))) THEN
-   ASSUM_LIST (fn ths => ASSUME_TAC (
-     REWRITE_RULE [FDOM_FUPDATE, (NOT_EQ_SYM (el 3 ths))]
-        (el 5 ths))) THEN
-   RES_TAC THEN
-   ASM_REWRITE_TAC []
-]
-);
+val FDOM_FAPPLY = Q.prove
+(`!(f:'a |-> 'b) x. FDOM f x ==> ?y. FAPPLY f x = y`,
+ INDUCT_THEN fmap_SIMPLE_INDUCT ASSUME_TAC THENL
+ [REWRITE_TAC [FDOM_FEMPTY],
+  REWRITE_TAC [FDOM_FUPDATE] 
+    THEN REPEAT GEN_TAC 
+    THEN Q.ASM_CASES_TAC `x' = x` 
+    THEN ASM_REWRITE_TAC [] THENL
+    [Q.EXISTS_TAC `y` THEN REWRITE_TAC [FAPPLY_FUPDATE],
+     IMP_RES_TAC NOT_EQ_FAPPLY 
+       THEN DISCH_TAC THEN RES_TAC 
+       THEN Q.EXISTS_TAC `y'` 
+       THEN ASM_REWRITE_TAC []]]);
 
-val FDOM_FAPPLY = prove(
-Term`!(f:('a,'b) fmap) x. FDOM f x ==> ?y. FAPPLY f x = y`,
-INDUCT_THEN fmap_SIMPLE_INDUCT ASSUME_TAC THENL
-[REWRITE_TAC [FDOM_FEMPTY],
- REWRITE_TAC [FDOM_FUPDATE] THEN
- REPEAT GEN_TAC THEN
- ASM_CASES_TAC (Term`(x':'a)=x`) THEN
- ASM_REWRITE_TAC [] THENL
- [
-  EXISTS_TAC (Term`y:'b`) THEN
-  REWRITE_TAC [FAPPLY_FUPDATE],
-  IMP_RES_TAC NOT_EQ_FAPPLY THEN
-  DISCH_TAC THEN RES_TAC THEN
-  EXISTS_TAC (Term`y':'b`) THEN
-  ASM_REWRITE_TAC []
- ]
-]);
+val FDOM_FUPDATE_ABSORB = Q.prove 
+(`!(f:'a |-> 'b) x. FDOM f x ==> ?y. FUPDATE f (x,y) = f`,
+ REPEAT STRIP_TAC 
+   THEN IMP_RES_TAC FDOM_FAPPLY 
+   THEN Q.EXISTS_TAC `y`
+   THEN MATCH_MP_TAC FUPDATE_ABSORB_THM 
+   THEN ASM_REWRITE_TAC []);
 
-val FDOM_FUPDATE_ABSORB = prove (
-Term`!(f:('a,'b) fmap) x. (FDOM f x)  ==> (?y. FUPDATE f (x,y) = f)`,
-REPEAT STRIP_TAC THEN
-IMP_RES_TAC FDOM_FAPPLY THEN
-EXISTS_TAC (Term`y:'b`) THEN
-MATCH_MP_TAC FUPDATE_ABSORB_THM THEN
-ASM_REWRITE_TAC []
-);
+val FDOM_F_FEMPTY = Q.store_thm 
+("FDOM_F_FEMPTY1",
+ `!f:'a |-> 'b. (!a. ~FDOM f a) = (f = FEMPTY)`,
+ INDUCT_THEN fmap_SIMPLE_INDUCT ASSUME_TAC THENL
+ [REWRITE_TAC [FDOM_FEMPTY],
+  GEN_TAC THEN GEN_TAC
+    THEN REWRITE_TAC [NOT_EQ_SYM(Q.SPECL[`f`,`x`,`y`] NOT_EQ_FEMPTY_FUPDATE)] 
+    THEN CONV_TAC NOT_FORALL_CONV 
+    THEN Q.EXISTS_TAC `x`
+    THEN REWRITE_TAC [FDOM_FUPDATE]]);
 
-val FDOM_F_FEMPTY =
-store_thm ("FDOM_F_FEMPTY1",
-Term`!f. (!a. ~(FDOM (f:('a,'b) fmap) a)) = (f = FEMPTY)`,
-INDUCT_THEN fmap_SIMPLE_INDUCT ASSUME_TAC THENL
-[REWRITE_TAC [FDOM_FEMPTY],
- GEN_TAC THEN GEN_TAC THEN
- REWRITE_TAC [NOT_EQ_SYM (SPECL [Term`f:('a,'b)fmap`,Term`x:'a`,Term`y:'b`] NOT_EQ_FEMPTY_FUPDATE)] THEN
- CONV_TAC NOT_FORALL_CONV THEN
- EXISTS_TAC (Term`x:'a`) THEN
- REWRITE_TAC [FDOM_FUPDATE]
-]);
 
 (* ===================================================================== *)
 (* Cardinality                                                           *)
+(*                                                                       *)
+(* Define cardinality by copying the proofs in the sets library. To      *)
+(* simplify this we define cardinality as a function over the domain     *)
+(* FDOM f of the finite map. We need to define deletion from the domain. *)
 (* ===================================================================== *)
-(*
-Define cardinality by copying the prrofs in the sets library. To simplfy
-this we define cardinality as a function over the domain FDOM f
-of the finite map. We need to define deletion from the domain. *)
 
-val FDOMDEL_DEF = new_definition ("FDOMDEL_DEF",
-Term`FDOMDEL (d:'a->bool) x a = d a /\ (~(a = x))`);
+val FDOMDEL_DEF = Q.new_definition 
+("FDOMDEL_DEF",
+ `FDOMDEL (d:'a->bool) x a = d a /\ (~(a = x))`);
 
 
-val FDOMDEL_COMM = prove (
-Term`!(s:'a->bool) x y. FDOMDEL (FDOMDEL s x) y = FDOMDEL (FDOMDEL s y) x`,
-CONV_TAC (DEPTH_CONV FUN_EQ_CONV) THEN
-REWRITE_TAC [FDOMDEL_DEF] THEN
-REPEAT STRIP_TAC THEN EQ_TAC THEN STRIP_TAC THEN ASM_REWRITE_TAC []);
+val FDOMDEL_COMM = Q.prove 
+(`!(s:'a->bool) x y. FDOMDEL (FDOMDEL s x) y = FDOMDEL (FDOMDEL s y) x`,
+CONV_TAC (DEPTH_CONV FUN_EQ_CONV) 
+  THEN REWRITE_TAC [FDOMDEL_DEF] 
+  THEN REPEAT STRIP_TAC 
+  THEN EQ_TAC 
+  THEN STRIP_TAC 
+  THEN ASM_REWRITE_TAC []);
 
-val FDOM_FDOM_DEL = prove (
-Term`!(f:('a,'b)fmap) x.
-     ~(FDOM f x) ==> (!y. (FDOMDEL (FDOM (FUPDATE f (x,y))) x) = FDOM f)`,
-CONV_TAC (DEPTH_CONV FUN_EQ_CONV) THEN
-REWRITE_TAC [FDOMDEL_DEF, FDOM_FUPDATE] THEN
-REPEAT STRIP_TAC THEN
-ASM_CASES_TAC (Term`(x':'a)=x`) THEN
-ASM_REWRITE_TAC []);
+val FDOM_FDOM_DEL = Q.prove 
+(`!(f:'a |-> 'b) x.
+     ~FDOM f x ==> !y. (FDOMDEL (FDOM (FUPDATE f (x,y))) x) = FDOM f`,
+ CONV_TAC (DEPTH_CONV FUN_EQ_CONV) 
+  THEN REWRITE_TAC [FDOMDEL_DEF, FDOM_FUPDATE] 
+  THEN REPEAT STRIP_TAC 
+  THEN Q.ASM_CASES_TAC `x' = x` 
+  THEN ASM_REWRITE_TAC []);
 
-val FDOMDEL_FEMPTY = prove(
-Term`!x. FDOMDEL (FDOM (FEMPTY:('a,'b)fmap)) x = (FDOM (FEMPTY:('a,'b)fmap))`,
-CONV_TAC (DEPTH_CONV FUN_EQ_CONV) THEN
-REWRITE_TAC [FDOMDEL_DEF, FDOM_FEMPTY]);
+val FDOMDEL_FEMPTY = Q.prove
+(`!x. FDOMDEL (FDOM (FEMPTY:'a |-> 'b)) x = FDOM (FEMPTY:'a |-> 'b)`,
+CONV_TAC (DEPTH_CONV FUN_EQ_CONV) 
+ THEN REWRITE_TAC [FDOMDEL_DEF, FDOM_FEMPTY]);
 
 (* --------------------------------------------------------------------- *)
 (* card_rel_def: defining equations for a relation `R s n`, which means  *)
@@ -467,90 +425,89 @@ Term`(!s. R s 0 = (s = (FDOM (FEMPTY:('a,'b)fmap)))) /\
 (* Prove that such a relation exists.                                    *)
 (* --------------------------------------------------------------------- *)
 
+val CARD_REL_EXISTS = prove_rec_fn_exists num_Axiom card_rel_def ;
 
-val CARD_REL_EXISTS =
-    prove_rec_fn_exists (prim_recTheory.num_Axiom) card_rel_def ;
-
-
-val CARD_REL_DEL_LEMMA = TAC_PROOF((strip_conj card_rel_def,
+val CARD_REL_DEL_LEMMA = TAC_PROOF
+((strip_conj card_rel_def,
 Term`!(n:num) (s:'a -> bool) (x:'a).
-    s x ==>
-    R (FDOMDEL s x) n  ==>
-    (!y:'a. s y ==> R (FDOMDEL s y) n)`),
-   Num_induct.INDUCT_TAC THENL
-   [REPEAT GEN_TAC THEN DISCH_TAC THEN
-    ASM_REWRITE_TAC [] THEN
-    CONV_TAC (DEPTH_CONV FUN_EQ_CONV) THEN
-    ASM_REWRITE_TAC [FDOMDEL_DEF, FDOM_FEMPTY] THEN
-    STRIP_TAC THEN GEN_TAC THEN
-    FIRST_ASSUM (STRIP_ASSUME_TAC o
-        REWRITE_RULE [DE_MORGAN_THM] o (SPEC (Term`y:'a`))) THEN
-    ASM_REWRITE_TAC [],
-    ASM_REWRITE_TAC [] THEN REPEAT STRIP_TAC THEN
-    let val th = (SPEC (Term`y:'a = x'`) EXCLUDED_MIDDLE)
-    in
-    DISJ_CASES_THEN2 SUBST_ALL_TAC ASSUME_TAC th
-    end THENL
-    [
-     CONV_TAC (DEPTH_CONV FUN_EQ_CONV) THEN
-     PURE_ONCE_REWRITE_TAC [FDOMDEL_COMM] THEN
-     EXISTS_TAC (Term`x:'a`) THEN ASM_REWRITE_TAC[] THEN
-     UNDISCH_TAC (Term`FDOMDEL (s:'a->bool)  x x'`) THEN
-     ASM_REWRITE_TAC [FDOMDEL_DEF] THEN
-     DISCH_THEN(fn th => REWRITE_TAC [NOT_EQ_SYM th]),
-
-     let val th = (SPEC (Term`x:'a = y`) EXCLUDED_MIDDLE)
-     in
-     DISJ_CASES_THEN2 SUBST_ALL_TAC ASSUME_TAC th
-     end THENL
-     [EXISTS_TAC (Term`x':'a`) THEN ASM_REWRITE_TAC [],
-      EXISTS_TAC (Term`x:'a`) THEN ASM_REWRITE_TAC [FDOMDEL_DEF] THEN
-      RES_THEN (TRY o IMP_RES_THEN ASSUME_TAC) THEN
-      PURE_ONCE_REWRITE_TAC [FDOMDEL_COMM] THEN
-      FIRST_ASSUM MATCH_MP_TAC THEN ASM_REWRITE_TAC [FDOMDEL_DEF] THEN
-      CONV_TAC (ONCE_DEPTH_CONV SYM_CONV) THEN FIRST_ASSUM ACCEPT_TAC]]]);
-
-
+      s x ==> R (FDOMDEL s x) n
+       ==>
+      !y:'a. s y ==> R (FDOMDEL s y) n`),
+ INDUCT_TAC THENL
+ [REPEAT GEN_TAC THEN DISCH_TAC 
+    THEN ASM_REWRITE_TAC [] 
+    THEN CONV_TAC (DEPTH_CONV FUN_EQ_CONV) 
+    THEN ASM_REWRITE_TAC [FDOMDEL_DEF, FDOM_FEMPTY] 
+    THEN STRIP_TAC THEN GEN_TAC 
+    THEN FIRST_ASSUM (STRIP_ASSUME_TAC o
+           REWRITE_RULE [DE_MORGAN_THM] o (SPEC (Term`y:'a`))) 
+    THEN ASM_REWRITE_TAC [],
+  ASM_REWRITE_TAC [] THEN REPEAT STRIP_TAC 
+    THEN let val th = Q.SPEC `y:'a = x'` EXCLUDED_MIDDLE
+         in DISJ_CASES_THEN2 SUBST_ALL_TAC ASSUME_TAC th end THENL
+    [CONV_TAC (DEPTH_CONV FUN_EQ_CONV) 
+       THEN PURE_ONCE_REWRITE_TAC [FDOMDEL_COMM] 
+       THEN Q.EXISTS_TAC `x` 
+       THEN ASM_REWRITE_TAC[] 
+       THEN Q.UNDISCH_TAC `FDOMDEL (s:'a->bool) x x'` 
+       THEN ASM_REWRITE_TAC [FDOMDEL_DEF] 
+       THEN DISCH_THEN(fn th => REWRITE_TAC [NOT_EQ_SYM th]),
+     let val th = Q.SPEC `x = y` EXCLUDED_MIDDLE
+     in DISJ_CASES_THEN2 SUBST_ALL_TAC ASSUME_TAC th end THENL
+     [Q.EXISTS_TAC `x'` THEN ASM_REWRITE_TAC [],
+      Q.EXISTS_TAC `x` 
+        THEN ASM_REWRITE_TAC [FDOMDEL_DEF] 
+        THEN RES_THEN (TRY o IMP_RES_THEN ASSUME_TAC) 
+        THEN PURE_ONCE_REWRITE_TAC [FDOMDEL_COMM] 
+        THEN FIRST_ASSUM MATCH_MP_TAC THEN ASM_REWRITE_TAC [FDOMDEL_DEF] 
+        THEN CONV_TAC (ONCE_DEPTH_CONV SYM_CONV) 
+        THEN FIRST_ASSUM ACCEPT_TAC]]]);
 
 (* --------------------------------------------------------------------- *)
 (* So `R s` specifies a unique number.                                   *)
 (* --------------------------------------------------------------------- *)
 
-val CARD_REL_UNIQUE = TAC_PROOF((strip_conj card_rel_def,
-Term`!n:num. !s:'a->bool. R s n ==> (!m. R s m ==> (n = m))`),
-   Num_induct.INDUCT_TAC THEN ASM_REWRITE_TAC [] THENL
-   [GEN_TAC THEN STRIP_TAC THEN Num_induct.INDUCT_TAC THEN
-    CONV_TAC (ONCE_DEPTH_CONV SYM_CONV) THENL
-    [STRIP_TAC THEN REFL_TAC,
-     ASM_REWRITE_TAC[numTheory.NOT_SUC,FDOM_FEMPTY]],
-    GEN_TAC THEN STRIP_TAC THEN Num_induct.INDUCT_TAC THENL
-    [ASM_REWRITE_TAC [numTheory.NOT_SUC] THEN
-      CONV_TAC (ONCE_DEPTH_CONV FUN_EQ_CONV) THEN
-      CONV_TAC NOT_FORALL_CONV THEN
-      EXISTS_TAC (Term`x:'a`) THEN
-      ASM_REWRITE_TAC [FDOM_FEMPTY],
-      ASM_REWRITE_TAC [prim_recTheory.INV_SUC_EQ] THEN STRIP_TAC THEN
-      IMP_RES_TAC CARD_REL_DEL_LEMMA THEN RES_TAC]]);
+val CARD_REL_UNIQUE = TAC_PROOF
+((strip_conj card_rel_def,
+ Term`!n:num. !s:'a->bool. R s n ==> !m. R s m ==> (n = m)`),
+ INDUCT_TAC THEN ASM_REWRITE_TAC [] THENL
+   [GEN_TAC THEN STRIP_TAC 
+       THEN INDUCT_TAC
+       THEN CONV_TAC (ONCE_DEPTH_CONV SYM_CONV) THENL
+       [STRIP_TAC THEN REFL_TAC,
+        ASM_REWRITE_TAC[NOT_SUC,FDOM_FEMPTY]],
+    GEN_TAC THEN STRIP_TAC THEN INDUCT_TAC THENL
+    [ASM_REWRITE_TAC [NOT_SUC] 
+       THEN CONV_TAC (ONCE_DEPTH_CONV FUN_EQ_CONV) 
+       THEN CONV_TAC NOT_FORALL_CONV 
+       THEN Q.EXISTS_TAC `x`
+       THEN ASM_REWRITE_TAC [FDOM_FEMPTY],
+     ASM_REWRITE_TAC [INV_SUC_EQ] 
+       THEN STRIP_TAC
+       THEN IMP_RES_TAC CARD_REL_DEL_LEMMA 
+       THEN RES_TAC]]);
 
 
 (* --------------------------------------------------------------------- *)
 (* Now, ?n. R s n if s is finite.                                        *)
 (* --------------------------------------------------------------------- *)
 
-val CARD_REL_EXISTS_LEMMA = TAC_PROOF((strip_conj card_rel_def,
-Term`!f:('a,'b)fmap. ?n:num. R (FDOM f) n`),
-  INDUCT_THEN fmap_SIMPLE_INDUCT ASSUME_TAC THENL
-  [EXISTS_TAC (Term`0`) THEN ASM_REWRITE_TAC[],
-   FIRST_ASSUM (fn th => fn g => CHOOSE_THEN ASSUME_TAC th g) THEN
-   GEN_TAC THEN GEN_TAC THEN
-   ASM_CASES_TAC (Term`FDOM (f:('a,'b)fmap) x`) THENL
-   [
-    IMP_RES_TAC FDOM_EQ_FDOM_FUPDATE THEN
-    EXISTS_TAC (Term`n:num`) THEN ASM_REWRITE_TAC [],
-    IMP_RES_TAC FDOM_FDOM_DEL THEN
-    EXISTS_TAC (Term`SUC n`) THEN ASM_REWRITE_TAC [] THEN
-    EXISTS_TAC (Term`x:'a`) THEN
-    ASM_REWRITE_TAC [FDOM_FUPDATE] ]]);
+val CARD_REL_EXISTS_LEMMA = TAC_PROOF
+((strip_conj card_rel_def,
+ Term`!f:'a |-> 'b. ?n:num. R (FDOM f) n`),
+ INDUCT_THEN fmap_SIMPLE_INDUCT ASSUME_TAC THENL
+ [Q.EXISTS_TAC `0` THEN ASM_REWRITE_TAC[],
+  FIRST_ASSUM (CHOOSE_THEN ASSUME_TAC)
+    THEN GEN_TAC THEN GEN_TAC 
+    THEN Q.ASM_CASES_TAC `FDOM (f:'a |-> 'b) x` THENL
+    [IMP_RES_TAC FDOM_EQ_FDOM_FUPDATE 
+       THEN Q.EXISTS_TAC `n` 
+       THEN ASM_REWRITE_TAC [],
+     IMP_RES_TAC FDOM_FDOM_DEL 
+       THEN Q.EXISTS_TAC `SUC n`
+       THEN ASM_REWRITE_TAC [] 
+       THEN Q.EXISTS_TAC `x`
+       THEN ASM_REWRITE_TAC [FDOM_FUPDATE]]]);
 
 
 (* --------------------------------------------------------------------- *)
@@ -558,62 +515,64 @@ Term`!f:('a,'b)fmap. ?n:num. R (FDOM f) n`),
 (* Proof modified for Version 12 IMP_RES_THEN            [TFM 91.01.23] *)
 (* --------------------------------------------------------------------- *)
 
-val CARD_REL_THM =
-    TAC_PROOF
-    ((Dsyntax.strip_conj card_rel_def,
-     (Term`!m (f:('a,'b)fmap). (((@n:num. R (FDOM f) n) = m) = R (FDOM f) m)`)),
-     REPEAT STRIP_TAC THEN
-     STRIP_ASSUME_TAC (SPEC (Term`f:('a,'b)fmap`) CARD_REL_EXISTS_LEMMA) THEN
-     EQ_TAC THENL
-     [DISCH_THEN (SUBST1_TAC o SYM) THEN CONV_TAC SELECT_CONV THEN
-      EXISTS_TAC (Term`n:num`) THEN FIRST_ASSUM MATCH_ACCEPT_TAC,
-      STRIP_TAC THEN
-      IMP_RES_THEN ASSUME_TAC CARD_REL_UNIQUE THEN
-      CONV_TAC SYM_CONV THEN
-      FIRST_ASSUM MATCH_MP_TAC THEN
-      CONV_TAC SELECT_CONV THEN
-      EXISTS_TAC (Term`n:num`) THEN FIRST_ASSUM MATCH_ACCEPT_TAC]);
+val CARD_REL_THM = TAC_PROOF
+((strip_conj card_rel_def,
+  Term`!m (f:'a |-> 'b). (((@n:num. R (FDOM f) n) = m) = R (FDOM f) m)`),
+  REPEAT STRIP_TAC 
+   THEN STRIP_ASSUME_TAC (SPEC_ALL CARD_REL_EXISTS_LEMMA)
+   THEN EQ_TAC THENL
+   [DISCH_THEN (SUBST1_TAC o SYM) THEN CONV_TAC SELECT_CONV 
+      THEN Q.EXISTS_TAC `n` 
+      THEN FIRST_ASSUM MATCH_ACCEPT_TAC,
+    STRIP_TAC 
+      THEN IMP_RES_THEN ASSUME_TAC CARD_REL_UNIQUE 
+      THEN CONV_TAC SYM_CONV 
+      THEN FIRST_ASSUM MATCH_MP_TAC 
+      THEN CONV_TAC SELECT_CONV 
+      THEN Q.EXISTS_TAC `n` 
+      THEN FIRST_ASSUM MATCH_ACCEPT_TAC]);
 
 
 (* --------------------------------------------------------------------- *)
 (* Now, prove the existence of the required cardinality function.       *)
 (* --------------------------------------------------------------------- *)
 
-val DOM_CARD_EXISTS = TAC_PROOF(([],
-(Term`?CARD.
-       (CARD (FDOM (FEMPTY:('a,'b)fmap)) = 0) /\
-       (!(f:('a,'b)fmap) x y.
-           CARD(FDOM (FUPDATE f (x,y))) = (FDOM f x => CARD (FDOM f) |
-                                                    SUC(CARD (FDOM f))))`)),
-     STRIP_ASSUME_TAC CARD_REL_EXISTS THEN
-     EXISTS_TAC (Term`\s:'a->bool. @n:num. R s n`) THEN
-     CONV_TAC (ONCE_DEPTH_CONV BETA_CONV) THEN CONJ_TAC THENL
-     [ASM_REWRITE_TAC [CARD_REL_THM],
-      REPEAT STRIP_TAC THEN COND_CASES_TAC THENL
-      [IMP_RES_TAC FDOM_EQ_FDOM_FUPDATE THEN ASM_REWRITE_TAC [],
-       ASM_REWRITE_TAC [CARD_REL_THM] THEN
-       EXISTS_TAC (Term`x:'a`) THEN
-       IMP_RES_TAC FDOM_FDOM_DEL THEN
-       ASM_REWRITE_TAC [FDOM_FUPDATE] THEN
-       CONV_TAC SELECT_CONV THEN
-       REWRITE_TAC [CARD_REL_EXISTS_LEMMA]
-      ]]);
+val FEMPTY = Term`FEMPTY : 'a |-> 'b`;
+val fmap   = Term`f : 'a |-> 'b`;
+
+val DOM_CARD_EXISTS = Q.prove
+(`?CARD. (CARD (FDOM ^FEMPTY) = 0) /\
+         (!^fmap x y.
+           CARD(FDOM (FUPDATE f (x,y))) = 
+            if FDOM f x then CARD (FDOM f) 
+                        else SUC (CARD (FDOM f)))`,
+ STRIP_ASSUME_TAC CARD_REL_EXISTS 
+   THEN Q.EXISTS_TAC `\s. @n:num. R s n`
+   THEN CONV_TAC (ONCE_DEPTH_CONV BETA_CONV) 
+   THEN CONJ_TAC THENL
+   [ASM_REWRITE_TAC [CARD_REL_THM],
+    REPEAT STRIP_TAC THEN COND_CASES_TAC THENL
+    [IMP_RES_TAC FDOM_EQ_FDOM_FUPDATE THEN ASM_REWRITE_TAC [],
+     ASM_REWRITE_TAC [CARD_REL_THM] 
+       THEN Q.EXISTS_TAC `x` 
+       THEN IMP_RES_TAC FDOM_FDOM_DEL 
+       THEN ASM_REWRITE_TAC [FDOM_FUPDATE] 
+       THEN CONV_TAC SELECT_CONV 
+       THEN REWRITE_TAC [CARD_REL_EXISTS_LEMMA]]]);
 
 
-(* --------------------------------------------------------------------- *)
-(* Finally lets make this a function over finite maps rather than domains*)
-(* --------------------------------------------------------------------- *)
+(* ----------------------------------------------------------------------- *)
+(* Finally let's make this a function over finite maps rather than domains *)
+(* ----------------------------------------------------------------------- *)
 
-val CARD_EXISTS = TAC_PROOF(([],
-(Term`?CARD.
-       (CARD (FEMPTY:('a,'b)fmap) = 0) /\
-       (!(f:('a,'b)fmap) x y.
-           CARD(FUPDATE f (x,y)) = (FDOM f x => CARD f |
-                                                    SUC(CARD f)))`)),
-STRIP_ASSUME_TAC DOM_CARD_EXISTS THEN
-EXISTS_TAC (Term`\(x:('a,'b)fmap). (CARD:('a -> bool) -> num)  (FDOM x)`) THEN
-BETA_TAC THEN
-ASM_REWRITE_TAC []);
+val CARD_EXISTS = Q.prove
+(`?CARD. (CARD ^FEMPTY = 0) /\
+       (!^fmap x y.
+           CARD(FUPDATE f (x,y)) = if FDOM f x then CARD f else SUC(CARD f))`,
+ STRIP_ASSUME_TAC DOM_CARD_EXISTS 
+   THEN Q.EXISTS_TAC `\x. CARD (FDOM x)`
+   THEN BETA_TAC
+   THEN ASM_REWRITE_TAC []);
 
 
 (* --------------------------------------------------------------------- *)
@@ -625,1473 +584,1280 @@ val FCARD_DEF = new_specification
                   consts=[{const_name="FCARD",fixity=Prefix}]};
 
 (* --------------------------------------------------------------------- *)
-(* Various cardinality results.                                         *)
+(* Basic cardinality results.                                            *)
 (* --------------------------------------------------------------------- *)
 
 val FCARD_FEMPTY = save_thm("FCARD_FEMPTY",CONJUNCT1 FCARD_DEF);
 
 val FCARD_FUPDATE = save_thm("FCARD_FUPDATE",CONJUNCT2 FCARD_DEF);
 
-val FCARD_0_FEMPTY_LEMMA = prove(
-Term`!f: ('a,'b) fmap. (FCARD f = 0) ==> (f = FEMPTY)`,
-INDUCT_THEN fmap_SIMPLE_INDUCT ASSUME_TAC THENL
-[
- REWRITE_TAC [FCARD_FEMPTY],
- GEN_TAC THEN GEN_TAC THEN
- REWRITE_TAC [FCARD_FUPDATE] THEN
- ASM_CASES_TAC (Term`FDOM (f:('a,'b) fmap) x`) THEN
- ASM_REWRITE_TAC [] THENL
- [ DISCH_THEN (fn th =>
-    FIRST_ASSUM (fn ass => SUBST_ALL_TAC (MATCH_MP ass th))) THEN
-   POP_ASSUM (CHECK_ASSUME_TAC o (REWRITE_RULE [FDOM_FEMPTY])),
-   REWRITE_TAC [numTheory.NOT_SUC]
- ]
-]);
+val FCARD_0_FEMPTY_LEMMA = Q.prove
+(`!^fmap. (FCARD f = 0) ==> (f = FEMPTY)`,
+ INDUCT_THEN fmap_SIMPLE_INDUCT ASSUME_TAC THENL
+ [REWRITE_TAC [FCARD_FEMPTY],
+  GEN_TAC THEN GEN_TAC 
+    THEN REWRITE_TAC [FCARD_FUPDATE] 
+    THEN Q.ASM_CASES_TAC `FDOM f x` 
+    THEN ASM_REWRITE_TAC [] THENL
+    [DISCH_THEN (fn th => FIRST_ASSUM (fn ass => 
+                   SUBST_ALL_TAC (MATCH_MP ass th))) 
+       THEN POP_ASSUM (CHECK_ASSUME_TAC o (REWRITE_RULE [FDOM_FEMPTY])),
+     REWRITE_TAC [NOT_SUC]]]);
 
-val FCARD_0_FEMPTY = store_thm("FCARD_0_FEMPTY",
-Term`!f: ('a,'b) fmap. (FCARD f = 0) = (f = FEMPTY)`,
+
+val FCARD_0_FEMPTY = Q.store_thm("FCARD_0_FEMPTY",
+`!^fmap. (FCARD f = 0) = (f = FEMPTY)`,
 GEN_TAC THEN EQ_TAC THENL
-[
- REWRITE_TAC [FCARD_0_FEMPTY_LEMMA],
- DISCH_THEN (fn th => ASM_REWRITE_TAC [th, FCARD_FEMPTY])
-]);
+[REWRITE_TAC [FCARD_0_FEMPTY_LEMMA],
+ DISCH_THEN (fn th => ASM_REWRITE_TAC [th, FCARD_FEMPTY])]);
 
 
+(*---------------------------------------------------------------------------
+         A more useful induction theorem
+ ---------------------------------------------------------------------------*)
 
-(*-----------------------------------------------------
+val exist_map_no_x_rep = (BETA_RULE o BETA_RULE) (Q.prove
+(`!f:'a->'b+one. 
+   is_fmap f 
+    ==> !x. ?f'. !y. 
+           is_fmap f' 
+        /\ (^update_rep f x y  = ^update_rep f' x y)
+        /\ (!x'. f' x' = (if x' = x then INR one else f x'))
+        /\ (FDOM (fmap_ABS f') = FDOMDEL (FDOM (fmap_ABS f)) x)`,
+ BETA_TAC 
+  THEN HO_MATCH_MP_TAC strong_ind
+  THEN CONJ_TAC THENL
+  [GEN_TAC  
+     THEN EXISTS_TAC empty_rep THEN BETA_TAC
+     THEN REWRITE_TAC[SYM FEMPTY_DEF,FDOM_FEMPTY,FDOMDEL_FEMPTY,is_fmap_empty]
+     THEN GEN_TAC THEN COND_CASES_TAC THEN ASM_REWRITE_TAC[],
+   BETA_TAC 
+     THEN CONV_TAC (DEPTH_CONV FORALL_IMP_CONV)
+     THEN GEN_TAC THEN STRIP_TAC
+     THEN REPEAT GEN_TAC
+     THEN POP_ASSUM (STRIP_ASSUME_TAC o SPEC_ALL)
+     THEN Q.ASM_CASES_TAC `a = x` THENL
+     [Q.EXISTS_TAC `f'` 
+        THEN GEN_TAC 
+        THEN IMP_RES_TAC is_fmap_REP_ABS
+        THEN CONV_TAC (ONCE_DEPTH_CONV FUN_EQ_CONV) 
+        THEN REWRITE_TAC [FDOMDEL_DEF] 
+        THEN ONCE_ASM_REWRITE_TAC [] 
+        THEN REWRITE_TAC [FDOMDEL_DEF] 
+        THEN POP_ASSUM (fn thm => REWRITE_TAC [REWRITE_RULE [thm, FUPDATE_DEF]
+               (SPEC (Term`fmap_ABS (f:'a -> 'b + one)`) FDOM_FUPDATE)]) 
+        THEN ASM_REWRITE_TAC [update_same_rep]  
+        THEN STRIP_TAC THENL
+        [GEN_TAC THEN COND_CASES_TAC THEN REWRITE_TAC [],
+         GEN_TAC THEN Q.ASM_CASES_TAC `x' = x`
+         THEN ASM_REWRITE_TAC []],
+      Q.EXISTS_TAC `^update_rep (f':'a -> 'b + one) a b`
+         THEN BETA_TAC THEN GEN_TAC 
+         THEN IMP_RES_TAC  update_commutes_rep 
+         THEN POP_ASSUM (fn thm => REWRITE_TAC [thm]) 
+         THEN REPEAT STRIP_TAC THENL
+         [MATCH_MP_TAC is_fmap_update THEN ASM_REWRITE_TAC [],
+          MATCH_MP_TAC EQ_EXT 
+             THEN GEN_TAC THEN BETA_TAC 
+             THEN COND_CASES_TAC 
+             THEN ASM_REWRITE_TAC [] 
+             THEN COND_CASES_TAC THEN REWRITE_TAC [],
+          Q.ASM_CASES_TAC `x' = a` THEN ASM_REWRITE_TAC [],
+          CONV_TAC (ONCE_DEPTH_CONV FUN_EQ_CONV)
+             THEN ASSUM_LIST (fn ths => REWRITE_TAC 
+                    [REWRITE_RULE [MATCH_MP is_fmap_REP_ABS
+                             (CONJUNCT1 (SPEC (Term`y:'b`) (el 2 ths))),
+                            FUPDATE_DEF] (Q.SPEC `fmap_ABS f'` FDOM_FUPDATE)])
+             THEN ASM_REWRITE_TAC [FDOMDEL_DEF] 
+             THEN IMP_RES_TAC is_fmap_REP_ABS 
+             THEN POP_ASSUM (fn thm => REWRITE_TAC 
+                               [REWRITE_RULE [thm, FUPDATE_DEF]
+                                (Q.SPEC `fmap_ABS f` FDOM_FUPDATE)]) 
+             THEN GEN_TAC 
+             THEN Q.ASM_CASES_TAC `x' = a` 
+             THEN ASM_REWRITE_TAC []]]]));
 
------------------------------------------------------*)
+val conj_context_lemma = Q.prove 
+(`!p q r. (p /\ r /\ (p ==> r ==> q)) ==> (p /\ q /\ r)`,
+ REPEAT STRIP_TAC THEN RES_TAC THEN ASM_REWRITE_TAC []);
 
+val lemma2 = Q.prove 
+(`!(x:'a |-> 'b) y. (x = y) ==> (FCARD x = FCARD y)`,
+ REPEAT STRIP_TAC THEN ASM_REWRITE_TAC []);
 
-
-
-val exist_map_no_x_rep = (BETA_RULE o BETA_RULE) (prove
-(Term`!(f:'a->'b+one). is_fmap f ==>
-(!x. ?f'. !y.
-(is_fmap f') /\
-(^update_rep f x y  = ^update_rep f' x y) /\
-(!x'. (f' x' =  ((x' = x) => INR one | f x'))) /\
-(FDOM (fmap_ABS f') = (FDOMDEL (FDOM (fmap_ABS f)) x)))`,
-BETA_TAC THEN
-ind_defLib.RULE_INDUCT_THEN strong_is_fmap_ind ASSUME_TAC ASSUME_TAC THENL
-[
- GEN_TAC THEN
- EXISTS_TAC (Term`^empty_rep :'a->'b+one`) THEN
- STRIP_TAC THEN
- REWRITE_TAC [SYM (FEMPTY_DEF), FDOM_FEMPTY, FDOMDEL_FEMPTY, is_fmap_empty] THEN
- GEN_TAC THEN COND_CASES_TAC THEN ASM_REWRITE_TAC []
- ,
- REPEAT GEN_TAC THEN BETA_TAC THEN
- POP_ASSUM (STRIP_ASSUME_TAC o SPEC (Term`x:'a`)) THEN
- ASM_CASES_TAC (Term`(a:'a) = x`) THENL
- [
-  EXISTS_TAC (Term`f':'a -> 'b + one`) THEN
-  GEN_TAC THEN
-  IMP_RES_TAC is_fmap_REP_ABS THEN
-   CONV_TAC (ONCE_DEPTH_CONV FUN_EQ_CONV) THEN
-  REWRITE_TAC [FDOMDEL_DEF] THEN
-  ONCE_ASM_REWRITE_TAC [] THEN
-  REWRITE_TAC [FDOMDEL_DEF] THEN
-
-  POP_ASSUM (fn thm => REWRITE_TAC [REWRITE_RULE [thm, FUPDATE_DEF]
-        (SPEC (Term`fmap_ABS (f:'a -> 'b + one)`) FDOM_FUPDATE)]) THEN
-  ASM_REWRITE_TAC [update_same_rep]  THEN
-  STRIP_TAC THENL
-  [GEN_TAC THEN COND_CASES_TAC THEN REWRITE_TAC [],
-   GEN_TAC THEN ASM_CASES_TAC (Term`(x':'a) = x`) THEN
-   ASM_REWRITE_TAC []]
-  ,
-  EXISTS_TAC (Term`^update_rep (f':'a -> 'b + one) a b`) THEN
-  BETA_TAC THEN GEN_TAC THEN
-  IMP_RES_TAC  update_commutes_rep THEN
-  POP_ASSUM (fn thm => REWRITE_TAC [thm]) THEN
-  REPEAT STRIP_TAC THENL
-  [
-   MATCH_MP_TAC is_fmap_update THEN ASM_REWRITE_TAC [],
-   MATCH_MP_TAC EQ_EXT THEN GEN_TAC THEN BETA_TAC THEN
-   COND_CASES_TAC THEN ASM_REWRITE_TAC [] THEN
-   COND_CASES_TAC THEN REWRITE_TAC [],
-   ASM_CASES_TAC (Term`(x':'a) = a`) THEN ASM_REWRITE_TAC [],
-   CONV_TAC (ONCE_DEPTH_CONV FUN_EQ_CONV) THEN
-   ASSUM_LIST (fn ths =>
-    REWRITE_TAC [REWRITE_RULE [
-     MATCH_MP is_fmap_REP_ABS
-     (CONJUNCT1 (SPEC (Term`y:'b`) (el 2 ths))),  FUPDATE_DEF]
-        (SPEC (Term`fmap_ABS (f':'a -> 'b + one)`) FDOM_FUPDATE)]) THEN
-   ASM_REWRITE_TAC [FDOMDEL_DEF] THEN
-   IMP_RES_TAC is_fmap_REP_ABS THEN
-   POP_ASSUM (fn thm => REWRITE_TAC [REWRITE_RULE [thm, FUPDATE_DEF]
-        (SPEC (Term`fmap_ABS (f:'a -> 'b + one)`) FDOM_FUPDATE)]) THEN
-   GEN_TAC THEN
-   ASM_CASES_TAC (Term`(x':'a) = a`) THEN
-   ASM_REWRITE_TAC []
-  ]]
- ]
-));
-
-
-
-val conj_context_lemma = prove (
-Term`!p q r. (p /\ r /\ (p ==> r ==> q)) ==> (p /\ q /\ r)`,
-REPEAT STRIP_TAC THEN RES_TAC THEN ASM_REWRITE_TAC []);
-
-val lemma2 = prove (Term`!(x:('a,'b) fmap) y. (x = y) ==> (FCARD x = FCARD y)`,
-REPEAT STRIP_TAC THEN ASM_REWRITE_TAC []);
-
-val CARD_DOM_SUC = prove
-(Term`!n (f:('a,'b) fmap). (FCARD  f = SUC n) ==>
-   ?f' x y. (~FDOM f' x) /\
-             (FCARD  f' = n) /\
-             (f = FUPDATE f' (x,y)) `,
-GEN_TAC THEN
-INDUCT_THEN fmap_SIMPLE_INDUCT ASSUME_TAC THENL
-[
- REWRITE_TAC [FCARD_FEMPTY,
-              NOT_EQ_SYM (SPEC (Term`n:num`) (numTheory.NOT_SUC)) ],
- REPEAT GEN_TAC THEN
- REWRITE_TAC [FCARD_FUPDATE] THEN
- COND_CASES_TAC THENL
-[
- DISCH_TAC THEN
- STRIP_ASSUME_TAC
-  (REWRITE_RULE [fmap_ISO_DEF]
-   (SPEC (Term`x:'a`)
-     (MATCH_MP exist_map_no_x_rep
-        (SPEC (Term`f:('a,'b) fmap`) is_fmap_REP)))) THEN
- POP_ASSUM (STRIP_ASSUME_TAC o SPEC (Term`y:'b`)) THEN
- EXISTS_TAC (Term`(fmap_ABS f'):('a,'b) fmap`) THEN
- EXISTS_TAC (Term`x:'a`) THEN
- EXISTS_TAC (Term`y:'b`) THEN
- IMP_RES_TAC is_fmap_REP_ABS THEN
- MATCH_MP_TAC conj_context_lemma THEN
- REPEAT CONJ_TAC THENL
- [ ASM_REWRITE_TAC [FDOM_DEF, sumTheory.ISL],
-   ASM_REWRITE_TAC [FUPDATE_DEF],
-   DISCH_TAC THEN
-   ASSUM_LIST (fn ass =>
-   DISCH_THEN (fn th =>
-   ASSUME_TAC (SYM
-        (REWRITE_RULE (FCARD_FUPDATE::prim_recTheory.INV_SUC_EQ::ass)
-                      (MATCH_MP lemma2 th))))) THEN
- ASM_REWRITE_TAC []]
-,
- DISCH_THEN (ASSUME_TAC o REWRITE_RULE [prim_recTheory.INV_SUC_EQ]) THEN
-  EXISTS_TAC (Term`f:('a,'b) fmap`) THEN
- EXISTS_TAC (Term`x:'a`) THEN
- EXISTS_TAC (Term`y:'b`) THEN
- ASM_REWRITE_TAC []
-]])
-   ;
-
+val CARD_DOM_SUC = Q.prove
+(`!n (f:'a |-> 'b). 
+    (FCARD f = SUC n)
+      ==>
+    ?f' x y. ~FDOM f' x /\ (FCARD f' = n) /\ (f = FUPDATE f' (x,y))`,
+ GEN_TAC 
+  THEN INDUCT_THEN fmap_SIMPLE_INDUCT ASSUME_TAC THENL
+  [REWRITE_TAC [FCARD_FEMPTY, NOT_EQ_SYM (SPEC_ALL NOT_SUC)],
+   REPEAT GEN_TAC 
+     THEN REWRITE_TAC [FCARD_FUPDATE] 
+     THEN COND_CASES_TAC THENL
+     [DISCH_TAC 
+       THEN STRIP_ASSUME_TAC
+             (REWRITE_RULE [fmap_ISO_DEF]
+               (Q.SPEC `x` 
+                 (MATCH_MP exist_map_no_x_rep
+                   (Q.SPEC `f` is_fmap_REP)))) 
+       THEN POP_ASSUM (STRIP_ASSUME_TAC o Q.SPEC `y`)
+       THEN Q.EXISTS_TAC `fmap_ABS f'` 
+       THEN Q.EXISTS_TAC `x` 
+       THEN Q.EXISTS_TAC `y`
+       THEN IMP_RES_TAC is_fmap_REP_ABS 
+       THEN MATCH_MP_TAC conj_context_lemma 
+       THEN REPEAT CONJ_TAC THENL
+       [ASM_REWRITE_TAC [FDOM_DEF, sumTheory.ISL],
+        ASM_REWRITE_TAC [FUPDATE_DEF],
+        DISCH_TAC 
+           THEN ASSUM_LIST (fn ass =>
+                DISCH_THEN (fn th =>
+                  ASSUME_TAC 
+                    (SYM (REWRITE_RULE (FCARD_FUPDATE::INV_SUC_EQ::ass)
+                             (MATCH_MP lemma2 th)))))
+           THEN ASM_REWRITE_TAC []],
+      DISCH_THEN (ASSUME_TAC o REWRITE_RULE [INV_SUC_EQ])
+         THEN Q.EXISTS_TAC `f`
+         THEN Q.EXISTS_TAC `x` 
+         THEN Q.EXISTS_TAC `y`
+         THEN ASM_REWRITE_TAC []]]);
 
 
 val card_induct =
-let
-val thm1 =
-   BETA_RULE (SPEC (Term`\i. (!f: ('a,'b) fmap.
-                     (FCARD f = i) ==> P f)`)
-                    (numTheory.INDUCTION));
-val thm2 =
-          GEN_ALL
-           (DISCH_ALL
-            (GEN (Term`f1: ('a,'b) fmap`)
-             (REWRITE_RULE []
-              (SPECL [Term`FCARD (f1: ('a,'b) fmap)`,
-                     Term`f1: ('a,'b) fmap`] (
-               UNDISCH_ALL thm1)))))
-in
- prove (
-Term`!P.
-     (P FEMPTY) /\
-     (!n.
-       (!f:('a,'b) fmap. (FCARD f = n) ==> P f) ==>
-       (!f:('a,'b) fmap. (FCARD f = SUC n) ==> P f)) ==>
-     (!f:('a,'b) fmap. P f)`,
-  REPEAT STRIP_TAC THEN
-  MATCH_MP_TAC thm2 THEN
-  CONJ_TAC THENL
-  [
-   REWRITE_TAC [FCARD_0_FEMPTY] THEN
-   REPEAT STRIP_TAC THEN
-   ASM_REWRITE_TAC [],
-   ASM_REWRITE_TAC []
-  ])
-end;
+ let val thm1 = BETA_RULE 
+       (SPEC (Term`\i. (!f: ('a,'b) fmap. (FCARD f = i) ==> P f)`) INDUCTION)
+     val thm2 = GEN_ALL (DISCH_ALL
+       (GEN (Term`f1: ('a,'b) fmap`)
+            (REWRITE_RULE []
+                 (Q.SPECL [`FCARD (f1: ('a,'b) fmap)`,`f1: ('a,'b) fmap`] 
+                      (UNDISCH_ALL thm1)))))
+ in Q.prove 
+ (`!P. P FEMPTY /\
+       (!n. (!f:('a,'b) fmap. (FCARD f = n) ==> P f) ==>
+            (!f:('a,'b) fmap. (FCARD f = SUC n) ==> P f)) 
+       ==>
+       !^fmap. P f`,
+  REPEAT STRIP_TAC 
+     THEN MATCH_MP_TAC thm2 
+     THEN CONJ_TAC THENL
+     [REWRITE_TAC [FCARD_0_FEMPTY] 
+        THEN REPEAT STRIP_TAC 
+        THEN ASM_REWRITE_TAC [],
+      ASM_REWRITE_TAC []])
+ end;
 
 
-val fmap_INDUCT = store_thm("fmap_INDUCT",
-Term`!P. P FEMPTY /\
-       (!f. P f ==> (!x y.  (~FDOM f x) ==> P(FUPDATE f (x,y)))) ==>
-       !f:('a,'b) fmap. P f`,
-GEN_TAC  THEN STRIP_TAC THEN
-MATCH_MP_TAC card_induct THEN
-ASM_REWRITE_TAC [] THEN
-REPEAT STRIP_TAC THEN
-IMP_RES_TAC  CARD_DOM_SUC THEN
-RES_TAC THEN RES_TAC THEN
-ASM_REWRITE_TAC []);
+val fmap_INDUCT = Q.store_thm("fmap_INDUCT",
+`!P. P FEMPTY /\
+     (!f. P f ==> !x y. ~FDOM f x ==> P (FUPDATE f (x,y)))
+       ==>
+     !^fmap. P f`,
+GEN_TAC THEN STRIP_TAC 
+  THEN MATCH_MP_TAC card_induct 
+  THEN ASM_REWRITE_TAC [] 
+  THEN REPEAT STRIP_TAC 
+  THEN IMP_RES_TAC  CARD_DOM_SUC 
+  THEN RES_TAC THEN RES_TAC 
+  THEN ASM_REWRITE_TAC []);
 
 
-(*EQUALITY*)
+(*---------------------------------------------------------------------------
+     Equality of finite maps
+ ---------------------------------------------------------------------------*)
 
-(*We now need to prove a lemma *)
-
-val FUPDATE_ABSORB_THM = prove (Term
-`!(f:('a,'b) fmap) x y.
-   (FDOM f x)  /\ (FAPPLY f x = y) ==> (FUPDATE f (x,y) = f)`,
-
-INDUCT_THEN  fmap_SIMPLE_INDUCT STRIP_ASSUME_TAC THEN
-REWRITE_TAC [FDOM_FEMPTY] THEN
-REPEAT STRIP_TAC THEN
-ASM_CASES_TAC (Term`(x:'a) = x'`) THENL
-[  ASM_REWRITE_TAC [FUPDATE_EQ] THEN
-   ASM_CASES_TAC (Term`(y:'b) = y'`) THEN
-   ASM_REWRITE_TAC [] THEN
-   ASSUM_LIST
-   (fn ths => ASSUME_TAC (
-     REWRITE_RULE [el 2 ths, FAPPLY_FUPDATE, el 1 ths] (el 3 ths))) THEN
-   UNDISCH_TAC (Term`F`) THEN
-   REWRITE_TAC [],
-   IMP_RES_TAC FUPDATE_COMMUTES THEN
-   ASM_REWRITE_TAC [] THEN
-   ASSUM_LIST (fn ths => ASSUME_TAC (
-     REWRITE_RULE [
-       MATCH_MP NOT_EQ_FAPPLY (NOT_EQ_SYM (el 2 ths))]
-        (el 3 ths))) THEN
-   ASSUM_LIST (fn ths => ASSUME_TAC (
-     REWRITE_RULE [FDOM_FUPDATE, (NOT_EQ_SYM (el 3 ths))]
-        (el 5 ths))) THEN
-   RES_TAC THEN
-   ASM_REWRITE_TAC []
-]
-);
+val FUPDATE_ABSORB_THM = Q.prove 
+(`!(f:'a |-> 'b) x y.
+    FDOM f x /\ (FAPPLY f x = y) ==> (FUPDATE f (x,y) = f)`,
+ INDUCT_THEN fmap_SIMPLE_INDUCT STRIP_ASSUME_TAC 
+   THEN REWRITE_TAC [FDOM_FEMPTY] 
+   THEN REPEAT STRIP_TAC 
+   THEN Q.ASM_CASES_TAC `x = x'` THENL
+   [ASM_REWRITE_TAC [FUPDATE_EQ] 
+      THEN ASM_CASES_TAC (Term`(y:'b) = y'`) 
+      THEN ASM_REWRITE_TAC [] 
+      THEN ASSUM_LIST (fn ths => ASSUME_TAC 
+             (REWRITE_RULE [el 2 ths, FAPPLY_FUPDATE, el 1 ths] (el 3 ths)))
+      THEN UNDISCH_TAC F 
+      THEN REWRITE_TAC [],
+    IMP_RES_TAC FUPDATE_COMMUTES 
+      THEN ASM_REWRITE_TAC [] 
+      THEN ASSUM_LIST (fn ths => ASSUME_TAC 
+           (REWRITE_RULE [MATCH_MP NOT_EQ_FAPPLY (NOT_EQ_SYM (el 2 ths))]
+                    (el 3 ths))) 
+      THEN ASSUM_LIST (fn ths => ASSUME_TAC 
+             (REWRITE_RULE [FDOM_FUPDATE,(NOT_EQ_SYM (el 3 ths))](el 5 ths)))
+      THEN RES_TAC 
+      THEN ASM_REWRITE_TAC []]);
 
 
-val update_eq_not_x =
-     prove (Term`!(f:('a,'b) fmap).
-(!x. ?f'.  !y.
-(FUPDATE f (x,y)  = FUPDATE f' (x,y)) /\
-(~FDOM f' x))`,
-INDUCT_THEN fmap_SIMPLE_INDUCT ASSUME_TAC THENL
-[
- GEN_TAC THEN EXISTS_TAC (Term`FEMPTY : ('a,'b) fmap`) THEN
- REWRITE_TAC [FDOM_FEMPTY],
- GEN_TAC THEN GEN_TAC THEN GEN_TAC THEN
- POP_ASSUM (STRIP_ASSUME_TAC o (SPEC (Term`x':'a`))) THEN
- ASM_CASES_TAC (Term`(x':'a) = x`) THENL
- [
-  EXISTS_TAC (Term`f':('a,'b) fmap`) THEN
-  ASM_REWRITE_TAC [FUPDATE_EQ] THEN
-  POP_ASSUM (fn th => ASM_REWRITE_TAC [SYM th]),
-  EXISTS_TAC (Term`FUPDATE (f':('a,'b) fmap) (x,y)`) THEN
-  IMP_RES_TAC  FUPDATE_COMMUTES THEN
-  POP_ASSUM (ASSUME_TAC o (ONCE_REWRITE_RULE [EQ_SYM_EQ])) THEN
-  ASM_REWRITE_TAC [FDOM_FUPDATE]
- ]
-]);
+val update_eq_not_x = Q.prove 
+(`!(f:'a |-> 'b). 
+      !x. ?f'. !y. (FUPDATE f (x,y) = FUPDATE f' (x,y)) /\ ~FDOM f' x`,
+ INDUCT_THEN fmap_SIMPLE_INDUCT ASSUME_TAC THENL
+ [GEN_TAC THEN Q.EXISTS_TAC `FEMPTY` 
+   THEN REWRITE_TAC [FDOM_FEMPTY],
+  NTAC 3 GEN_TAC
+    THEN POP_ASSUM (STRIP_ASSUME_TAC o Q.SPEC`x'`)
+    THEN Q.ASM_CASES_TAC `x' = x` THENL
+    [Q.EXISTS_TAC `f'`
+       THEN ASM_REWRITE_TAC [FUPDATE_EQ] 
+       THEN POP_ASSUM (fn th => ASM_REWRITE_TAC [SYM th]),
+     Q.EXISTS_TAC `FUPDATE f' (x,y)`
+       THEN IMP_RES_TAC FUPDATE_COMMUTES 
+       THEN POP_ASSUM (ASSUME_TAC o (ONCE_REWRITE_RULE [EQ_SYM_EQ])) 
+       THEN ASM_REWRITE_TAC [FDOM_FUPDATE]]]);
 
 
-val lemma9 = BETA_RULE (prove (
-Term`!x y (f1:('a,'b)fmap) f2. (f1 = f2) ==>
-    (( \ (f:('a,'b)fmap).FUPDATE f (x,y)) f1
-          = ( \( f:('a,'b)fmap).FUPDATE f (x,y)) f2)`,
-REPEAT STRIP_TAC THEN
-AP_TERM_TAC THEN
-ASM_REWRITE_TAC []));
+val lemma9 = BETA_RULE (Q.prove 
+(`!x y (f1:('a,'b)fmap) f2. 
+   (f1 = f2) ==>
+    ((\f.FUPDATE f (x,y)) f1 = (\f. FUPDATE f (x,y)) f2)`,
+ REPEAT STRIP_TAC 
+   THEN AP_TERM_TAC 
+   THEN ASM_REWRITE_TAC []));
 
-val NOT_FDOM_FAPPLY_FEMPTY = store_thm ("NOT_FDOM_FAPPLY_FEMPTY",
-Term`!(f:('a,'b)fmap) x. (~FDOM f x) ==>
-          (FAPPLY f x = FAPPLY FEMPTY x)`,
-INDUCT_THEN fmap_INDUCT ASSUME_TAC THENL
-[REWRITE_TAC [],
- REPEAT GEN_TAC THEN STRIP_TAC THEN GEN_TAC  THEN
- ASM_CASES_TAC (Term`(x':'a) = x`) THENL
- [ASM_REWRITE_TAC [FDOM_FUPDATE],
- IMP_RES_TAC NOT_EQ_FAPPLY THEN
-  ASM_REWRITE_TAC [FDOM_FUPDATE]
- ]
-]);
+val NOT_FDOM_FAPPLY_FEMPTY = Q.store_thm 
+("NOT_FDOM_FAPPLY_FEMPTY",
+ `!^fmap x. ~FDOM f x ==> (FAPPLY f x = FAPPLY FEMPTY x)`,
+ INDUCT_THEN fmap_INDUCT ASSUME_TAC THENL
+ [REWRITE_TAC [],
+  REPEAT GEN_TAC 
+    THEN STRIP_TAC 
+    THEN GEN_TAC 
+    THEN Q.ASM_CASES_TAC `x' = x` THENL
+    [ASM_REWRITE_TAC [FDOM_FUPDATE],
+     IMP_RES_TAC NOT_EQ_FAPPLY 
+       THEN ASM_REWRITE_TAC [FDOM_FUPDATE]]]);
 
+val fmap_EQ_2 = Q.prove 
+(`!(f:'a |-> 'b) g. (FDOM f = FDOM g) /\ (FAPPLY f = FAPPLY g) ==> (f = g)`,
+ INDUCT_THEN fmap_INDUCT ASSUME_TAC THENL
+ [GEN_TAC 
+    THEN CONV_TAC (DEPTH_CONV FUN_EQ_CONV) 
+    THEN PURE_REWRITE_TAC [FDOM_FEMPTY] 
+    THEN PURE_ONCE_REWRITE_TAC [EQ_SYM_EQ, FDOM_F_FEMPTY] 
+    THEN REWRITE_TAC [FDOM_F_FEMPTY] 
+    THEN STRIP_TAC THEN ASM_REWRITE_TAC [],
+  REPEAT GEN_TAC THEN STRIP_TAC THEN GEN_TAC 
+    THEN STRIP_ASSUME_TAC (Q.SPECL [`g`,`x`] update_eq_not_x) 
+    THEN POP_ASSUM (ASSUME_TAC o Q.SPEC `FAPPLY g x`)
+    THEN CONV_TAC (DEPTH_CONV FUN_EQ_CONV) 
+    THEN STRIP_TAC 
+    THEN ASSUM_LIST (fn ths => ASSUME_TAC
+        (REWRITE_RULE [FDOM_FUPDATE] (Q.SPEC `x` (el 2 ths)))) 
+    THEN ASSUM_LIST (fn ths => ONCE_REWRITE_TAC 
+           [SYM(REWRITE_RULE [el 1 ths]
+                 (Q.SPECL [`g`, `x`,`FAPPLY g x`] FUPDATE_ABSORB_THM))]) 
+    THEN ASM_REWRITE_TAC [] 
+    THEN ASSUM_LIST (fn ths => REWRITE_TAC [
+                   ONCE_REWRITE_RULE [EQ_SYM_EQ] (el 2 ths)]) 
+    THEN REWRITE_TAC [FAPPLY_FUPDATE] 
+    THEN MATCH_MP_TAC lemma9 
+    THEN FIRST_ASSUM MATCH_MP_TAC 
+    THEN CONV_TAC (DEPTH_CONV FUN_EQ_CONV) 
+    THEN CONJ_TAC THENL
+    [ASSUM_LIST (fn ths => ASSUME_TAC
+        (CONV_RULE (DEPTH_CONV FUN_EQ_CONV)
+          (SYM (CONJUNCT1 (MATCH_MP fmap_EQ_1 (CONJUNCT1 (el 4 ths))))))) 
+       THEN GEN_TAC 
+       THEN Q.ASM_CASES_TAC `x' = x` THENL
+       [ASM_REWRITE_TAC [],
+        ASSUM_LIST (fn ths => REWRITE_TAC
+             [REWRITE_RULE [FDOM_FUPDATE, el 1 ths] (Q.SPEC `x'` (el 2 ths))]) 
+          THEN ASSUM_LIST (fn ths => REWRITE_TAC
+               [REWRITE_RULE[FDOM_FUPDATE,el 1 ths] (Q.SPEC`x'` (el 5 ths))])],
+     ASSUM_LIST (fn ths => ASSUME_TAC (CONV_RULE (DEPTH_CONV FUN_EQ_CONV)
+            (SYM (CONJUNCT2 (MATCH_MP fmap_EQ_1 (CONJUNCT1 (el 4 ths))))))) 
+       THEN GEN_TAC 
+       THEN Q.ASM_CASES_TAC `x' = x` THENL
+       [IMP_RES_TAC NOT_FDOM_FAPPLY_FEMPTY 
+          THEN ASM_REWRITE_TAC [] 
+          THEN ONCE_REWRITE_TAC [EQ_SYM_EQ] 
+          THEN MATCH_MP_TAC NOT_FDOM_FAPPLY_FEMPTY 
+          THEN ASM_REWRITE_TAC [],
+        IMP_RES_TAC NOT_EQ_FAPPLY 
+          THEN POP_ASSUM (fn th => 
+                ASSUME_TAC (ONCE_REWRITE_RULE [EQ_SYM_EQ] (Q.SPEC `y` th)))
+          THEN POP_ASSUM (fn th => ONCE_REWRITE_TAC [th]) 
+          THEN ASM_REWRITE_TAC [] 
+          THEN ASSUM_LIST (fn ths => REWRITE_TAC [
+                   ONCE_REWRITE_RULE[FAPPLY_FUPDATE] (Q.SPEC `x` (el 4 ths))])
+          THEN ONCE_ASM_REWRITE_TAC [] 
+          THEN IMP_RES_TAC NOT_EQ_FAPPLY 
+          THEN POP_ASSUM (fn th => ONCE_REWRITE_TAC [th]) 
+          THEN REWRITE_TAC []]]]);
 
+val fmap_EQ = Q.store_thm
+("fmap_EQ",
+ `!(f:'a |-> 'b) g. (FDOM f = FDOM g) /\ (FAPPLY f = FAPPLY g) = (f = g)`,
+ REPEAT STRIP_TAC THEN EQ_TAC THEN REWRITE_TAC [fmap_EQ_1, fmap_EQ_2]);
 
-val fmap_EQ_2 = prove (
-Term`!(f:('a,'b) fmap) g.
-    (FDOM f = FDOM g) /\ (FAPPLY f = FAPPLY g) ==> (f = g)`,
-INDUCT_THEN fmap_INDUCT ASSUME_TAC THENL
-[
- GEN_TAC THEN
- CONV_TAC (DEPTH_CONV FUN_EQ_CONV) THEN
- PURE_REWRITE_TAC [FDOM_FEMPTY] THEN
- PURE_ONCE_REWRITE_TAC [EQ_SYM_EQ, FDOM_F_FEMPTY] THEN
- REWRITE_TAC [FDOM_F_FEMPTY] THEN
- STRIP_TAC THEN ASM_REWRITE_TAC [],
+(*---------------------------------------------------------------------------
+       A more useful equality
+ ---------------------------------------------------------------------------*)
 
-  REPEAT GEN_TAC THEN STRIP_TAC THEN GEN_TAC THEN
-   STRIP_ASSUME_TAC (SPECL [Term`g:('a,'b)fmap`,Term`x:'a`] update_eq_not_x) THEN
-   POP_ASSUM (ASSUME_TAC o (SPEC (Term`FAPPLY (g:('a,'b)fmap) x`))) THEN
-   CONV_TAC (DEPTH_CONV FUN_EQ_CONV) THEN
-   STRIP_TAC THEN
-   ASSUM_LIST (fn ths => ASSUME_TAC
-        (REWRITE_RULE [FDOM_FUPDATE] (SPEC (Term`x:'a`) (el 2 ths)))) THEN
-   ASSUM_LIST (fn ths => ONCE_REWRITE_TAC [SYM
-        (REWRITE_RULE [el 1 ths]
-           (SPECL [Term`g:('a,'b)fmap`,Term`x:'a`,
-                  Term`FAPPLY (g:('a,'b)fmap) x`]
-                               FUPDATE_ABSORB_THM))]) THEN
-   ASM_REWRITE_TAC [] THEN
-   ASSUM_LIST (fn ths => REWRITE_TAC [
-                   ONCE_REWRITE_RULE [EQ_SYM_EQ] (el 2 ths)]) THEN
-   REWRITE_TAC [FAPPLY_FUPDATE] THEN
-   MATCH_MP_TAC lemma9 THEN
-   FIRST_ASSUM MATCH_MP_TAC THEN
-  CONV_TAC (DEPTH_CONV FUN_EQ_CONV) THEN
-  CONJ_TAC THENL
-  [
-    ASSUM_LIST (fn ths => ASSUME_TAC
-     (CONV_RULE (DEPTH_CONV FUN_EQ_CONV)
-      (SYM (CONJUNCT1 (MATCH_MP fmap_EQ_1 (CONJUNCT1 (el 4 ths))))))) THEN
-    GEN_TAC THEN
-    ASM_CASES_TAC (Term`(x':'a) = x`) THENL
-    [ASM_REWRITE_TAC [],
-     ASSUM_LIST (fn ths => REWRITE_TAC
-          [REWRITE_RULE [FDOM_FUPDATE, el 1 ths ]
-                         (SPEC (Term`x':'a`) (el 2 ths))]) THEN
-     ASSUM_LIST (fn ths => REWRITE_TAC
-          [REWRITE_RULE [FDOM_FUPDATE, el 1 ths ]
-                         (SPEC (Term`x':'a`) (el 5 ths))])
-    ] ,
-
-    ASSUM_LIST (fn ths => ASSUME_TAC
-     (CONV_RULE (DEPTH_CONV FUN_EQ_CONV)
-      (SYM (CONJUNCT2 (MATCH_MP fmap_EQ_1 (CONJUNCT1 (el 4 ths))))))) THEN
-    GEN_TAC THEN
-    ASM_CASES_TAC (Term`(x':'a) = x`) THENL
-    [IMP_RES_TAC NOT_FDOM_FAPPLY_FEMPTY THEN
-     ASM_REWRITE_TAC [] THEN
-     ONCE_REWRITE_TAC [EQ_SYM_EQ] THEN
-     MATCH_MP_TAC NOT_FDOM_FAPPLY_FEMPTY THEN
-     ASM_REWRITE_TAC [],
-     IMP_RES_TAC NOT_EQ_FAPPLY THEN
-     POP_ASSUM (fn th => ASSUME_TAC (ONCE_REWRITE_RULE [EQ_SYM_EQ]
-                           (SPEC (Term`y:'b`) th))) THEN
-     POP_ASSUM (fn th => ONCE_REWRITE_TAC [th]) THEN
-     ASM_REWRITE_TAC [] THEN
-     ASSUM_LIST (fn ths => REWRITE_TAC [
-                   ONCE_REWRITE_RULE [FAPPLY_FUPDATE]
-                    (SPEC (Term`x:'a`) (el 4 ths))]) THEN
-     ONCE_ASM_REWRITE_TAC [] THEN
-     IMP_RES_TAC  NOT_EQ_FAPPLY THEN
-     POP_ASSUM (fn th => ONCE_REWRITE_TAC [th]) THEN
-     REWRITE_TAC []
-    ]
-  ]
- ]
-);
-
-val fmap_EQ = store_thm("fmap_EQ",
-Term`!(f:('a,'b) fmap) g.
-    (FDOM f = FDOM g) /\ (FAPPLY f = FAPPLY g) = (f = g)`,
-REPEAT STRIP_TAC THEN EQ_TAC THEN REWRITE_TAC [fmap_EQ_1, fmap_EQ_2]);
-
-(*and now a more useful equality*)
-val fmap_EQ_THM = store_thm("fmap_EQ_THM",
-Term`!(f:('a,'b) fmap) g.
-    (FDOM f = FDOM g) /\
-    (!x. FDOM f x ==> (FAPPLY f x = FAPPLY g x)) = (f = g)`,
-REPEAT STRIP_TAC THEN EQ_TAC THENL
-[
- STRIP_TAC THEN
- ASM_REWRITE_TAC [ONCE_REWRITE_RULE [EQ_SYM_EQ] fmap_EQ] THEN
- MATCH_MP_TAC EQ_EXT THEN
- GEN_TAC THEN
- ASM_CASES_TAC (Term`FDOM (f:('a,'b) fmap) x`) THENL
- [RES_TAC,
-  ASSUM_LIST (fn ths => ASSUME_TAC (REWRITE_RULE [el 3 ths] (el 1 ths))) THEN
-  IMP_RES_TAC NOT_FDOM_FAPPLY_FEMPTY THEN
-  ASM_REWRITE_TAC []
- ],
- STRIP_TAC THEN ASM_REWRITE_TAC []
-]
-);
+val fmap_EQ_THM = Q.store_thm
+("fmap_EQ_THM",
+ `!(f:'a |-> 'b) g.
+     (FDOM f = FDOM g) /\
+     (!x. FDOM f x ==> (FAPPLY f x = FAPPLY g x)) = (f = g)`,
+ REPEAT STRIP_TAC THEN EQ_TAC THENL
+ [STRIP_TAC 
+    THEN ASM_REWRITE_TAC [ONCE_REWRITE_RULE [EQ_SYM_EQ] fmap_EQ] 
+    THEN MATCH_MP_TAC EQ_EXT 
+    THEN GEN_TAC 
+    THEN Q.ASM_CASES_TAC `FDOM f x` THENL
+    [RES_TAC,
+     ASSUM_LIST (fn ths => ASSUME_TAC (REWRITE_RULE [el 3 ths] (el 1 ths))) 
+        THEN IMP_RES_TAC NOT_FDOM_FAPPLY_FEMPTY 
+        THEN ASM_REWRITE_TAC []],
+  STRIP_TAC THEN ASM_REWRITE_TAC []]);
 
 
+(*---------------------------------------------------------------------------
+           Submaps
+ ---------------------------------------------------------------------------*)
 
-(*Additional theorems and definitions*)
-
-
-
-(* Define a notion of submap *)
-
-val SUBMAP_DEF = new_infixr_definition ("SUBMAP_DEF",
- Term`!(f : ('a,'b) fmap) g. SUBMAP f g =
-              !x. (FDOM f x) ==>
-                 (FDOM g x /\
-                  (FAPPLY f x = FAPPLY g x))`,450);
-
-(*And prove a few theorems to illustrate this*)
-
-val SUBMAP_FEMPTY = store_thm("SUBMAP_FEMPTY",
-Term`!(f : ('a,'b) fmap). FEMPTY SUBMAP f`,
-REWRITE_TAC [SUBMAP_DEF, FDOM_FEMPTY]);
+val SUBMAP_DEF = new_infixr_definition 
+("SUBMAP_DEF",
+ Term`!^fmap g. 
+         SUBMAP f g =
+          !x. FDOM f x ==> FDOM g x /\ (FAPPLY f x = FAPPLY g x)`, 450);
 
 
+val SUBMAP_FEMPTY = Q.store_thm
+("SUBMAP_FEMPTY",
+ `!(f : ('a,'b) fmap). FEMPTY SUBMAP f`,
+ REWRITE_TAC [SUBMAP_DEF, FDOM_FEMPTY]);
 
-val SUBMAP_REFL = store_thm("SUBMAP_REFL",
-Term`!(f : ('a,'b) fmap). f SUBMAP  f`,
-REWRITE_TAC [SUBMAP_DEF]);
+val SUBMAP_REFL = Q.store_thm
+("SUBMAP_REFL",
+ `!(f:('a,'b) fmap). f SUBMAP  f`,
+ REWRITE_TAC [SUBMAP_DEF]);
 
-val SUBMAP_ANTISYM = store_thm("SUBMAP_ANTISYM",
-Term`!(f : ('a,'b) fmap) g.
-     (f SUBMAP g /\ g SUBMAP f) = (f = g)`,
-GEN_TAC THEN GEN_TAC THEN EQ_TAC THENL
-[
- REWRITE_TAC[SUBMAP_DEF, ONCE_REWRITE_RULE [EQ_SYM_EQ] fmap_EQ_THM] THEN
- STRIP_TAC THEN CONJ_TAC THENL
- [
-  MATCH_MP_TAC EQ_EXT THEN
-  GEN_TAC THEN
-  EQ_TAC THEN STRIP_TAC THEN RES_TAC,
-  GEN_TAC THEN STRIP_TAC THEN RES_TAC
- ],
- STRIP_TAC THEN ASM_REWRITE_TAC [SUBMAP_REFL]
-]);
-
-(*Restriction*)
+val SUBMAP_ANTISYM = Q.store_thm
+("SUBMAP_ANTISYM",
+ `!(f:('a,'b) fmap) g. (f SUBMAP g /\ g SUBMAP f) = (f = g)`,
+ GEN_TAC THEN GEN_TAC THEN EQ_TAC THENL
+ [REWRITE_TAC[SUBMAP_DEF, ONCE_REWRITE_RULE [EQ_SYM_EQ] fmap_EQ_THM] 
+    THEN STRIP_TAC THEN CONJ_TAC THENL
+    [MATCH_MP_TAC EQ_EXT 
+       THEN GEN_TAC 
+       THEN EQ_TAC 
+       THEN STRIP_TAC 
+       THEN RES_TAC,
+     GEN_TAC THEN STRIP_TAC THEN RES_TAC],
+  STRIP_TAC THEN ASM_REWRITE_TAC [SUBMAP_REFL]]);
 
 
-val res_lemma = prove (
-Term`!(f : ('a,'b) fmap) (r: 'a -> bool).
-        ?res.
-           (!x.(FDOM res x) = ((FDOM f x) /\ r x)) /\
-           (!x.FAPPLY res x =
-               ((FDOM f x /\ r x) =>
-                   (FAPPLY f x) | (FAPPLY FEMPTY x)))`,
-INDUCT_THEN fmap_INDUCT ASSUME_TAC THENL
-[
- GEN_TAC THEN
- EXISTS_TAC (Term`FEMPTY:('a,'b)fmap`) THEN
- REWRITE_TAC [FDOM_FEMPTY],
- REPEAT STRIP_TAC THEN
- ASSUM_LIST (fn ths =>
-   STRIP_ASSUME_TAC (SPEC (Term`r:'a->bool`) (el 2 ths))) THEN
- ASM_CASES_TAC (Term`(r:'a -> bool) x`) THENL
- [
-  EXISTS_TAC (Term`FUPDATE (res:('a,'b)fmap) (x,y)`) THEN
-  CONJ_TAC THEN GEN_TAC THENL
-  [
-   ASM_CASES_TAC (Term`(x':'a) = x`) THEN  ASM_REWRITE_TAC [FDOM_FUPDATE],
-   ASM_CASES_TAC (Term`(x':'a) = x`) THENL
-   [
-     ASM_REWRITE_TAC [FDOM_FUPDATE, FAPPLY_FUPDATE],
-     IMP_RES_TAC NOT_EQ_FAPPLY THEN
-     ASM_REWRITE_TAC [FDOM_FUPDATE]
-   ]
-  ],
-  EXISTS_TAC (Term`res:('a,'b)fmap`) THEN
-  CONJ_TAC THEN GEN_TAC  THENL
-  [
-   ASM_CASES_TAC (Term`(x':'a) = x`) THEN  ASM_REWRITE_TAC [FDOM_FUPDATE],
-   ASM_CASES_TAC (Term`(x':'a) = x`) THENL
-   [
-     ASM_REWRITE_TAC [FDOM_FUPDATE, FAPPLY_FUPDATE],
-     IMP_RES_TAC NOT_EQ_FAPPLY THEN
-     ASM_REWRITE_TAC [FDOM_FUPDATE]
-   ]
-  ]
- ]
-]);
+(*---------------------------------------------------------------------------
+    Restriction
+ ---------------------------------------------------------------------------*)
 
-val res_exists = CONV_RULE (ONCE_DEPTH_CONV SKOLEM_CONV) res_lemma;
+val res_lemma = Q.prove 
+(`!^fmap (r:'a -> bool).
+     ?res. (!x. FDOM res x = FDOM f x /\ r x)
+       /\  (!x. FAPPLY res x = 
+                 if FDOM f x /\ r x then FAPPLY f x else FAPPLY FEMPTY x)`,
+ INDUCT_THEN fmap_INDUCT ASSUME_TAC THENL
+ [GEN_TAC 
+    THEN Q.EXISTS_TAC `FEMPTY`
+    THEN REWRITE_TAC [FDOM_FEMPTY],
+  REPEAT STRIP_TAC 
+    THEN ASSUM_LIST (fn ths => STRIP_ASSUME_TAC (Q.SPEC `r` (el 2 ths))) 
+    THEN ASM_CASES_TAC (Term`(r:'a -> bool) x`) THENL
+    [Q.EXISTS_TAC `FUPDATE res (x,y)`
+      THEN CONJ_TAC THEN GEN_TAC THENL
+      [Q.ASM_CASES_TAC `x' = x` 
+          THEN ASM_REWRITE_TAC [FDOM_FUPDATE],
+       Q.ASM_CASES_TAC `x' = x` THENL
+       [ASM_REWRITE_TAC [FDOM_FUPDATE, FAPPLY_FUPDATE],
+        IMP_RES_TAC NOT_EQ_FAPPLY 
+           THEN ASM_REWRITE_TAC [FDOM_FUPDATE]]],
+     Q.EXISTS_TAC `res`
+       THEN CONJ_TAC THEN GEN_TAC THENL
+       [Q.ASM_CASES_TAC `x' = x` 
+           THEN ASM_REWRITE_TAC [FDOM_FUPDATE],
+        Q.ASM_CASES_TAC `x' = x` THENL
+        [ASM_REWRITE_TAC [FDOM_FUPDATE, FAPPLY_FUPDATE],
+         IMP_RES_TAC NOT_EQ_FAPPLY THEN ASM_REWRITE_TAC [FDOM_FUPDATE]]]]]);
+
 
 val DRESTRICT_DEF =
-   new_specification {name = "DRESTRICT_DEF",
-                      consts = [{fixity = Prefix,
-                                 const_name = "DRESTRICT"}],
-                      sat_thm = res_exists};
+  new_specification 
+    {name = "DRESTRICT_DEF",
+     consts = [{fixity = Prefix, const_name="DRESTRICT"}],
+     sat_thm = CONV_RULE (ONCE_DEPTH_CONV SKOLEM_CONV) res_lemma};
 
 
-val DRESTRICT_FEMPTY =
-store_thm ("DRESTRICT_FEMPTY",
-Term`!r. DRESTRICT (FEMPTY:('a,'b)fmap) r = FEMPTY`,
-REWRITE_TAC [ONCE_REWRITE_RULE [EQ_SYM_EQ] fmap_EQ] THEN
-CONV_TAC (DEPTH_CONV FUN_EQ_CONV) THEN
-REWRITE_TAC [DRESTRICT_DEF, FDOM_FEMPTY]);
+val DRESTRICT_FEMPTY = Q.store_thm 
+("DRESTRICT_FEMPTY",
+ `!r. DRESTRICT ^FEMPTY r = FEMPTY`,
+ REWRITE_TAC [ONCE_REWRITE_RULE [EQ_SYM_EQ] fmap_EQ] 
+   THEN CONV_TAC (DEPTH_CONV FUN_EQ_CONV) 
+   THEN REWRITE_TAC [DRESTRICT_DEF, FDOM_FEMPTY]);
 
-val DRESTRICT_FUPDATE =
-store_thm("DRESTRICT_FUPDATE",
-Term`!(f:('a,'b)fmap) r x y.
+val DRESTRICT_FUPDATE = Q.store_thm
+("DRESTRICT_FUPDATE",
+ `!^fmap r x y.
      DRESTRICT (FUPDATE f (x,y)) r =
-            (r x => (FUPDATE (DRESTRICT f r) (x,y))
-                                | DRESTRICT f r)`,
-REPEAT STRIP_TAC THEN
-COND_CASES_TAC THEN
-REWRITE_TAC [ONCE_REWRITE_RULE [EQ_SYM_EQ] fmap_EQ] THEN
-CONV_TAC (DEPTH_CONV FUN_EQ_CONV) THEN
-ASM_REWRITE_TAC [FDOM_FUPDATE,DRESTRICT_DEF] THEN
-REPEAT STRIP_TAC THEN
-ASM_CASES_TAC (Term`(x':'a) = x`) THEN
-ASM_REWRITE_TAC [FAPPLY_FUPDATE] THEN
-TRY (IMP_RES_TAC NOT_EQ_FAPPLY) THEN
-ASM_REWRITE_TAC [DRESTRICT_DEF]);
+        if r x then FUPDATE (DRESTRICT f r) (x,y) else DRESTRICT f r`,
+ REPEAT STRIP_TAC 
+   THEN COND_CASES_TAC 
+   THEN REWRITE_TAC [ONCE_REWRITE_RULE [EQ_SYM_EQ] fmap_EQ] 
+   THEN CONV_TAC (DEPTH_CONV FUN_EQ_CONV) 
+   THEN ASM_REWRITE_TAC [FDOM_FUPDATE,DRESTRICT_DEF] 
+   THEN REPEAT STRIP_TAC 
+   THEN Q.ASM_CASES_TAC `x' = x`
+   THEN ASM_REWRITE_TAC [FAPPLY_FUPDATE] 
+   THEN TRY (IMP_RES_TAC NOT_EQ_FAPPLY) 
+   THEN ASM_REWRITE_TAC [DRESTRICT_DEF]);
 
 
-val STRONG_DRESTRICT_FUPDATE =
-store_thm ("STRONG_DRESTRICT_FUPDATE",
-Term`!(f:('a,'b)fmap) r x y.
-  r x ==>
-  (DRESTRICT (FUPDATE f (x,y)) r
-    = FUPDATE (DRESTRICT f (\v. ~(v=x) /\ r v)) (x,y))`,
-REPEAT STRIP_TAC THEN
-REWRITE_TAC [ONCE_REWRITE_RULE [EQ_SYM_EQ] fmap_EQ] THEN
-CONJ_TAC THEN
-MATCH_MP_TAC EQ_EXT THEN GEN_TAC THENL
-[
- ASM_REWRITE_TAC [FDOM_FUPDATE,DRESTRICT_DEF] THEN
- BETA_TAC THEN
- ASM_CASES_TAC (Term`(x':'a) = x`) THEN ASM_REWRITE_TAC [],
- ASM_CASES_TAC (Term`(x':'a) = x`) THENL
- [
-  ASM_REWRITE_TAC [FDOM_FUPDATE,FAPPLY_FUPDATE,DRESTRICT_DEF] THEN
-  BETA_TAC,
-  IMP_RES_TAC NOT_EQ_FAPPLY THEN
-  ASM_REWRITE_TAC [DRESTRICT_FUPDATE, DRESTRICT_DEF] THEN
-  BETA_TAC THEN
-  ASM_REWRITE_TAC [FDOM_FUPDATE]
- ]
-]);
+val STRONG_DRESTRICT_FUPDATE = Q.store_thm 
+("STRONG_DRESTRICT_FUPDATE",
+ `!^fmap r x y.
+      r x ==> (DRESTRICT (FUPDATE f (x,y)) r
+                 = 
+               FUPDATE (DRESTRICT f (\v. ~(v=x) /\ r v)) (x,y))`,
+ REPEAT STRIP_TAC 
+   THEN REWRITE_TAC [ONCE_REWRITE_RULE [EQ_SYM_EQ] fmap_EQ] 
+   THEN CONJ_TAC 
+   THEN MATCH_MP_TAC EQ_EXT 
+   THEN GEN_TAC THENL
+   [ASM_REWRITE_TAC [FDOM_FUPDATE,DRESTRICT_DEF] 
+      THEN BETA_TAC 
+      THEN Q.ASM_CASES_TAC `x' = x`
+      THEN ASM_REWRITE_TAC [],
+    Q.ASM_CASES_TAC `x' = x` THENL
+    [ASM_REWRITE_TAC [FDOM_FUPDATE,FAPPLY_FUPDATE,DRESTRICT_DEF] 
+       THEN BETA_TAC,
+     IMP_RES_TAC NOT_EQ_FAPPLY 
+       THEN ASM_REWRITE_TAC [DRESTRICT_FUPDATE, DRESTRICT_DEF] 
+       THEN BETA_TAC 
+       THEN ASM_REWRITE_TAC [FDOM_FUPDATE]]]);
 
 
-val FDOM_DRESTRICT = store_thm ("FDOM_DRESTRICT",
-Term`!(f:('a,'b)fmap) r x.
-  ~(r x) ==> ~(FDOM (DRESTRICT f r) x)`,
-REPEAT GEN_TAC THEN  STRIP_TAC THEN
-ASM_REWRITE_TAC [DRESTRICT_DEF]);
+val FDOM_DRESTRICT = Q.store_thm 
+("FDOM_DRESTRICT",
+ `!^fmap r x. ~r x ==> ~FDOM (DRESTRICT f r) x`,
+REPEAT GEN_TAC THEN STRIP_TAC THEN ASM_REWRITE_TAC [DRESTRICT_DEF]);
 
-val lemma = prove(Term`!(a:'a) b. (a = b) ==> (b = a)`,
-REPEAT STRIP_TAC THEN ASM_REWRITE_TAC []);
+val lemma = Q.prove
+(`!(a:'a) b. (a = b) ==> (b = a)`,
+ REPEAT STRIP_TAC THEN ASM_REWRITE_TAC []);
 
-val NOT_FDOM_DRESTRICT = store_thm ("NOT_FDOM_DRESTRICT",
-Term`!(f:('a,'b)fmap) x. ~(FDOM f x) ==> (DRESTRICT f (\a. ~(a = x)) = f)`,
-STRIP_TAC THEN
-ASM_REWRITE_TAC [GSYM fmap_EQ] THEN
- CONV_TAC (DEPTH_CONV FUN_EQ_CONV) THEN
-ASM_REWRITE_TAC [DRESTRICT_DEF] THEN
-REPEAT STRIP_TAC THEN
-ASM_CASES_TAC (Term`(x':'a)=x`) THEN
-BETA_TAC THEN
-ASM_REWRITE_TAC  [ NOT_FDOM_FAPPLY_FEMPTY] THEN
-ASM_CASES_TAC (Term`FDOM (f:('a,'b)fmap) x'`) THEN
-ASM_REWRITE_TAC  [] THEN
-MATCH_MP_TAC lemma THEN
-MATCH_MP_TAC  NOT_FDOM_FAPPLY_FEMPTY THEN
-ASM_REWRITE_TAC  [ NOT_FDOM_FAPPLY_FEMPTY]
-);
-
-
-val DRESTRICT_SUBMAP = store_thm("DRESTRICT_SUBMAP",
-Term`!(f:('a,'b)fmap) r.
-       (DRESTRICT f r) SUBMAP f`,
-INDUCT_THEN fmap_INDUCT STRIP_ASSUME_TAC THENL
-[
- REWRITE_TAC [DRESTRICT_FEMPTY, SUBMAP_FEMPTY],
- REPEAT STRIP_TAC THEN
- REWRITE_TAC [DRESTRICT_FUPDATE] THEN
- COND_CASES_TAC THEN
- UNDISCH_TAC (Term`!r. DRESTRICT (f:('a,'b)fmap) r SUBMAP f`) THEN
- REWRITE_TAC [SUBMAP_DEF] THENL
- [
-  STRIP_TAC THEN GEN_TAC THEN
-  ASM_REWRITE_TAC [FDOM_FUPDATE] THEN
-  ASM_CASES_TAC (Term`x':'a = x`) THENL
-  [
-   ASM_REWRITE_TAC [FAPPLY_FUPDATE],
-   ASM_REWRITE_TAC [] THEN
-   IMP_RES_TAC NOT_EQ_FAPPLY THEN
-   ASM_REWRITE_TAC []
-  ],
-   STRIP_TAC THEN GEN_TAC THEN
-  ASM_REWRITE_TAC [FDOM_FUPDATE] THEN
-  ASM_CASES_TAC (Term`x':'a = x`) THENL
-  [
-    POP_ASSUM SUBST_ALL_TAC THEN
-    DISCH_TAC THEN
-    ASM_REWRITE_TAC [] THEN
-    RES_TAC THEN
-    RES_TAC,
-    DISCH_TAC THEN
-    ASM_REWRITE_TAC [] THEN
-    IMP_RES_TAC NOT_EQ_FAPPLY THEN
-    RES_TAC THEN
-    ASM_REWRITE_TAC []
-  ]
-]]);
-
-val DRESTRICT_DRESTRICT = store_thm ("DRESTRICT_DRESTRICT",
-Term`!(f:('a,'b)fmap) P Q. DRESTRICT (DRESTRICT f P) Q = DRESTRICT f (\x. P x /\ Q x)`,
-MATCH_MP_TAC (
-BETA_RULE (
-SPEC (Term`\(f:('a,'b)fmap). !P Q. DRESTRICT (DRESTRICT f P) Q = DRESTRICT f (\x. P x /\ Q x)`)
-fmap_INDUCT)) THEN
-REWRITE_TAC [DRESTRICT_FEMPTY, DRESTRICT_FUPDATE] THEN
-REPEAT STRIP_TAC THEN
-ASM_CASES_TAC (Term`(P:'a-> bool) x`) THEN
-ASM_CASES_TAC (Term`(Q:'a-> bool) x`) THEN
-BETA_TAC THEN
-ASM_REWRITE_TAC [DRESTRICT_FUPDATE]);
-
-val DRESTRICT_IS_FEMPTY = store_thm ("DRESTRICT_IS_FEMPTY",
-Term`!r. (!x. ~(r x)) ==> !(f:('a,'b)fmap). DRESTRICT  f  r = FEMPTY`,
-GEN_TAC THEN DISCH_TAC THEN
-MATCH_MP_TAC (
-BETA_RULE (
-SPEC (Term`\(f:('a,'b)fmap). DRESTRICT  f  r = FEMPTY`)
-fmap_INDUCT)) THEN
-ASM_REWRITE_TAC  [DRESTRICT_FEMPTY, DRESTRICT_FUPDATE] THEN
-REPEAT STRIP_TAC THEN ASM_REWRITE_TAC []);
-
-val FUPDATE_DRESTRICT = store_thm("FUPDATE_DRESTRICT",
-Term`!(f:('a,'b)fmap) x y. FUPDATE f (x,y) = FUPDATE (DRESTRICT f (\v. ~(v = x))) (x,y)`,
-REPEAT STRIP_TAC THEN
-REWRITE_TAC [ONCE_REWRITE_RULE [EQ_SYM_EQ] fmap_EQ] THEN
-CONJ_TAC THEN
-MATCH_MP_TAC EQ_EXT THEN GEN_TAC THENL
-[
- ASM_REWRITE_TAC [FDOM_FUPDATE,DRESTRICT_DEF] THEN
- BETA_TAC THEN
- ASM_CASES_TAC (Term`(x':'a) = x`) THEN ASM_REWRITE_TAC [],
- ASM_CASES_TAC (Term`(x':'a) = x`) THENL
- [
-  ASM_REWRITE_TAC [FDOM_FUPDATE,FAPPLY_FUPDATE,DRESTRICT_DEF] THEN
-  BETA_TAC,
-  IMP_RES_TAC NOT_EQ_FAPPLY THEN
-  ASM_REWRITE_TAC [DRESTRICT_FUPDATE, DRESTRICT_DEF] THEN
-  BETA_TAC THEN
-  ASM_REWRITE_TAC [FDOM_FUPDATE] THEN
-  ASM_CASES_TAC (Term`FDOM (f:('a,'b)fmap) x'`) THEN
-  ASM_REWRITE_TAC [] THEN
-  MATCH_MP_TAC NOT_FDOM_FAPPLY_FEMPTY THEN
-  ASM_REWRITE_TAC []
- ]
-]);
-
-val lemma = prove(Term`(\x':'a. (~(x' = x) /\ r x') /\ ~(x' = x)) =
-                     (\x'. ~(x' = x) /\ r x')`,
-CONV_TAC FUN_EQ_CONV THEN
-BETA_TAC THEN GEN_TAC THEN EQ_TAC THEN REPEAT STRIP_TAC THEN
-ASM_REWRITE_TAC [] THEN
-RES_TAC);
+val NOT_FDOM_DRESTRICT = Q.store_thm
+("NOT_FDOM_DRESTRICT",
+ `!^fmap x. ~(FDOM f x) ==> (DRESTRICT f (\a. ~(a = x)) = f)`,
+ STRIP_TAC 
+  THEN ASM_REWRITE_TAC [GSYM fmap_EQ] 
+  THEN CONV_TAC (DEPTH_CONV FUN_EQ_CONV) 
+  THEN ASM_REWRITE_TAC [DRESTRICT_DEF] 
+  THEN REPEAT STRIP_TAC 
+  THEN Q.ASM_CASES_TAC `x' = x` 
+  THEN BETA_TAC 
+  THEN ASM_REWRITE_TAC [NOT_FDOM_FAPPLY_FEMPTY] 
+  THEN Q.ASM_CASES_TAC `FDOM f x'`
+  THEN ASM_REWRITE_TAC []
+  THEN MATCH_MP_TAC lemma 
+  THEN MATCH_MP_TAC NOT_FDOM_FAPPLY_FEMPTY 
+  THEN ASM_REWRITE_TAC [NOT_FDOM_FAPPLY_FEMPTY]);
 
 
-val STRONG_DRESTRICT_FUPDATE_THM =
-store_thm ("STRONG_DRESTRICT_FUPDATE_THM",
-Term`!(f:('a,'b)fmap) r x y.
-  (DRESTRICT (FUPDATE f (x,y)) r
-    = (r x => FUPDATE (DRESTRICT f (\v. ~(v=x) /\ r v)) (x,y) |
-              (DRESTRICT f (\v. ~(v=x) /\ r v)) ))`,
-REPEAT STRIP_TAC THEN
-ASM_CASES_TAC (Term`(r:'a -> bool) x`) THEN
-ASM_REWRITE_TAC  [STRONG_DRESTRICT_FUPDATE] THEN
-ONCE_REWRITE_TAC [FUPDATE_DRESTRICT] THEN
-ASM_REWRITE_TAC  [DRESTRICT_FUPDATE, DRESTRICT_DRESTRICT] THEN
-BETA_TAC THEN ASM_REWRITE_TAC  [lemma]);
+val DRESTRICT_SUBMAP = Q.store_thm
+("DRESTRICT_SUBMAP",
+ `!^fmap r. (DRESTRICT f r) SUBMAP f`,
+ INDUCT_THEN fmap_INDUCT STRIP_ASSUME_TAC THENL
+ [REWRITE_TAC [DRESTRICT_FEMPTY, SUBMAP_FEMPTY],
+  REPEAT STRIP_TAC 
+    THEN REWRITE_TAC [DRESTRICT_FUPDATE] 
+    THEN COND_CASES_TAC 
+    THEN Q.UNDISCH_TAC `!r. (DRESTRICT f r) SUBMAP f`
+    THEN REWRITE_TAC [SUBMAP_DEF] THENL
+    [STRIP_TAC THEN GEN_TAC 
+       THEN ASM_REWRITE_TAC [FDOM_FUPDATE] 
+       THEN Q.ASM_CASES_TAC `x' = x` THENL
+       [ASM_REWRITE_TAC [FAPPLY_FUPDATE],
+        ASM_REWRITE_TAC [] 
+          THEN IMP_RES_TAC NOT_EQ_FAPPLY 
+          THEN ASM_REWRITE_TAC []],
+     STRIP_TAC THEN GEN_TAC 
+        THEN ASM_REWRITE_TAC [FDOM_FUPDATE] 
+        THEN Q.ASM_CASES_TAC `x' = x` THENL
+        [POP_ASSUM SUBST_ALL_TAC 
+           THEN DISCH_TAC 
+           THEN ASM_REWRITE_TAC [] 
+           THEN RES_TAC 
+           THEN RES_TAC,
+         DISCH_TAC 
+           THEN ASM_REWRITE_TAC [] 
+           THEN IMP_RES_TAC NOT_EQ_FAPPLY 
+           THEN RES_TAC 
+           THEN ASM_REWRITE_TAC []]]]);
+
+val DRESTRICT_DRESTRICT = Q.store_thm 
+("DRESTRICT_DRESTRICT",
+ `!^fmap P Q. DRESTRICT (DRESTRICT f P) Q = DRESTRICT f (\x. P x /\ Q x)`,
+ HO_MATCH_MP_TAC fmap_INDUCT
+   THEN REWRITE_TAC [DRESTRICT_FEMPTY, DRESTRICT_FUPDATE] 
+   THEN REPEAT STRIP_TAC 
+   THEN Q.ASM_CASES_TAC `P x`
+   THEN ASM_CASES_TAC (Term`(Q:'a-> bool) x`) 
+   THEN BETA_TAC 
+   THEN ASM_REWRITE_TAC [DRESTRICT_FUPDATE]);
+
+val DRESTRICT_IS_FEMPTY = Q.store_thm 
+("DRESTRICT_IS_FEMPTY",
+ `!r. (!x. ~r x) ==> !^fmap. DRESTRICT f r = FEMPTY`,
+ GEN_TAC THEN DISCH_TAC 
+   THEN HO_MATCH_MP_TAC fmap_INDUCT
+   THEN ASM_REWRITE_TAC  [DRESTRICT_FEMPTY, DRESTRICT_FUPDATE] 
+   THEN REPEAT STRIP_TAC THEN ASM_REWRITE_TAC []);
+
+val FUPDATE_DRESTRICT = Q.store_thm
+("FUPDATE_DRESTRICT",
+ `!^fmap x y. FUPDATE f (x,y) = FUPDATE (DRESTRICT f (\v. ~(v = x))) (x,y)`,
+ REPEAT STRIP_TAC 
+    THEN REWRITE_TAC [ONCE_REWRITE_RULE [EQ_SYM_EQ] fmap_EQ] 
+    THEN CONJ_TAC 
+    THEN MATCH_MP_TAC EQ_EXT 
+    THEN GEN_TAC THENL
+    [ASM_REWRITE_TAC [FDOM_FUPDATE,DRESTRICT_DEF] 
+       THEN BETA_TAC 
+       THEN Q.ASM_CASES_TAC `x' = x`
+       THEN ASM_REWRITE_TAC [],
+     Q.ASM_CASES_TAC `x' = x` THENL
+     [ASM_REWRITE_TAC [FDOM_FUPDATE,FAPPLY_FUPDATE,DRESTRICT_DEF] 
+        THEN BETA_TAC,
+      IMP_RES_TAC NOT_EQ_FAPPLY 
+        THEN ASM_REWRITE_TAC [DRESTRICT_FUPDATE, DRESTRICT_DEF] 
+        THEN BETA_TAC 
+        THEN ASM_REWRITE_TAC [FDOM_FUPDATE] 
+        THEN Q.ASM_CASES_TAC `FDOM f x'`
+        THEN ASM_REWRITE_TAC [] 
+        THEN MATCH_MP_TAC NOT_FDOM_FAPPLY_FEMPTY 
+        THEN ASM_REWRITE_TAC []]]);
+
+val lemma = Q.prove
+(`(\x':'a. (~(x' = x) /\ r x') /\ ~(x' = x)) = (\x'. ~(x' = x) /\ r x')`,
+ CONV_TAC FUN_EQ_CONV 
+   THEN BETA_TAC 
+   THEN GEN_TAC 
+   THEN EQ_TAC 
+   THEN REPEAT STRIP_TAC 
+   THEN ASM_REWRITE_TAC [] 
+   THEN RES_TAC);
 
 
+val STRONG_DRESTRICT_FUPDATE_THM = Q.store_thm 
+("STRONG_DRESTRICT_FUPDATE_THM",
+ `!^fmap r x y.
+  DRESTRICT (FUPDATE f (x,y)) r
+     = 
+  if r x then FUPDATE (DRESTRICT f (\v. ~(v=x) /\ r v)) (x,y)
+         else DRESTRICT f (\v. ~(v=x) /\ r v)`,
+ REPEAT STRIP_TAC 
+   THEN Q.ASM_CASES_TAC `r x` 
+   THEN ASM_REWRITE_TAC [STRONG_DRESTRICT_FUPDATE] 
+   THEN ONCE_REWRITE_TAC [FUPDATE_DRESTRICT] 
+   THEN ASM_REWRITE_TAC [DRESTRICT_FUPDATE, DRESTRICT_DRESTRICT] 
+   THEN BETA_TAC 
+   THEN ASM_REWRITE_TAC [lemma]);
 
 
-(*----------------------------------------*)
+(*---------------------------------------------------------------------------
+     Union of finite maps
+ ---------------------------------------------------------------------------*)
 
+val union_lemma = Q.prove 
+(`!^fmap g.
+     ?union.
+       (!x. FDOM union x = FDOM f x \/ FDOM g x) /\
+       (!x. FAPPLY union x = if FDOM f x then FAPPLY f x else FAPPLY g x)`,
+ INDUCT_THEN fmap_INDUCT ASSUME_TAC THENL
+ [GEN_TAC 
+    THEN Q.EXISTS_TAC `g`
+    THEN REWRITE_TAC [FDOM_FEMPTY],
+  REPEAT STRIP_TAC 
+    THEN ASSUM_LIST (fn ths => STRIP_ASSUME_TAC (Q.SPEC `g` (el 2 ths))) 
+    THEN Q.EXISTS_TAC `FUPDATE union (x,y)`
+    THEN ASM_REWRITE_TAC[FDOM_FUPDATE] 
+    THEN CONJ_TAC THEN GEN_TAC THENL
+    [Q.ASM_CASES_TAC `x' = x` THEN ASM_REWRITE_TAC[],
+     Q.ASM_CASES_TAC `x' = x` THENL
+     [ASM_REWRITE_TAC [FAPPLY_FUPDATE],
+      IMP_RES_TAC NOT_EQ_FAPPLY 
+         THEN ASM_REWRITE_TAC []]]]);
 
-val union_lemma = prove (
-Term`!(f : ('a,'b) fmap) g.
-        ?union.
-           (!x.(FDOM union x) = ((FDOM f x) \/ (FDOM g x))) /\
-           (!x.FAPPLY union x =
-               ((FDOM f x) =>
-                   (FAPPLY f x) | (FAPPLY g x)))`,
-INDUCT_THEN fmap_INDUCT ASSUME_TAC THENL
-[GEN_TAC THEN
- EXISTS_TAC (Term`g:('a,'b)fmap`) THEN
- REWRITE_TAC [FDOM_FEMPTY]
-,
- REPEAT STRIP_TAC THEN
- ASSUM_LIST (fn ths =>
-   STRIP_ASSUME_TAC (SPEC (Term`g:('a,'b)fmap`) (el 2 ths))) THEN
- EXISTS_TAC (Term`FUPDATE (union:('a,'b)fmap) (x,y)`) THEN
- ASM_REWRITE_TAC[FDOM_FUPDATE] THEN
- CONJ_TAC THEN GEN_TAC THENL
- [ASM_CASES_TAC (Term`(x':'a) = x`) THEN ASM_REWRITE_TAC[],
-  ASM_CASES_TAC (Term`(x':'a) = x`) THENL
-  [ASM_REWRITE_TAC [FAPPLY_FUPDATE],
-   IMP_RES_TAC NOT_EQ_FAPPLY THEN
-   ASM_REWRITE_TAC []
-  ]
- ]
-]);
-
-
-val union_exists = CONV_RULE (ONCE_DEPTH_CONV SKOLEM_CONV) union_lemma;
 
 val FUNION_DEF =
-   new_specification {name = "FUNION_DEF",
-                      consts = [{fixity = Prefix,
-                                 const_name = "FUNION"}],
-                      sat_thm = union_exists};
+  new_specification 
+     {name = "FUNION_DEF",
+      consts = [{fixity = Prefix, const_name = "FUNION"}],
+      sat_thm = CONV_RULE (ONCE_DEPTH_CONV SKOLEM_CONV) union_lemma}
 
 
-val FUNION_FEMPTY_1 =
-store_thm ("FUNION_FEMPTY_1",
-Term`!g. FUNION (FEMPTY:('a,'b)fmap) g = g`,
-REWRITE_TAC [ONCE_REWRITE_RULE [EQ_SYM_EQ] fmap_EQ] THEN
-CONV_TAC (DEPTH_CONV FUN_EQ_CONV) THEN
-REWRITE_TAC [FUNION_DEF, FDOM_FEMPTY]);
+val FUNION_FEMPTY_1 = Q.store_thm
+("FUNION_FEMPTY_1",
+ `!g. FUNION ^FEMPTY g = g`,
+ REWRITE_TAC [ONCE_REWRITE_RULE [EQ_SYM_EQ] fmap_EQ] 
+    THEN CONV_TAC (DEPTH_CONV FUN_EQ_CONV) 
+    THEN REWRITE_TAC [FUNION_DEF, FDOM_FEMPTY]);
 
-val FUNION_FEMPTY_2 =
-store_thm ("FUNION_FEMPTY_2",
-Term`!f. FUNION f (FEMPTY:('a,'b)fmap)  = f`,
- REPEAT STRIP_TAC THEN
- REWRITE_TAC [ONCE_REWRITE_RULE [EQ_SYM_EQ] fmap_EQ] THEN
- CONV_TAC (DEPTH_CONV FUN_EQ_CONV) THEN
- REWRITE_TAC [FUNION_DEF, FDOM_FEMPTY] THEN
- STRIP_TAC THEN
- COND_CASES_TAC THENL
- [REWRITE_TAC[],
-  IMP_RES_TAC NOT_FDOM_FAPPLY_FEMPTY THEN
-  ASM_REWRITE_TAC []
- ]
-);
+val FUNION_FEMPTY_2 = Q.store_thm 
+("FUNION_FEMPTY_2",
+ `!f. FUNION f ^FEMPTY = f`,
+ REPEAT STRIP_TAC 
+   THEN REWRITE_TAC [ONCE_REWRITE_RULE [EQ_SYM_EQ] fmap_EQ] 
+   THEN CONV_TAC (DEPTH_CONV FUN_EQ_CONV) 
+   THEN REWRITE_TAC [FUNION_DEF, FDOM_FEMPTY] 
+   THEN STRIP_TAC 
+   THEN COND_CASES_TAC THENL
+   [REWRITE_TAC[],
+    IMP_RES_TAC NOT_FDOM_FAPPLY_FEMPTY THEN ASM_REWRITE_TAC []]);
 
-val FUNION_FUPDATE_1 =
-store_thm ("FUNION_FUPDATE_1",
-Term`!(f:('a,'b)fmap) g x y.
-     FUNION (FUPDATE f (x,y)) g =
-        FUPDATE (FUNION f g) (x,y)`,
- REPEAT STRIP_TAC THEN
- REWRITE_TAC [ONCE_REWRITE_RULE [EQ_SYM_EQ] fmap_EQ] THEN
- CONV_TAC (DEPTH_CONV FUN_EQ_CONV) THEN
- REPEAT STRIP_TAC THENL
- [
-   REWRITE_TAC [FUNION_DEF, FDOM_FUPDATE] THEN
-   ASM_CASES_TAC (Term`(x':'a) = x`) THEN ASM_REWRITE_TAC[],
-   ASM_CASES_TAC (Term`(x':'a) = x`) THENL
-   [ASM_REWRITE_TAC [FUNION_DEF, FAPPLY_FUPDATE, FDOM_FUPDATE],
-    IMP_RES_TAC NOT_EQ_FAPPLY THEN
-    ASM_REWRITE_TAC [FUNION_DEF, FDOM_FUPDATE]
-   ]
- ]);
+val FUNION_FUPDATE_1 = Q.store_thm 
+("FUNION_FUPDATE_1",
+ `!^fmap g x y.
+     FUNION (FUPDATE f (x,y)) g = FUPDATE (FUNION f g) (x,y)`,
+ REPEAT STRIP_TAC 
+   THEN REWRITE_TAC [ONCE_REWRITE_RULE [EQ_SYM_EQ] fmap_EQ] 
+   THEN CONV_TAC (DEPTH_CONV FUN_EQ_CONV) 
+   THEN REPEAT STRIP_TAC THENL
+   [REWRITE_TAC [FUNION_DEF, FDOM_FUPDATE] 
+      THEN Q.ASM_CASES_TAC `x' = x` 
+      THEN ASM_REWRITE_TAC[],
+    Q.ASM_CASES_TAC `x' = x` THENL
+    [ASM_REWRITE_TAC [FUNION_DEF, FAPPLY_FUPDATE, FDOM_FUPDATE],
+     IMP_RES_TAC NOT_EQ_FAPPLY 
+       THEN ASM_REWRITE_TAC [FUNION_DEF, FDOM_FUPDATE]]]);
 
-val FUNION_FUPDATE_2 =
-store_thm ("FUNION_FUPDATE_2",
-Term`!(f:('a,'b)fmap) g x y.
-     FUNION f (FUPDATE g (x,y)) =
-        (FDOM f x => FUNION f g
-                       | FUPDATE (FUNION f g) (x,y))`,
- REPEAT STRIP_TAC THEN
- COND_CASES_TAC THEN
- REWRITE_TAC [ONCE_REWRITE_RULE [EQ_SYM_EQ] fmap_EQ] THEN
- CONV_TAC (DEPTH_CONV FUN_EQ_CONV) THEN
- REPEAT STRIP_TAC THENL
- [
-   REWRITE_TAC [FUNION_DEF, FDOM_FUPDATE] THEN
-   ASM_CASES_TAC (Term`(x':'a) = x`) THEN ASM_REWRITE_TAC[],
-   ASM_CASES_TAC (Term`(x':'a) = x`) THENL
-   [ASM_REWRITE_TAC [FUNION_DEF, FAPPLY_FUPDATE, FDOM_FUPDATE],
-    IMP_RES_TAC NOT_EQ_FAPPLY THEN
-    ASM_REWRITE_TAC [FUNION_DEF, FDOM_FUPDATE]
-   ],
-   REWRITE_TAC [FUNION_DEF, FDOM_FUPDATE] THEN
-   ASM_CASES_TAC (Term`(x':'a) = x`) THEN ASM_REWRITE_TAC[],
-   ASM_CASES_TAC (Term`(x':'a) = x`) THENL
-   [ASM_REWRITE_TAC [FUNION_DEF, FAPPLY_FUPDATE, FDOM_FUPDATE],
-    IMP_RES_TAC NOT_EQ_FAPPLY THEN
-    ASM_REWRITE_TAC [FUNION_DEF, FDOM_FUPDATE]
-   ]
- ]);
+val FUNION_FUPDATE_2 = Q.store_thm 
+("FUNION_FUPDATE_2",
+ `!^fmap g x y.
+     FUNION f (FUPDATE g (x,y)) = 
+        if FDOM f x then FUNION f g 
+                    else FUPDATE (FUNION f g) (x,y)`,
+ REPEAT STRIP_TAC 
+   THEN COND_CASES_TAC 
+   THEN REWRITE_TAC [ONCE_REWRITE_RULE [EQ_SYM_EQ] fmap_EQ] 
+   THEN CONV_TAC (DEPTH_CONV FUN_EQ_CONV) 
+   THEN REPEAT STRIP_TAC THENL
+   [REWRITE_TAC [FUNION_DEF, FDOM_FUPDATE] 
+      THEN Q.ASM_CASES_TAC `x' = x`
+      THEN ASM_REWRITE_TAC[],
+    Q.ASM_CASES_TAC `x' = x` THENL
+    [ASM_REWRITE_TAC [FUNION_DEF, FAPPLY_FUPDATE, FDOM_FUPDATE],
+     IMP_RES_TAC NOT_EQ_FAPPLY 
+       THEN ASM_REWRITE_TAC [FUNION_DEF, FDOM_FUPDATE]],
+    REWRITE_TAC [FUNION_DEF, FDOM_FUPDATE] 
+      THEN Q.ASM_CASES_TAC `x' = x` THEN ASM_REWRITE_TAC[],
+    Q.ASM_CASES_TAC `x' = x` THENL
+    [ASM_REWRITE_TAC [FUNION_DEF, FAPPLY_FUPDATE, FDOM_FUPDATE],
+     IMP_RES_TAC NOT_EQ_FAPPLY 
+        THEN ASM_REWRITE_TAC [FUNION_DEF, FDOM_FUPDATE]]]);
 
-val FDOM_FUNION = store_thm ("FDOM_FUNION",
-Term`!(f:('a,'b)fmap) g x.
-  FDOM (FUNION f g) x = (FDOM f x) \/ (FDOM g x)`,
-REPEAT STRIP_TAC THEN
-REWRITE_TAC [FUNION_DEF]);
+val FDOM_FUNION = Q.store_thm
+("FDOM_FUNION",
+ `!^fmap g x. FDOM (FUNION f g) x = FDOM f x \/ FDOM g x`,
+ REPEAT STRIP_TAC THEN REWRITE_TAC [FUNION_DEF]);
 
 
-val DRESTRICT_FUNION = store_thm ("DRESTRICT_FUNION",
-Term`!(f:('a,'b)fmap) r q.
-  DRESTRICT f (\x. (r x) \/ (q x)) =
-     FUNION (DRESTRICT f r) (DRESTRICT f q)`,
-REPEAT GEN_TAC THEN
- REWRITE_TAC [ONCE_REWRITE_RULE [EQ_SYM_EQ] fmap_EQ] THEN
- CONV_TAC (DEPTH_CONV FUN_EQ_CONV) THEN
- REWRITE_TAC [DRESTRICT_DEF,FUNION_DEF] THEN
- BETA_TAC THEN REWRITE_TAC [LEFT_AND_OVER_OR ] THEN
- GEN_TAC THEN
- ASM_CASES_TAC (Term`FDOM (f:('a,'b)fmap) x`) THEN
- ASM_REWRITE_TAC [] THEN
- ASM_CASES_TAC (Term`(r:'a->bool)x`) THEN
- ASM_REWRITE_TAC []);
-
-val DRESTRICT_TRUE = store_thm ("DRESTRICT_TRUE",
-Term`!(f:('a,'b)fmap). DRESTRICT f (\x.T) = f`,
-GEN_TAC THEN
-REWRITE_TAC [ONCE_REWRITE_RULE [EQ_SYM_EQ] fmap_EQ] THEN
- CONV_TAC (DEPTH_CONV FUN_EQ_CONV) THEN
-REWRITE_TAC [DRESTRICT_DEF] THEN
-GEN_TAC THEN COND_CASES_TAC THENL
-[REWRITE_TAC [] ,
- ONCE_REWRITE_TAC [EQ_SYM_EQ] THEN
- MATCH_MP_TAC NOT_FDOM_FAPPLY_FEMPTY THEN
- ASM_REWRITE_TAC []
-]);
+val DRESTRICT_FUNION = Q.store_thm
+("DRESTRICT_FUNION",
+ `!^fmap r q. 
+     DRESTRICT f (\x. r x \/ q x) = FUNION (DRESTRICT f r) (DRESTRICT f q)`,
+ REPEAT GEN_TAC 
+  THEN REWRITE_TAC [ONCE_REWRITE_RULE [EQ_SYM_EQ] fmap_EQ] 
+  THEN CONV_TAC (DEPTH_CONV FUN_EQ_CONV) 
+  THEN REWRITE_TAC [DRESTRICT_DEF,FUNION_DEF] 
+  THEN BETA_TAC 
+  THEN REWRITE_TAC [LEFT_AND_OVER_OR] 
+  THEN GEN_TAC 
+  THEN Q.ASM_CASES_TAC `FDOM f x`
+  THEN ASM_REWRITE_TAC [] 
+  THEN Q.ASM_CASES_TAC `r x`
+  THEN ASM_REWRITE_TAC []);
 
 
+val DRESTRICT_TRUE = Q.store_thm
+("DRESTRICT_TRUE",
+ `!^fmap. DRESTRICT f (\x.T) = f`,
+ GEN_TAC 
+  THEN REWRITE_TAC [ONCE_REWRITE_RULE [EQ_SYM_EQ] fmap_EQ] 
+  THEN CONV_TAC (DEPTH_CONV FUN_EQ_CONV) 
+  THEN REWRITE_TAC [DRESTRICT_DEF] 
+  THEN GEN_TAC THEN COND_CASES_TAC THENL
+  [REWRITE_TAC [] ,
+   ONCE_REWRITE_TAC [EQ_SYM_EQ] 
+     THEN MATCH_MP_TAC NOT_FDOM_FAPPLY_FEMPTY 
+     THEN ASM_REWRITE_TAC []]);
 
 
-val lookup_DEF = new_definition ("lookup_DEF",
-Term`!(f:('a,'b)fmap) x.FLOOKUP f x = (FDOM f x => INL (FAPPLY f x)|
-                                     INR one)`);
+(*---------------------------------------------------------------------------
+    "assoc" for finite maps
+ ---------------------------------------------------------------------------*)
+
+val lookup_DEF = Q.new_definition 
+("lookup_DEF",
+ `FLOOKUP ^fmap x = if FDOM f x then INL (FAPPLY f x)
+                                else INR one`);
 
 
-(* Now lets define every_fmap *)
+(*---------------------------------------------------------------------------
+       Universal quantifier on finite maps
+ ---------------------------------------------------------------------------*)
 
-val FEVERY_DEF =
- new_definition ("FEVERY_DEF",
- Term`FEVERY P (f:('a,'b)fmap) =
-       !x. FDOM f x ==> P (x,(FAPPLY f x))`);
+val FEVERY_DEF = Q.new_definition 
+("FEVERY_DEF",
+ `FEVERY P ^fmap = !x. FDOM f x ==> P (x, FAPPLY f x)`);
 
-val FEVERY_FEMPTY = prove (
-Term`!(P:('a # 'b)-> bool) . FEVERY P FEMPTY`,
-STRIP_TAC THEN
-REWRITE_TAC [FEVERY_DEF, FDOM_FEMPTY]);
+val FEVERY_FEMPTY = Q.prove 
+(`!P:'a#'b -> bool. FEVERY P FEMPTY`,
+ STRIP_TAC 
+   THEN REWRITE_TAC [FEVERY_DEF, FDOM_FEMPTY]);
 
-val FEVERY_FUPDATE = prove (
-Term`!P (f:('a,'b)fmap) x y.
-     FEVERY P (FUPDATE f (x,y)) =
-        P (x,y) /\ FEVERY P (DRESTRICT f (\v. ~(x = v)))`,
-REPEAT GEN_TAC THEN
-REWRITE_TAC [FEVERY_DEF, FDOM_FUPDATE] THEN
-EQ_TAC THEN REPEAT STRIP_TAC THENL
-[
- POP_ASSUM (fn th =>
-     REWRITE_TAC [(REWRITE_RULE [FAPPLY_FUPDATE] (SPEC (Term`x:'a`) th))])
- ,
- REWRITE_TAC [DRESTRICT_DEF] THEN
- POP_ASSUM (fn th => STRIP_ASSUME_TAC (BETA_RULE
-                 (REWRITE_RULE [DRESTRICT_DEF] th))) THEN
- BETA_TAC THEN
- ASM_REWRITE_TAC [] THEN
- POP_ASSUM (ASSUME_TAC o NOT_EQ_SYM) THEN
- IMP_RES_TAC NOT_EQ_FAPPLY THEN
- POP_ASSUM (fn th => ASSUME_TAC (ONCE_REWRITE_RULE [EQ_SYM_EQ]
-    (SPEC (Term`y:'b`) th))) THEN
- ONCE_ASM_REWRITE_TAC [] THEN
- FIRST_ASSUM MATCH_MP_TAC THEN
- ASM_REWRITE_TAC []
- ,
- ASM_REWRITE_TAC [FAPPLY_FUPDATE]
- ,
- ASSUM_LIST (fn ths => ASSUME_TAC (BETA_RULE (
-          REWRITE_RULE [DRESTRICT_DEF] (SPEC (Term`x':'a`) (el 2 ths)))))
- THEN
- UNDISCH_TAC (Term`FDOM (f:('a,'b)fmap) x' /\ ~(x = x') ==>
-          P
-            (x',
-             ((FDOM f x' /\ ~(x = x'))
-              => (FAPPLY f x')
-              | (FAPPLY FEMPTY x')))`)
- THEN
- ASM_CASES_TAC (Term`(x:'a)=x'`) THEN
- ASM_REWRITE_TAC [FAPPLY_FUPDATE] THENL
- [POP_ASSUM (fn th => REWRITE_TAC [SYM th]) THEN
-  ASM_REWRITE_TAC [],
-  POP_ASSUM (ASSUME_TAC o NOT_EQ_SYM) THEN
-  IMP_RES_TAC NOT_EQ_FAPPLY THEN
-  ASM_REWRITE_TAC []
- ]
-]);
+val FEVERY_FUPDATE = Q.prove
+(`!P ^fmap x y. 
+     FEVERY P (FUPDATE f (x,y)) 
+        =
+     P (x,y) /\ FEVERY P (DRESTRICT f (\v. ~(x = v)))`,
+ REPEAT GEN_TAC 
+   THEN REWRITE_TAC [FEVERY_DEF, FDOM_FUPDATE] 
+   THEN EQ_TAC 
+   THEN REPEAT STRIP_TAC THENL
+   [POP_ASSUM(fn th => REWRITE_TAC
+               [REWRITE_RULE[FAPPLY_FUPDATE](Q.SPEC `x` th)]),
+    REWRITE_TAC [DRESTRICT_DEF] 
+      THEN POP_ASSUM (fn th => STRIP_ASSUME_TAC (BETA_RULE
+                  (REWRITE_RULE [DRESTRICT_DEF] th)))
+      THEN BETA_TAC 
+      THEN ASM_REWRITE_TAC [] 
+      THEN POP_ASSUM (ASSUME_TAC o NOT_EQ_SYM) 
+      THEN IMP_RES_TAC NOT_EQ_FAPPLY 
+      THEN POP_ASSUM (fn th => ASSUME_TAC 
+            (ONCE_REWRITE_RULE [EQ_SYM_EQ] (Q.SPEC `y` th)))
+      THEN ONCE_ASM_REWRITE_TAC [] 
+      THEN FIRST_ASSUM MATCH_MP_TAC 
+      THEN ASM_REWRITE_TAC [],
+    ASM_REWRITE_TAC [FAPPLY_FUPDATE],
+    ASSUM_LIST (fn ths => ASSUME_TAC (BETA_RULE
+           (REWRITE_RULE [DRESTRICT_DEF] (Q.SPEC `x'` (el 2 ths)))))
+      THEN Q.PAT_ASSUM `a ==> b` MP_TAC
+      THEN Q.ASM_CASES_TAC `x = x'`
+      THEN ASM_REWRITE_TAC [FAPPLY_FUPDATE] THENL
+      [POP_ASSUM (fn th => REWRITE_TAC [SYM th]) THEN ASM_REWRITE_TAC [],
+       POP_ASSUM (ASSUME_TAC o NOT_EQ_SYM) 
+         THEN IMP_RES_TAC NOT_EQ_FAPPLY 
+         THEN ASM_REWRITE_TAC []]]);
 
 
+val FUPDATE_EXISTING = Q.store_thm 
+("FUPDATE_EXISTING",
+ `!^fmap v t. FDOM f v /\ (FAPPLY f v = t) = (f = FUPDATE f (v,t))`,
+ REPEAT STRIP_TAC 
+   THEN REWRITE_TAC [ONCE_REWRITE_RULE [EQ_SYM_EQ] fmap_EQ] 
+   THEN CONV_TAC (DEPTH_CONV FUN_EQ_CONV) 
+   THEN EQ_TAC THENL
+   [REPEAT STRIP_TAC 
+      THEN Q.ASM_CASES_TAC `x = v`
+      THEN ASM_REWRITE_TAC [FDOM_FUPDATE,FAPPLY_FUPDATE] 
+      THEN IMP_RES_TAC NOT_EQ_FAPPLY 
+      THEN ASM_REWRITE_TAC[],
+    REPEAT STRIP_TAC 
+      THEN ONCE_ASM_REWRITE_TAC [] 
+      THEN REWRITE_TAC [FDOM_FUPDATE, FAPPLY_FUPDATE]]);
 
 
+(*---------------------------------------------------------------------------
+          Finiteness
+ ---------------------------------------------------------------------------*)
 
-(*----------------------------------------------------
-More theorems
-----------------------------------------------------*)
-
-
-val FUPDATE_EXISTING = store_thm ("FUPDATE_EXISTING",
-Term`!(f:('a,'b)fmap) v t.
-   (FDOM f v) /\ (FAPPLY f v = t)
-    = (f = FUPDATE f (v,t))`,
-REPEAT STRIP_TAC THEN
-REWRITE_TAC [ONCE_REWRITE_RULE [EQ_SYM_EQ] fmap_EQ] THEN
-CONV_TAC (DEPTH_CONV FUN_EQ_CONV) THEN
-EQ_TAC THENL
-[REPEAT STRIP_TAC THEN
- ASM_CASES_TAC (Term`(x:'a)=v`) THEN
- ASM_REWRITE_TAC [FDOM_FUPDATE,FAPPLY_FUPDATE] THEN
- IMP_RES_TAC NOT_EQ_FAPPLY THEN
- ASM_REWRITE_TAC[],
- REPEAT STRIP_TAC THEN
- ONCE_ASM_REWRITE_TAC [] THEN
- REWRITE_TAC [FDOM_FUPDATE, FAPPLY_FUPDATE]
-]);
-
-
-
-(*Finiteness*)
-val FINITE_FMAP = store_thm ("FINITE_FMAP",
-Term`!(f:('a,'b)fmap). ?g. ?n.
-    !x. (FDOM f x) = (?i.  (i <  n) /\  (g i = x))`,
-INDUCT_THEN fmap_INDUCT STRIP_ASSUME_TAC THENL
-[
- EXISTS_TAC (Term`\(x:num).(@(y:'a).F)`) THEN
- EXISTS_TAC (Term`0`) THEN
- REWRITE_TAC [FDOM_FEMPTY, prim_recTheory.NOT_LESS_0],
- REPEAT STRIP_TAC THEN
- EXISTS_TAC (Term`\i:num.(i = n) => (x:'a) | g i`) THEN
- EXISTS_TAC (Term`SUC n`) THEN
- GEN_TAC THEN
- REWRITE_TAC [FDOM_FUPDATE] THEN
- ASM_CASES_TAC (Term`(x':'a) = x`) THEN
- ASM_REWRITE_TAC [] THENL
- [
-  EXISTS_TAC (Term`n:num`) THEN
-  BETA_TAC THEN
-  REWRITE_TAC [prim_recTheory.LESS_SUC_REFL],
-  EQ_TAC THEN STRIP_TAC THENL
-  [
-   EXISTS_TAC (Term`i:num`) THEN
-   IMP_RES_TAC (prim_recTheory.LESS_NOT_EQ) THEN
-   BETA_TAC THEN ASM_REWRITE_TAC [prim_recTheory.LESS_THM],
-   EXISTS_TAC (Term`i:num`) THEN
-   UNDISCH_TAC (Term`(\i:num. (i = n) => (x:'a) | (g i)) i = x'`) THEN
-   BETA_TAC THEN
-   IMP_RES_TAC (prim_recTheory.LESS_LEMMA1) THEN
-   ASM_REWRITE_TAC [] THENL
-   [
-    DISCH_THEN (ASSUME_TAC o SYM) THEN RES_TAC,
-    IMP_RES_TAC (prim_recTheory.LESS_NOT_EQ) THEN
-    ASM_REWRITE_TAC []
-   ]
-  ]
- ]
-]);
+val FINITE_FMAP = Q.store_thm 
+("FINITE_FMAP",
+ `!^fmap. 
+     ?g. ?n. !x. FDOM f x = ?i. i < n /\ (g i = x)`,
+ INDUCT_THEN fmap_INDUCT STRIP_ASSUME_TAC THENL
+ [Q.EXISTS_TAC `\x. @y:'a.F` 
+    THEN Q.EXISTS_TAC `0` 
+    THEN REWRITE_TAC [FDOM_FEMPTY, prim_recTheory.NOT_LESS_0],
+  REPEAT STRIP_TAC 
+    THEN Q.EXISTS_TAC `\i. if i=n then x:'a else g i`
+    THEN Q.EXISTS_TAC `SUC n`
+    THEN GEN_TAC 
+    THEN REWRITE_TAC [FDOM_FUPDATE] 
+    THEN Q.ASM_CASES_TAC `x' = x`
+    THEN ASM_REWRITE_TAC [] THENL
+    [Q.EXISTS_TAC `n`
+       THEN BETA_TAC 
+       THEN REWRITE_TAC [LESS_SUC_REFL],
+     EQ_TAC THEN STRIP_TAC THENL
+     [Q.EXISTS_TAC `i` 
+        THEN IMP_RES_TAC LESS_NOT_EQ
+        THEN BETA_TAC 
+        THEN ASM_REWRITE_TAC [LESS_THM],
+      Q.EXISTS_TAC `i`
+        THEN Q.UNDISCH_TAC `(\i:num. if i=n then x else g i) i = x'`
+        THEN BETA_TAC 
+        THEN IMP_RES_TAC LESS_LEMMA1
+        THEN ASM_REWRITE_TAC [] THENL
+        [DISCH_THEN (ASSUME_TAC o SYM) THEN RES_TAC,
+         IMP_RES_TAC LESS_NOT_EQ THEN ASM_REWRITE_TAC []]]]]);
 
 
 
-(*Completeness*)
-(*Commented out since this is of theoretical interest but is of no
-practical use
-
-val rep_DEF =
- new_definition("rep",
-Term`!f:('a,'b)fmap. rep f = \x. (FDOM f x => INL (FAPPLY f x) | INR one)`)
+(*---------------------------------------------------------------------------
+          Completeness
+ ---------------------------------------------------------------------------*)
 
 
-val rep_empty = prove(Term`rep (FEMPTY:('a,'b)fmap) = (\x. INR one)`,
-REWRITE_TAC [rep_DEF,FDOM_FEMPTY]);
+val rep_DEF = Q.new_definition
+("rep",
+ `!^fmap. rep f = \x. if FDOM f x then INL (FAPPLY f x) else INR one`);
 
-val rep_update = prove(
-Term`!(f:('a,'b)fmap) a b.
-      rep (FUPDATE  f (a,b)) = \x. (x=a => INL b | rep f x)`,
-REPEAT GEN_TAC THEN
-REWRITE_TAC[rep_DEF] THEN
-MATCH_MP_TAC EQ_EXT THEN
-GEN_TAC THEN BETA_TAC THEN
-ASM_CASES_TAC (Term`(x:'a)=a`) THENL
-[
- ASM_REWRITE_TAC [FDOM_FUPDATE,FAPPLY_FUPDATE],
- IMP_RES_TAC NOT_EQ_FAPPLY THEN
- ASM_REWRITE_TAC [FDOM_FUPDATE]
-]);
+val rep_empty = Q.prove
+(`rep ^FEMPTY = \x. INR one`,
+ REWRITE_TAC [rep_DEF,FDOM_FEMPTY]);
 
+val rep_update = Q.prove
+(`!^fmap a b. rep (FUPDATE f (a,b)) = \x. if x=a then INL b else rep f x`,
+ REPEAT GEN_TAC 
+   THEN REWRITE_TAC[rep_DEF] 
+   THEN MATCH_MP_TAC EQ_EXT 
+   THEN GEN_TAC THEN BETA_TAC 
+   THEN Q.ASM_CASES_TAC `x = a` THENL
+   [ASM_REWRITE_TAC [FDOM_FUPDATE,FAPPLY_FUPDATE],
+    IMP_RES_TAC NOT_EQ_FAPPLY 
+      THEN ASM_REWRITE_TAC [FDOM_FUPDATE]]);
 
-val rep_onto = prove(
-Term`!fn:'a -> ('b+one). is_fmap fn ==> (?fm. rep fm = fn)`,
-is_fmap_RULE_INDUCT_TAC THENL
-[EXISTS_TAC(Term`FEMPTY:('a,'b)fmap`) THEN
- REWRITE_TAC [rep_empty],
- GEN_TAC THEN GEN_TAC THEN
- EXISTS_TAC (Term`FUPDATE (fm:('a,'b)fmap) (a,b)`) THEN
- ASM_REWRITE_TAC [rep_update]
-]);
+val rep_onto = Q.prove
+(`!fn:'a -> 'b+one. is_fmap fn ==> ?fm. rep fm = fn`,
+ HO_MATCH_MP_TAC ind 
+   THEN CONJ_TAC THENL
+ [Q.EXISTS_TAC `FEMPTY` THEN REWRITE_TAC [rep_empty],
+  REPEAT STRIP_TAC
+    THEN Q.EXISTS_TAC `FUPDATE fm (a,b)`
+    THEN ASM_REWRITE_TAC [rep_update]]);
 
+val rep_one_one_lemma = Q.prove
+(`!^fmap g. (rep f = rep g) ==> (FDOM f = FDOM g)`,
+ CONV_TAC (DEPTH_CONV FUN_EQ_CONV) 
+   THEN REWRITE_TAC [rep_DEF] 
+   THEN BETA_TAC 
+   THEN REPEAT STRIP_TAC 
+   THEN POP_ASSUM (ASSUME_TAC o Q.SPEC `x`)
+   THEN POP_ASSUM MP_TAC
+   THEN REPEAT COND_CASES_TAC
+   THEN ASM_REWRITE_TAC[sum_distinct, GSYM sum_distinct]);
 
-val rep_one_one_lemma = prove(
-Term`!(f:('a,'b)fmap) g. (rep f = rep g) ==> (FDOM f = FDOM g)`,
-CONV_TAC (DEPTH_CONV FUN_EQ_CONV) THEN
-REWRITE_TAC [rep_DEF] THEN
-BETA_TAC THEN
-REPEAT STRIP_TAC THEN
-POP_ASSUM (ASSUME_TAC o SPEC (Term`x:'a`)) THEN
-UNDISCH_TAC  (Term`((FDOM (f:('a,'b)fmap)  x) => (INL (FAPPLY f x)) | (INR one)) =
-          ((FDOM g x) => (INL (FAPPLY g x)) | (INR one))`) THEN
-ASM_CASES_TAC(Term`FDOM (f:('a,'b)fmap) x`) THEN
-ASM_CASES_TAC(Term`FDOM (g:('a,'b)fmap) x`) THEN
-ASM_REWRITE_TAC [] THEN
-DISCH_THEN (CHECK_ASSUME_TAC o REWRITE_RULE [definition "sum" "ISL"] o
-            AP_TERM (Term`(ISL:'b+one -> bool)`)));
+val rep_one_one = Q.prove
+(`!^fmap g. (rep f = rep g) ==> (f = g)`,
+ REPEAT GEN_TAC 
+   THEN DISCH_THEN (fn th => 
+     let val lm = MATCH_MP rep_one_one_lemma th 
+     in ASSUME_TAC (CONV_RULE FUN_EQ_CONV (REWRITE_RULE [rep_DEF,lm] th))
+          THEN ASSUME_TAC lm
+     end) 
+   THEN REWRITE_TAC [ONCE_REWRITE_RULE [EQ_SYM_EQ] fmap_EQ_THM] 
+   THEN ASM_REWRITE_TAC [] 
+   THEN GEN_TAC 
+   THEN DISCH_THEN (fn th => FIRST_ASSUM (fn asm => 
+         MP_TAC (REWRITE_RULE [th] (BETA_RULE (Q.SPEC `x` asm)))))
+   THEN REWRITE_TAC [INR_INL_11]);
 
-
-val rep_ono_one = prove(
-Term`!(f:('a,'b)fmap) g. (rep f = rep g) ==> (f = g)`,
-REPEAT GEN_TAC THEN
-DISCH_THEN (fn th => let val lm = MATCH_MP rep_one_one_lemma th in
-                      ASSUME_TAC
-                           (CONV_RULE FUN_EQ_CONV
-                               (REWRITE_RULE [rep_DEF,lm] th)) THEN
-                      ASSUME_TAC lm
-                     end) THEN
-REWRITE_TAC [ONCE_REWRITE_RULE [EQ_SYM_EQ] fmap_EQ_THM] THEN
-ASM_REWRITE_TAC [] THEN
-GEN_TAC THEN
-DISCH_THEN (fn th => FIRST_ASSUM
-             (fn asm  => ASSUME_TAC (
-                 REWRITE_RULE [th] (BETA_RULE (SPEC (Term`x:'a`) asm))))) THEN
-POP_ASSUM (fn th =>
-     ASM_REWRITE_TAC [ REWRITE_RULE [definition "sum" "OUTL"] (
-            AP_TERM (Term`(OUTL:'b+one -> 'b)`) th)]));
+val lemma2 = Q.prove
+(`!fm:('a,'b)fmap. is_fmap (rep fm)`,
+ INDUCT_THEN fmap_INDUCT STRIP_ASSUME_TAC THENL
+ [REWRITE_TAC [rep_empty, is_fmap_empty],
+  REPEAT STRIP_TAC 
+   THEN IMP_RES_TAC is_fmap_update 
+   THEN ASM_REWRITE_TAC [rep_update]]);
 
 
-val lemma2 = prove(
-Term`!fm:('a,'b)fmap. is_fmap (rep fm)`,
-INDUCT_THEN fmap_INDUCT STRIP_ASSUME_TAC THENL
-[REWRITE_TAC [rep_empty, is_fmap_empty],
- REPEAT STRIP_TAC THEN
- IMP_RES_TAC is_fmap_update THEN
- ASM_REWRITE_TAC [rep_update]
-]);
+(*---------------------------------------------------------------------------
+      Composition of finite maps
+ ---------------------------------------------------------------------------*)
 
+val f_o_f_lemma = Q.prove 
+(`!f:'b |-> 'c. 
+  !g:'a |-> 'b.
+     ?comp. (!x. FDOM comp x = FDOM g x /\ FDOM f (FAPPLY g x))
+       /\   (!x. FDOM comp x ==> (FAPPLY comp x = (FAPPLY f (FAPPLY g x))))`,
+ GEN_TAC 
+  THEN INDUCT_THEN fmap_INDUCT STRIP_ASSUME_TAC THENL
+  [Q.EXISTS_TAC `FEMPTY` THEN REWRITE_TAC [FDOM_FEMPTY],
+   REPEAT STRIP_TAC 
+    THEN Q.ASM_CASES_TAC `FDOM f y` THENL
+    [Q.EXISTS_TAC `FUPDATE comp (x, FAPPLY f y)` 
+      THEN CONJ_TAC THEN GEN_TAC THENL
+      [Q.ASM_CASES_TAC `x' = x` THENL
+       [ASM_REWRITE_TAC [FDOM_FUPDATE,FAPPLY_FUPDATE],
+        IMP_RES_TAC NOT_EQ_FAPPLY THEN ASM_REWRITE_TAC [FDOM_FUPDATE]],
+       Q.ASM_CASES_TAC `x' = x` THENL
+       [ASM_REWRITE_TAC [FDOM_FUPDATE, FAPPLY_FUPDATE],
+        IMP_RES_TAC NOT_EQ_FAPPLY 
+          THEN IMP_RES_TAC (Q.ISPEC `comp:'a|->'c` NOT_EQ_FAPPLY)
+          THEN ASM_REWRITE_TAC [FDOM_FUPDATE] 
+          THEN STRIP_TAC 
+          THEN FIRST_ASSUM MATCH_MP_TAC 
+          THEN ASM_REWRITE_TAC []]],
+     Q.EXISTS_TAC `comp` 
+       THEN CONJ_TAC THEN GEN_TAC THENL
+       [Q.ASM_CASES_TAC `x' = x` 
+         THEN ASM_REWRITE_TAC [FDOM_FUPDATE,FAPPLY_FUPDATE] 
+         THEN IMP_RES_TAC NOT_EQ_FAPPLY 
+         THEN ASM_REWRITE_TAC [],
+        Q.ASM_CASES_TAC `x' = x` THENL
+        [ASM_REWRITE_TAC [FDOM_FUPDATE, FAPPLY_FUPDATE],
+         STRIP_TAC 
+           THEN IMP_RES_TAC NOT_EQ_FAPPLY 
+           THEN RES_TAC 
+           THEN ASM_REWRITE_TAC [FDOM_FUPDATE]]]]]);
 
-
-*)
-
-(*Composition*)
-
-val f_o_f_lemma = prove (
-Term`!(f : ('b,'c) fmap) (g : ('a,'b) fmap).
-        ?comp.
-           (!x.(FDOM comp x) =
-                      ((FDOM g x) /\ FDOM f (FAPPLY g x))) /\
-           (!x.FDOM comp x ==> (FAPPLY comp x =
-               (FAPPLY f (FAPPLY g x))))`,
-GEN_TAC THEN
-INDUCT_THEN fmap_INDUCT STRIP_ASSUME_TAC THENL
-[
- EXISTS_TAC (Term`FEMPTY:('a,'c)fmap`) THEN
- REWRITE_TAC [FDOM_FEMPTY],
- REPEAT STRIP_TAC THEN
- (*ASSUM_LIST (fn ths =>
-   STRIP_ASSUME_TAC (SPEC (Term`f: ('b,'c) fmap`) (el 2 ths))) THEN *)
- ASM_CASES_TAC (Term`FDOM (f:('b,'c) fmap) y`) THENL
- [
-  EXISTS_TAC (Term`FUPDATE (comp:('a,'c)fmap) (x,(FAPPLY f (y:'b)))`) THEN
-  CONJ_TAC THEN GEN_TAC THENL
-  [
-   ASM_CASES_TAC (Term`(x':'a) = x`) THENL
-   [
-     ASM_REWRITE_TAC [FDOM_FUPDATE,FAPPLY_FUPDATE],
-      IMP_RES_TAC NOT_EQ_FAPPLY THEN
-     ASM_REWRITE_TAC [FDOM_FUPDATE]
-   ],
-   ASM_CASES_TAC (Term`(x':'a) = x`) THENL
-   [
-     ASM_REWRITE_TAC [FDOM_FUPDATE, FAPPLY_FUPDATE],
-     IMP_RES_TAC NOT_EQ_FAPPLY THEN
-     IMP_RES_TAC (ISPEC (Term`comp:('a,'c)fmap`) NOT_EQ_FAPPLY)THEN
-     ASM_REWRITE_TAC [FDOM_FUPDATE] THEN
-     STRIP_TAC THEN
-     FIRST_ASSUM MATCH_MP_TAC THEN
-     ASM_REWRITE_TAC []
-   ]
-  ],
-  EXISTS_TAC (Term`comp:('a,'c)fmap`) THEN
-  CONJ_TAC THEN GEN_TAC  THENL
-  [
-   ASM_CASES_TAC (Term`(x':'a) = x`) THEN
-   ASM_REWRITE_TAC [FDOM_FUPDATE,FAPPLY_FUPDATE] THEN
-   IMP_RES_TAC NOT_EQ_FAPPLY THEN
-   ASM_REWRITE_TAC [] ,
-   ASM_CASES_TAC (Term`(x':'a) = x`) THENL
-   [
-     ASM_REWRITE_TAC [FDOM_FUPDATE, FAPPLY_FUPDATE],
-     STRIP_TAC THEN
-     IMP_RES_TAC NOT_EQ_FAPPLY THEN
-     RES_TAC THEN
-     ASM_REWRITE_TAC [FDOM_FUPDATE]
-   ]
-  ]
- ]
-]);
-
-
-val f_o_f_exists = CONV_RULE (ONCE_DEPTH_CONV SKOLEM_CONV) f_o_f_lemma;
 
 val f_o_f_DEF =
-   new_specification {name = "f_o_f_DEF",
-                      consts = [{fixity = Infixl 500,
-                                 const_name = "f_o_f"}],
-                      sat_thm = f_o_f_exists};
+  new_specification 
+    {name = "f_o_f_DEF",
+     consts = [{fixity = Infixl 500, const_name = "f_o_f"}],
+     sat_thm = CONV_RULE (ONCE_DEPTH_CONV SKOLEM_CONV) f_o_f_lemma};
 
 val fmap_EQ_TAC =
-  PURE_REWRITE_TAC [
-    CONV_RULE (DEPTH_CONV FUN_EQ_CONV)
-      (GSYM (fmap_EQ_THM))];
+  PURE_REWRITE_TAC 
+   [CONV_RULE(DEPTH_CONV FUN_EQ_CONV) (GSYM fmap_EQ_THM)];
 
-val f_o_f_FEMPTY_1 =
-store_thm ("f_o_f_FEMPTY_1",
-(Term`!(f:('a,'b)fmap). (FEMPTY:('b,'c)fmap) f_o_f f = FEMPTY`),
-    GEN_TAC THEN fmap_EQ_TAC THEN
-    REWRITE_TAC [f_o_f_DEF,FDOM_FEMPTY]
-);
+val f_o_f_FEMPTY_1 = Q.store_thm 
+("f_o_f_FEMPTY_1",
+ `!^fmap. (FEMPTY:('b,'c)fmap) f_o_f f = FEMPTY`,
+ GEN_TAC THEN fmap_EQ_TAC 
+   THEN REWRITE_TAC [f_o_f_DEF,FDOM_FEMPTY]);
 
-val f_o_f_FEMPTY_2 =
-save_thm("f_o_f_FEMPTY_2", prove((Term`!(f:('b,'c)fmap). f f_o_f (FEMPTY:('a,'b)fmap) = FEMPTY`),
-    GEN_TAC THEN fmap_EQ_TAC THEN
-    REWRITE_TAC [f_o_f_DEF,FDOM_FEMPTY]
-));
+val f_o_f_FEMPTY_2 = Q.store_thm
+("f_o_f_FEMPTY_2", 
+ `!f:'b|->'c. f f_o_f (FEMPTY:('a,'b)fmap) = FEMPTY`,
+    GEN_TAC THEN fmap_EQ_TAC 
+      THEN REWRITE_TAC [f_o_f_DEF,FDOM_FEMPTY]);
 
-val o_f_lemma = prove (
-Term`!(f : 'b -> 'c) (g : ('a,'b) fmap).
-        ?comp.
-           (!x.(FDOM comp x) =
-                      (FDOM g x))  /\
-           (!x.FDOM comp x ==> (FAPPLY comp x =
-               (f (FAPPLY g x))))`,
-GEN_TAC THEN
-INDUCT_THEN fmap_INDUCT STRIP_ASSUME_TAC THENL
-[
- EXISTS_TAC (Term`FEMPTY:('a,'c)fmap`) THEN
- REWRITE_TAC [FDOM_FEMPTY],
- REPEAT STRIP_TAC THEN
- EXISTS_TAC (Term`FUPDATE (comp:('a,'c)fmap) (x,(f (y:'b)))`) THEN
- CONJ_TAC THEN GEN_TAC THEN ASM_REWRITE_TAC [FDOM_FUPDATE] THEN
- ASM_CASES_TAC (Term`(x':'a) = x`) THENL
-  [
-   STRIP_TAC THEN
-   ASM_REWRITE_TAC [FAPPLY_FUPDATE],
-   IMP_RES_TAC NOT_EQ_FAPPLY THEN
-   IMP_RES_TAC (ISPEC (Term`comp:('a,'c)fmap`) NOT_EQ_FAPPLY) THEN
-   ASM_REWRITE_TAC [] THEN
-   STRIP_TAC THEN
-   FIRST_ASSUM MATCH_MP_TAC THEN
-   ASM_REWRITE_TAC []
-  ]
-]);
-
-
-val o_f_exists = CONV_RULE (ONCE_DEPTH_CONV SKOLEM_CONV) o_f_lemma;
+val o_f_lemma = Q.prove 
+(`!f:'b->'c.
+  !g:'a|->'b.
+    ?comp. (!x. FDOM comp x = FDOM g x) 
+      /\   (!x. FDOM comp x ==> (FAPPLY comp x = f (FAPPLY g x)))`,
+ GEN_TAC 
+  THEN INDUCT_THEN fmap_INDUCT STRIP_ASSUME_TAC THENL
+  [Q.EXISTS_TAC `FEMPTY` THEN REWRITE_TAC [FDOM_FEMPTY],
+   REPEAT STRIP_TAC 
+     THEN Q.EXISTS_TAC `FUPDATE comp (x, f y)`
+     THEN CONJ_TAC 
+     THEN GEN_TAC 
+     THEN ASM_REWRITE_TAC [FDOM_FUPDATE] 
+     THEN Q.ASM_CASES_TAC `x' = x` THENL
+     [STRIP_TAC THEN ASM_REWRITE_TAC [FAPPLY_FUPDATE],
+      IMP_RES_TAC NOT_EQ_FAPPLY 
+        THEN IMP_RES_TAC (Q.ISPEC `comp:'a|->'c` NOT_EQ_FAPPLY)
+        THEN ASM_REWRITE_TAC [] 
+        THEN STRIP_TAC 
+        THEN FIRST_ASSUM MATCH_MP_TAC 
+        THEN ASM_REWRITE_TAC []]]);
 
 val o_f_DEF =
-   new_specification {name = "o_f_DEF",
-                      consts = [{fixity = Infixl 500,
-                                 const_name = "o_f"}],
-                      sat_thm = o_f_exists};
+   new_specification 
+     {name = "o_f_DEF",
+      consts = [{fixity = Infixl 500, const_name = "o_f"}],
+      sat_thm = CONV_RULE (ONCE_DEPTH_CONV SKOLEM_CONV) o_f_lemma};
 
 
-val o_f_FDOM = store_thm("o_f_FDOM",
-Term`!(f : 'b -> 'c) (g : ('a,'b) fmap).
-       (!x. FDOM  g x = (FDOM (f o_f g) x))`,
+val o_f_FDOM = Q.store_thm
+("o_f_FDOM",
+ `!f:'b -> 'c. !g:'a |->'b. !x. FDOM  g x = FDOM (f o_f g) x`,
 REWRITE_TAC [o_f_DEF]);
 
-val o_f_FAPPLY = store_thm("o_f_APPLY",
-Term`!(f : 'b -> 'c) (g : ('a,'b) fmap).
-       (!x. FDOM  g x ==> (FAPPLY (f o_f g) x = f (FAPPLY g x)))`,
-REPEAT STRIP_TAC THEN
-STRIP_ASSUME_TAC (SPECL [Term`f : 'b -> 'c`,Term`g : ('a,'b) fmap`] o_f_DEF) THEN
-FIRST_ASSUM MATCH_MP_TAC THEN
-ASM_REWRITE_TAC []);
+val o_f_FAPPLY = Q.store_thm
+("o_f_APPLY",
+ `!f:'b->'c. !g:('a,'b) fmap. 
+   !x. FDOM  g x ==> (FAPPLY (f o_f g) x = f (FAPPLY g x))`,
+ REPEAT STRIP_TAC 
+  THEN STRIP_ASSUME_TAC (Q.SPECL [`f:'b -> 'c`, `g:('a,'b) fmap`] o_f_DEF)
+  THEN FIRST_ASSUM MATCH_MP_TAC 
+  THEN ASM_REWRITE_TAC []);
 
 
+(*---------------------------------------------------------------------------
+          Range of a finite map
+ ---------------------------------------------------------------------------*)
+
+val FRANGE_DEF = Q.new_definition
+("FRANGE_DEF",
+ `FRANGE ^fmap y = ?x. FDOM f x /\ (FAPPLY f x = y)`);
+
+val FRANGE_FEMPTY = Q.store_thm 
+("FRANGE_FEMPTY",
+ `!x. ~FRANGE ^FEMPTY x`,
+ REWRITE_TAC [FRANGE_DEF, FDOM_FEMPTY]);
+
+val FRANGE_FUPDATE = Q.store_thm 
+("FRANGE_FUPDATE",
+ `!^fmap x y b.
+     FRANGE (FUPDATE f (x,y)) b 
+       =
+     (y = b) \/ FRANGE (DRESTRICT f (\a. ~(a = x))) b`,
+ REPEAT GEN_TAC 
+   THEN REWRITE_TAC [FRANGE_DEF,FDOM_FUPDATE,DRESTRICT_DEF] 
+   THEN BETA_TAC 
+   THEN EQ_TAC THEN STRIP_TAC THENL
+   [Q.PAT_ASSUM `p = q` MP_TAC
+      THEN ASM_REWRITE_TAC [FAPPLY_FUPDATE] 
+      THEN DISCH_TAC THEN ASM_REWRITE_TAC [],
+    Q.ASM_CASES_TAC `x' = x` THENL
+    [Q.PAT_ASSUM `FAPPLY p q = z` MP_TAC
+       THEN ASM_REWRITE_TAC [FAPPLY_FUPDATE] 
+       THEN DISCH_TAC THEN ASM_REWRITE_TAC [],
+     DISJ2_TAC 
+       THEN Q.EXISTS_TAC `x'` 
+       THEN ASM_REWRITE_TAC [] 
+       THEN IMP_RES_TAC NOT_EQ_FAPPLY 
+       THEN POP_ASSUM (ASSUME_TAC o Q.SPECL [`y:'b`, `f:('a,'b)fmap`]
+                        o ONCE_REWRITE_RULE [EQ_SYM_EQ]) 
+       THEN ASM_REWRITE_TAC []],
+    Q.EXISTS_TAC `x` THEN ASM_REWRITE_TAC [FAPPLY_FUPDATE],
+    Q.EXISTS_TAC `x'`
+       THEN IMP_RES_TAC NOT_EQ_FAPPLY 
+       THEN ASM_REWRITE_TAC [] 
+       THEN Q.PAT_ASSUM `p = q` MP_TAC
+       THEN ASM_REWRITE_TAC []]);
+
+val SUBMAP_FRANGE = Q.store_thm
+("SUBMAP_FRANGE",
+ `!^fmap g. f SUBMAP g ==> !x. FRANGE f x ==> FRANGE g x`,
+ REPEAT GEN_TAC 
+   THEN REWRITE_TAC [SUBMAP_DEF,FRANGE_DEF] 
+   THEN REPEAT STRIP_TAC 
+   THEN Q.EXISTS_TAC `x'`
+   THEN RES_TAC 
+   THEN POP_ASSUM SUBST_ALL_TAC 
+   THEN ASM_REWRITE_TAC []);
 
 
-(*Range*)
+(*---------------------------------------------------------------------------
+        Range restriction
+ ---------------------------------------------------------------------------*)
 
-val FRANGE_DEF =
-new_definition("FRANGE_DEF",
-Term`!(f:('a,'b)fmap) y. FRANGE f y = (?x.FDOM f x /\ (FAPPLY f x = y))`);
+val ranres_lemma = Q.prove 
+(`!^fmap (r:'b -> bool).
+    ?res. (!x. FDOM res x = FDOM f x /\ r (FAPPLY f x))
+      /\  (!x. FAPPLY res x =
+                 if FDOM f x /\ r (FAPPLY f x)
+                   then FAPPLY f x
+                   else FAPPLY FEMPTY x)`,
+ INDUCT_THEN fmap_INDUCT ASSUME_TAC THENL
+ [GEN_TAC 
+    THEN Q.EXISTS_TAC `FEMPTY`
+    THEN REWRITE_TAC [FDOM_FEMPTY],
+  REPEAT STRIP_TAC 
+    THEN ASSUM_LIST(fn ths => STRIP_ASSUME_TAC(Q.SPEC `r:'b->bool` (el 2 ths)))
+    THEN Q.ASM_CASES_TAC `r y` THENL
+    [Q.EXISTS_TAC `FUPDATE res (x,y)`
+       THEN CONJ_TAC THEN GEN_TAC 
+       THEN Q.ASM_CASES_TAC `x' = x` THENL
+       [ASM_REWRITE_TAC [FDOM_FUPDATE, FAPPLY_FUPDATE],
+        IMP_RES_TAC NOT_EQ_FAPPLY THEN ASM_REWRITE_TAC [FDOM_FUPDATE],
+        ASM_REWRITE_TAC [FDOM_FUPDATE, FAPPLY_FUPDATE],
+        IMP_RES_TAC NOT_EQ_FAPPLY THEN ASM_REWRITE_TAC [FDOM_FUPDATE]],
+     Q.EXISTS_TAC `res`
+       THEN CONJ_TAC THEN GEN_TAC
+       THEN Q.ASM_CASES_TAC `x' = x` THENL
+       [ASM_REWRITE_TAC [FDOM_FUPDATE, FAPPLY_FUPDATE],
+        IMP_RES_TAC NOT_EQ_FAPPLY THEN ASM_REWRITE_TAC [FDOM_FUPDATE],
+        ASM_REWRITE_TAC [FDOM_FUPDATE, FAPPLY_FUPDATE],
+        IMP_RES_TAC NOT_EQ_FAPPLY THEN ASM_REWRITE_TAC [FDOM_FUPDATE]]]]);
 
-val FRANGE_FEMPTY = store_thm ("FRANGE_FEMPTY",
-Term`!x. ~(FRANGE (FEMPTY:('a,'b)fmap) x)`,
-REWRITE_TAC [FRANGE_DEF, FDOM_FEMPTY]);
+val ranres_lemma = Q.prove 
+(`!^fmap (r:'b -> bool).
+    ?res. (!x. FDOM res x = FDOM f x /\ r (FAPPLY f x))
+      /\  (!x. FAPPLY res x =
+                 if FDOM f x /\ r (FAPPLY f x)
+                   then FAPPLY f x
+                   else FAPPLY FEMPTY x)`,
+ INDUCT_THEN fmap_INDUCT ASSUME_TAC THENL
+ [GEN_TAC 
+    THEN Q.EXISTS_TAC `FEMPTY`
+    THEN REWRITE_TAC [FDOM_FEMPTY],
+  REPEAT STRIP_TAC 
+    THEN ASSUM_LIST(fn ths => STRIP_ASSUME_TAC(Q.SPEC `r:'b->bool` (el 2 ths)))
+    THEN Q.ASM_CASES_TAC `r y` THENL
+    [Q.EXISTS_TAC `FUPDATE res (x,y)`, Q.EXISTS_TAC `res`]
+    THEN CONJ_TAC THEN GEN_TAC 
+    THEN Q.ASM_CASES_TAC `x' = x` THEN
+    ((ASM_REWRITE_TAC [FDOM_FUPDATE, FAPPLY_FUPDATE] THEN NO_TAC)
+       ORELSE 
+     (IMP_RES_TAC NOT_EQ_FAPPLY THEN ASM_REWRITE_TAC [FDOM_FUPDATE]))]);
 
-val FRANGE_FUPDATE = store_thm ("FRANGE_FUPDATE",
-Term`!(f:('a,'b)fmap)x y b.
-         FRANGE (FUPDATE f (x,y)) b =
-            (y = b) \/ FRANGE (DRESTRICT f (\a.~(a=x))) b`,
-REPEAT GEN_TAC THEN
-REWRITE_TAC [FRANGE_DEF,FDOM_FUPDATE,DRESTRICT_DEF] THEN
-BETA_TAC THEN
-EQ_TAC THEN STRIP_TAC  THENL
-[
- UNDISCH_TAC  (Term`FAPPLY (FUPDATE (f:('a,'b)fmap) (x,y)) x' = b`) THEN
- ASM_REWRITE_TAC [FAPPLY_FUPDATE] THEN
- DISCH_TAC THEN ASM_REWRITE_TAC [],
-
- ASM_CASES_TAC (Term`(x':'a)=x`) THENL
- [
-  UNDISCH_TAC
-    (Term`FAPPLY (FUPDATE (f:('a,'b)fmap) (x,y)) x' = b`) THEN
-  ASM_REWRITE_TAC [FAPPLY_FUPDATE] THEN
-  DISCH_TAC THEN ASM_REWRITE_TAC [],
-  DISJ2_TAC THEN
-  EXISTS_TAC (Term`x':'a`) THEN
-  ASM_REWRITE_TAC [] THEN
-  IMP_RES_TAC NOT_EQ_FAPPLY THEN
-  POP_ASSUM (ASSUME_TAC o SPECL [Term`y:'b`,Term`f:('a,'b)fmap`] o
-             ONCE_REWRITE_RULE [EQ_SYM_EQ]) THEN
-  ASM_REWRITE_TAC []
- ],
- EXISTS_TAC (Term`x:'a`) THEN
- ASM_REWRITE_TAC [FAPPLY_FUPDATE],
-  EXISTS_TAC (Term`x':'a`) THEN
-  IMP_RES_TAC NOT_EQ_FAPPLY THEN
-  ASM_REWRITE_TAC [] THEN
-  UNDISCH_TAC   (Term`((FDOM (f:('a,'b)fmap) x' /\ ~(x' = x))
-           => (FAPPLY f x')
-           | (FAPPLY FEMPTY x')) =
-          b`) THEN
-  ASM_REWRITE_TAC []
-]);
-
-val SUBMAP_FRANGE = store_thm("SUBMAP_FRANGE",
-Term`!(f : ('a,'b) fmap) g.
-    f SUBMAP g ==> !x.  FRANGE f x ==> FRANGE g x`,
-REPEAT GEN_TAC THEN
-REWRITE_TAC [SUBMAP_DEF,FRANGE_DEF] THEN
-REPEAT STRIP_TAC THEN
-EXISTS_TAC (Term`x':'a`) THEN
-RES_TAC THEN
-POP_ASSUM SUBST_ALL_TAC THEN
-ASM_REWRITE_TAC []);
-
-
-(*Range restriction*)
-
-val ranres_lemma = prove (
-Term`!(f : ('a,'b) fmap) (r: 'b -> bool).
-        ?res.
-           (!x.(FDOM res x) = ((FDOM f x) /\ r (FAPPLY f x))) /\
-           (!x.FAPPLY res x =
-               ((FDOM f x /\ r (FAPPLY f x)) =>
-                   (FAPPLY f x) | (FAPPLY FEMPTY x)))`,
-INDUCT_THEN fmap_INDUCT ASSUME_TAC THENL
-[
- GEN_TAC THEN
- EXISTS_TAC (Term`FEMPTY:('a,'b)fmap`) THEN
- REWRITE_TAC [FDOM_FEMPTY],
- REPEAT STRIP_TAC THEN
- ASSUM_LIST (fn ths =>
-   STRIP_ASSUME_TAC (SPEC (Term`r:'b->bool`) (el 2 ths))) THEN
- ASM_CASES_TAC (Term`(r:'b -> bool) y`) THENL
- [
-  EXISTS_TAC (Term`FUPDATE (res:('a,'b)fmap) (x,y)`) THEN
-  CONJ_TAC THEN GEN_TAC THEN
-   (ASM_CASES_TAC (Term`(x':'a) = x`) THENL
-   [
-     ASM_REWRITE_TAC [FDOM_FUPDATE, FAPPLY_FUPDATE],
-     IMP_RES_TAC NOT_EQ_FAPPLY THEN
-     ASM_REWRITE_TAC [FDOM_FUPDATE]
-   ])
-  ,
-  EXISTS_TAC (Term`res:('a,'b)fmap`) THEN
-  CONJ_TAC THEN GEN_TAC  THEN
-   (ASM_CASES_TAC (Term`(x':'a) = x`) THENL
-   [
-     ASM_REWRITE_TAC [FDOM_FUPDATE, FAPPLY_FUPDATE],
-     IMP_RES_TAC NOT_EQ_FAPPLY THEN
-     ASM_REWRITE_TAC [FDOM_FUPDATE]
-   ])
- ]
-]);
-
-val FRANGE_exists = CONV_RULE (ONCE_DEPTH_CONV SKOLEM_CONV) ranres_lemma;
 
 val RRESTRICT_DEF =
-   new_specification {name = "RRESTRICT_DEF",
-                      consts = [{fixity = Prefix,
-                                 const_name = "RRESTRICT"}],
-                      sat_thm = FRANGE_exists};
+   new_specification 
+     {name = "RRESTRICT_DEF",
+      consts = [{fixity = Prefix, const_name = "RRESTRICT"}],
+      sat_thm = CONV_RULE (ONCE_DEPTH_CONV SKOLEM_CONV) ranres_lemma};
 
-val RRESTRICT_FEMPTY =
-store_thm ("RRESTRICT_FEMPTY",
-Term`!r.RRESTRICT (FEMPTY:('a,'b)fmap) r = FEMPTY`,
-REWRITE_TAC [ONCE_REWRITE_RULE [EQ_SYM_EQ] fmap_EQ] THEN
-CONV_TAC (DEPTH_CONV FUN_EQ_CONV) THEN
-REWRITE_TAC [RRESTRICT_DEF, FDOM_FEMPTY]);
+val RRESTRICT_FEMPTY = Q.store_thm 
+("RRESTRICT_FEMPTY",
+ `!r.RRESTRICT ^FEMPTY r = FEMPTY`,
+ REWRITE_TAC [ONCE_REWRITE_RULE [EQ_SYM_EQ] fmap_EQ] 
+   THEN CONV_TAC (DEPTH_CONV FUN_EQ_CONV) 
+   THEN REWRITE_TAC [RRESTRICT_DEF, FDOM_FEMPTY]);
 
-val RRESTRICT_FUPDATE =
-store_thm ("RRESTRICT_FUPDATE",
-Term`!(f:('a,'b)fmap) r x y.
-     RRESTRICT (FUPDATE f (x,y)) r =
-            (r y => (FUPDATE (RRESTRICT f r) (x,y))
-                                | RRESTRICT
-                                     (DRESTRICT f (\a.~(a=x))) r)`,
-REPEAT STRIP_TAC THEN
-COND_CASES_TAC THENL
-[
-REWRITE_TAC [ONCE_REWRITE_RULE [EQ_SYM_EQ] fmap_EQ] THEN
-CONV_TAC (DEPTH_CONV FUN_EQ_CONV) THEN
-ASM_REWRITE_TAC [FDOM_FUPDATE,RRESTRICT_DEF,DRESTRICT_DEF] THEN
-REPEAT STRIP_TAC THEN
-ASM_CASES_TAC (Term`(x':'a) = x`) THEN
-ASM_REWRITE_TAC [FAPPLY_FUPDATE] THEN
-TRY (IMP_RES_TAC NOT_EQ_FAPPLY) THEN
-ASM_REWRITE_TAC [RRESTRICT_DEF],
-
-REWRITE_TAC [ONCE_REWRITE_RULE [EQ_SYM_EQ] fmap_EQ] THEN
-CONV_TAC (DEPTH_CONV FUN_EQ_CONV) THEN
-ASM_REWRITE_TAC [FDOM_FUPDATE,RRESTRICT_DEF,DRESTRICT_DEF] THEN
-REPEAT STRIP_TAC THEN
-ASM_CASES_TAC (Term`(x':'a) = x`) THEN
-BETA_TAC THENL
-[
-ASM_REWRITE_TAC [FAPPLY_FUPDATE],
-
-IMP_RES_TAC NOT_EQ_FAPPLY THEN
-ASM_REWRITE_TAC [RRESTRICT_DEF] THEN
-COND_CASES_TAC THEN ASM_REWRITE_TAC [],
-
-ASM_REWRITE_TAC [FAPPLY_FUPDATE],
-
-IMP_RES_TAC NOT_EQ_FAPPLY THEN
-ASM_REWRITE_TAC [RRESTRICT_DEF] THEN
-COND_CASES_TAC THEN ASM_REWRITE_TAC [] THEN
-POP_ASSUM (STRIP_ASSUME_TAC o REWRITE_RULE [DE_MORGAN_THM] ) THEN
-ASM_REWRITE_TAC [] THEN
-COND_CASES_TAC THEN ASM_REWRITE_TAC [] THEN
-POP_ASSUM (fn th => ASSUME_TAC
-      (REWRITE_RULE [CONJUNCT1 th] (CONJUNCT2 th) )) THEN
-RES_TAC
-]]);
+val RRESTRICT_FUPDATE = Q.store_thm
+("RRESTRICT_FUPDATE",
+`!^fmap r x y.
+    RRESTRICT (FUPDATE f (x,y)) r =
+      if r y then FUPDATE (RRESTRICT f r) (x,y)
+             else RRESTRICT (DRESTRICT f (\a. ~(a = x))) r`,
+ REPEAT STRIP_TAC 
+   THEN COND_CASES_TAC THENL
+   [REWRITE_TAC [ONCE_REWRITE_RULE [EQ_SYM_EQ] fmap_EQ] 
+      THEN CONV_TAC (DEPTH_CONV FUN_EQ_CONV) 
+      THEN ASM_REWRITE_TAC [FDOM_FUPDATE,RRESTRICT_DEF,DRESTRICT_DEF] 
+      THEN REPEAT STRIP_TAC 
+      THEN Q.ASM_CASES_TAC `x' = x`
+      THEN ASM_REWRITE_TAC [FAPPLY_FUPDATE] 
+      THEN TRY (IMP_RES_TAC NOT_EQ_FAPPLY) 
+      THEN ASM_REWRITE_TAC [RRESTRICT_DEF],
+    REWRITE_TAC [ONCE_REWRITE_RULE [EQ_SYM_EQ] fmap_EQ] 
+      THEN CONV_TAC (DEPTH_CONV FUN_EQ_CONV) 
+      THEN ASM_REWRITE_TAC [FDOM_FUPDATE,RRESTRICT_DEF,DRESTRICT_DEF] 
+      THEN REPEAT STRIP_TAC 
+      THEN Q.ASM_CASES_TAC `x' = x`
+      THEN BETA_TAC THENL
+      [ASM_REWRITE_TAC [FAPPLY_FUPDATE],
+       IMP_RES_TAC NOT_EQ_FAPPLY 
+          THEN ASM_REWRITE_TAC [RRESTRICT_DEF] 
+          THEN COND_CASES_TAC THEN ASM_REWRITE_TAC [],
+       ASM_REWRITE_TAC [FAPPLY_FUPDATE],
+       IMP_RES_TAC NOT_EQ_FAPPLY 
+          THEN ASM_REWRITE_TAC [RRESTRICT_DEF] 
+          THEN COND_CASES_TAC THEN ASM_REWRITE_TAC [] 
+          THEN POP_ASSUM (STRIP_ASSUME_TAC o REWRITE_RULE [DE_MORGAN_THM])
+          THEN ASM_REWRITE_TAC [] 
+          THEN COND_CASES_TAC THEN ASM_REWRITE_TAC [] 
+          THEN POP_ASSUM (fn th => ASSUME_TAC
+                 (REWRITE_RULE [CONJUNCT1 th] (CONJUNCT2 th))) 
+          THEN RES_TAC]]);
 
 
+(*---------------------------------------------------------------------------
+       Functions as finite maps.
 
-(*Functions as finite maps*)
+   We first define a function to test if a predicate is true for a finite
+   number of elements. Should actually be able to take this from
+   pred_setTheory.
+ ---------------------------------------------------------------------------*)
 
-(*First we define a function to test if a predicate is
-true for a finite number of elements*)
+val (rules,FINITE_PRED_INDUCT,cases) = 
+  gen_new_inductive_definition bool_monoset
+    (Term`FINITE_PRED (\a. F) /\
+    !f a. FINITE_PRED f ==> FINITE_PRED (\x. (x=a) \/ f x)`);
 
+val rules_list as [FINITE_PRED_EMPTY, FINITE_PRED_UPDATE] = CONJUNCTS rules;
 
+val ffmap_lemma = Q.prove 
+(`!(f:'a -> 'b) (P: 'a -> bool).
+     FINITE_PRED P ==>
+        ?ffmap. (!x. FDOM ffmap x = P x) 
+           /\   (!x. P x ==> (FAPPLY ffmap x = f x))`,
+ GEN_TAC 
+   THEN HO_MATCH_MP_TAC FINITE_PRED_INDUCT 
+   THEN CONJ_TAC THENL
+   [Q.EXISTS_TAC `FEMPTY`
+     THEN BETA_TAC 
+     THEN REWRITE_TAC [FDOM_FEMPTY],
+    REPEAT STRIP_TAC
+      THEN Q.EXISTS_TAC `FUPDATE ffmap (a, f a)`
+      THEN BETA_TAC 
+      THEN ASM_REWRITE_TAC [FDOM_FUPDATE] 
+      THEN STRIP_TAC 
+      THEN Q.ASM_CASES_TAC `x = a` THENL
+      [ASM_REWRITE_TAC [FAPPLY_FUPDATE],
+       ASM_REWRITE_TAC [] 
+         THEN DISCH_TAC 
+         THEN RES_TAC 
+         THEN IMP_RES_TAC NOT_EQ_FAPPLY 
+         THEN ASM_REWRITE_TAC []]]);
 
-val {rules = FINITE_PRED_RULES, induction = FINITE_PRED_INDUCT} =
- let val FINITE_PRED  = Term`FINITE_PRED :('a -> bool) -> bool`
-     infix -------------------------------------
-     fun (x ------------------------------------- y) = (x,y)
-  in
-   indDefine "FINITE_PRED"
-        [ ([],                               [])
-          -------------------------------------
-                 `^FINITE_PRED  (\a. F)`       ,
-
-
-          ([    `^FINITE_PRED  f`         ],[])
-          -------------------------------------
-          `^FINITE_PRED  (\x. (x = a) \/  f x)` ]  Prefix (`^FINITE_PRED  f`,[])
-   end
- handle x => Raise x;
-
-val [FINITE_PRED_EMPTY, FINITE_PRED_UPDATE] = FINITE_PRED_RULES;
-
-
-
-val ffmap_lemma = prove (
-Term`!(f:'a -> 'b) (P: 'a -> bool).
-       FINITE_PRED P ==>
-        ?ffmap.
-           (!x.(FDOM ffmap x) = (P x)) /\
-           (!x. P x  ==>  (FAPPLY ffmap x = f x))`,
-GEN_TAC THEN
-ind_defLib.RULE_INDUCT_THEN FINITE_PRED_INDUCT
-   STRIP_ASSUME_TAC STRIP_ASSUME_TAC THENL
-[
- EXISTS_TAC (Term`FEMPTY:('a,'b)fmap`) THEN
- BETA_TAC THEN
- REWRITE_TAC [FDOM_FEMPTY],
- GEN_TAC THEN
- EXISTS_TAC (Term`FUPDATE (ffmap:('a,'b)fmap) (a,f a)`) THEN
- BETA_TAC THEN
- ASM_REWRITE_TAC [FDOM_FUPDATE] THEN
- STRIP_TAC THEN ASM_CASES_TAC (Term`(x:'a)=a`) THENL
- [
-  ASM_REWRITE_TAC [FAPPLY_FUPDATE],
-  ASM_REWRITE_TAC [] THEN DISCH_TAC THEN
-  RES_TAC THEN
-  IMP_RES_TAC NOT_EQ_FAPPLY THEN
-  ASM_REWRITE_TAC []
- ]
-]);
-
-
-val ffmap_exists = CONV_RULE
-          (ONCE_DEPTH_CONV RIGHT_IMP_EXISTS_CONV THENC
-           ONCE_DEPTH_CONV SKOLEM_CONV) ffmap_lemma;
 
 val FUN_FMAP_DEF =
-   new_specification {name = "FUN_FMAP_DEF",
-                      consts = [{fixity = Prefix,
-                                 const_name = "FUN_FMAP"}],
-                      sat_thm = ffmap_exists} handle x => Raise x;
+   new_specification 
+     {name = "FUN_FMAP_DEF",
+      consts = [{fixity = Prefix, const_name = "FUN_FMAP"}],
+      sat_thm = CONV_RULE
+                  (ONCE_DEPTH_CONV RIGHT_IMP_EXISTS_CONV THENC
+                   ONCE_DEPTH_CONV SKOLEM_CONV) ffmap_lemma};
 
 
-(*Composition of finite map and function*)
+(*---------------------------------------------------------------------------
+         Composition of finite map and function
+ ---------------------------------------------------------------------------*)
 
-val f_o_DEF = new_infixl_definition("f_o_DEF",
-Term`f_o (f:('b,'c)fmap) (g:'a -> 'b)
-     = f f_o_f (FUN_FMAP g (\x. FDOM f (g x)))`,
-500);
+val f_o_DEF = new_infixl_definition
+("f_o_DEF",
+Term`f_o (f:('b,'c)fmap) (g:'a->'b) 
+      = f f_o_f (FUN_FMAP g (\x. FDOM f (g x)))`, 500);
 
-val FDOM_f_o = store_thm ("FDOM_f_o",
-Term`!(f : ('b, 'c)fmap)  (g : 'a -> 'b).
-      FINITE_PRED (\x. FDOM f (g x)) ==>
-              (!x. FDOM (f f_o g) x =  (FDOM f (g x)))`,
-REPEAT GEN_TAC THEN
-DISCH_THEN (fn th => STRIP_ASSUME_TAC (BETA_RULE
-   (SPEC (Term`g:'a->'b`)  (MATCH_MP FUN_FMAP_DEF th)))) THEN
-ASM_REWRITE_TAC [f_o_DEF,f_o_f_DEF ] THEN GEN_TAC THEN
-EQ_TAC THEN
-STRIP_TAC THEN
-RES_TAC THEN
-ASM_REWRITE_TAC []);
-
-
- val FAPPLY_f_o = store_thm ("FAPPLY_f_o",
-Term`!(f : ('b, 'c)fmap)  (g : 'a -> 'b).
-      FINITE_PRED (\x. FDOM f (g x)) ==>
-           (!x.FDOM (f f_o g) x ==>
-             (FAPPLY (f f_o g) x =  (FAPPLY f (g x)))) `,
-REPEAT GEN_TAC THEN
-DISCH_THEN (fn th => STRIP_ASSUME_TAC (BETA_RULE
-   (SPEC (Term`g:'a->'b`)  (MATCH_MP FUN_FMAP_DEF th))) THEN
-    STRIP_ASSUME_TAC (MATCH_MP FDOM_f_o th)    ) THEN
-GEN_TAC THEN
-DISCH_THEN (fn th => ASSUME_TAC (REWRITE_RULE [f_o_DEF] th) THEN
-                     FIRST_ASSUM (fn asm => ASSUME_TAC
-                           (EQ_MP (SPEC (Term`x:'a`) asm) th))) THEN
-STRIP_ASSUME_TAC  f_o_f_DEF THEN
-RES_TAC THEN
-ASM_REWRITE_TAC [f_o_DEF]);
+val FDOM_f_o = Q.store_thm 
+("FDOM_f_o",
+ `!(f:'b|->'c)  (g:'a->'b).
+     FINITE_PRED (\x. FDOM f (g x)) 
+       ==>
+     !x. FDOM (f f_o g) x = FDOM f (g x)`,
+ REPEAT GEN_TAC 
+   THEN DISCH_THEN (fn th => STRIP_ASSUME_TAC 
+          (BETA_RULE (Q.SPEC `g` (MATCH_MP FUN_FMAP_DEF th)))) 
+   THEN ASM_REWRITE_TAC [f_o_DEF,f_o_f_DEF ] 
+   THEN GEN_TAC 
+   THEN EQ_TAC 
+   THEN STRIP_TAC 
+   THEN RES_TAC 
+   THEN ASM_REWRITE_TAC []);
 
 
-val FINITE_PRED_11 = store_thm("FINITE_PRED_11",
-Term`!(g : 'a -> 'b). (!x y. (g x = g y) = (x = y)) ==>
-   !(f : ('b, 'c)fmap) .
-               FINITE_PRED (\x. FDOM f (g x))`,
-GEN_TAC THEN DISCH_TAC THEN
-INDUCT_THEN fmap_INDUCT ASSUME_TAC THENL
-[
- REWRITE_TAC [FDOM_FEMPTY, FINITE_PRED_EMPTY],
- REWRITE_TAC [FDOM_FUPDATE] THEN
- REPEAT STRIP_TAC THEN
- ASM_CASES_TAC (Term`?y. x = (g:'a -> 'b) y`) THENL
- [
-  POP_ASSUM STRIP_ASSUME_TAC THEN
-  IMP_RES_TAC FINITE_PRED_UPDATE THEN
-  POP_ASSUM (ASSUME_TAC o BETA_RULE) THEN
-  ASM_REWRITE_TAC [],
-  POP_ASSUM (ASSUME_TAC o GSYM o (CONV_RULE (DEPTH_CONV NOT_EXISTS_CONV))) THEN
-  ASM_REWRITE_TAC []
- ]
-]);
+val FAPPLY_f_o = Q.store_thm 
+("FAPPLY_f_o",
+ `!(f:'b |-> 'c)  (g:'a-> 'b).
+    FINITE_PRED (\x. FDOM f (g x)) 
+      ==>
+    !x. FDOM (f f_o g) x ==> (FAPPLY (f f_o g) x = FAPPLY f (g x))`,
+ REPEAT GEN_TAC 
+    THEN DISCH_THEN (fn th => STRIP_ASSUME_TAC 
+            (BETA_RULE (Q.SPEC `g` (MATCH_MP FUN_FMAP_DEF th)))
+    THEN STRIP_ASSUME_TAC (MATCH_MP FDOM_f_o th)) 
+    THEN GEN_TAC 
+    THEN DISCH_THEN (fn th => ASSUME_TAC (REWRITE_RULE [f_o_DEF] th) 
+            THEN FIRST_ASSUM(fn asm => ASSUME_TAC(EQ_MP (Q.SPEC `x` asm) th)))
+    THEN STRIP_ASSUME_TAC f_o_f_DEF 
+    THEN RES_TAC 
+    THEN ASM_REWRITE_TAC [f_o_DEF]);
+
+
+val FINITE_PRED_11 = Q.store_thm
+("FINITE_PRED_11",
+ `!(g:'a -> 'b). 
+      (!x y. (g x = g y) = (x = y)) 
+        ==>
+      !f:'b|->'c. FINITE_PRED (\x. FDOM f (g x))`,
+ GEN_TAC 
+   THEN DISCH_TAC 
+   THEN INDUCT_THEN fmap_INDUCT ASSUME_TAC THENL
+   [REWRITE_TAC [FDOM_FEMPTY, FINITE_PRED_EMPTY],
+    REWRITE_TAC [FDOM_FUPDATE] 
+       THEN REPEAT STRIP_TAC 
+       THEN Q.ASM_CASES_TAC `?y. x = g y` THENL
+       [POP_ASSUM STRIP_ASSUME_TAC 
+          THEN IMP_RES_TAC FINITE_PRED_UPDATE 
+          THEN POP_ASSUM (ASSUME_TAC o BETA_RULE) 
+          THEN ASM_REWRITE_TAC [],
+        POP_ASSUM (ASSUME_TAC o GSYM o CONV_RULE (DEPTH_CONV NOT_EXISTS_CONV))
+          THEN ASM_REWRITE_TAC []]]);
 
 
 val _ = export_theory();
